@prefix : <http://www.hozo.jp/owl/EXPOApr19.xml/> .
@prefix owl: <http://www.w3.org/2002/07/owl#> .
@prefix rdf: <http://www.w3.org/1999/02/22-rdf-syntax-ns#> .
@prefix xml: <http://www.w3.org/XML/1998/namespace> .
@prefix xsd: <http://www.w3.org/2001/XMLSchema#> .
@prefix rdfs: <http://www.w3.org/2000/01/rdf-schema#> .
@base <http://www.hozo.jp/owl/EXPOApr19.xml/> .

<http://www.hozo.jp/owl/EXPOApr19.xml/> rdf:type owl:Ontology ;
                                         rdfs:comment """
HOZO:OWL Export TEST
"""^^xsd:string .

#################################################################
#    Object Properties
#################################################################

###  http://www.hozo.jp/owl/EXPOApr19.xml/hasAttribute
:hasAttribute rdf:type owl:ObjectProperty ;
              rdfs:label "hasAttribute"^^xsd:string .


###  http://www.hozo.jp/owl/EXPOApr19.xml/hasPart
:hasPart rdf:type owl:ObjectProperty ;
         rdfs:label "hasPart"^^xsd:string .


###  http://www.hozo.jp/owl/EXPOApr19.xml/has_
:has_ rdf:type owl:ObjectProperty ;
      rdfs:subPropertyOf :hasPart ;
      rdfs:domain :RepresentationForm ;
      rdfs:range :Artifact .


###  http://www.hozo.jp/owl/EXPOApr19.xml/has_EXPO_concept
:has_EXPO_concept rdf:type owl:ObjectProperty ;
                  rdfs:subPropertyOf :hasPart ;
                  rdfs:domain :SynonymousExternalConcept ;
                  rdfs:range :Name .


###  http://www.hozo.jp/owl/EXPOApr19.xml/has_ExperimentalDesign
:has_ExperimentalDesign rdf:type owl:ObjectProperty ;
                        rdfs:subPropertyOf :hasPart ;
                        rdfs:domain :ScientificExperiment ;
                        rdfs:range :ExperimentalDesign .


###  http://www.hozo.jp/owl/EXPOApr19.xml/has_ID
:has_ID rdf:type owl:ObjectProperty ;
        rdfs:subPropertyOf :hasPart ;
        rdfs:domain :AdminInfoExperiment ;
        rdfs:range :IDExperiment .


###  http://www.hozo.jp/owl/EXPOApr19.xml/has_SUMO_sinonym
:has_SUMO_sinonym rdf:type owl:ObjectProperty ;
                  rdfs:subPropertyOf :hasAttribute ;
                  rdfs:domain :DomainOfExperiment ;
                  rdfs:range :SynonymousExternalConcept .


###  http://www.hozo.jp/owl/EXPOApr19.xml/has__interpretation
:has__interpretation rdf:type owl:ObjectProperty ;
                     rdfs:subPropertyOf :hasPart ;
                     rdfs:domain :ExperimentalObservation ;
                     rdfs:range :ResultsInterpretation .


###  http://www.hozo.jp/owl/EXPOApr19.xml/has__name
:has__name rdf:type owl:ObjectProperty ;
           rdfs:subPropertyOf :hasAttribute ;
           rdfs:domain :ExperimentalAction ;
           rdfs:range :ActionName .


###  http://www.hozo.jp/owl/EXPOApr19.xml/has_action_complexity
:has_action_complexity rdf:type owl:ObjectProperty ;
                       rdfs:subPropertyOf :hasAttribute ;
                       rdfs:domain :ExperimentalAction ;
                       rdfs:range :ActionComplexity .


###  http://www.hozo.jp/owl/EXPOApr19.xml/has_address
:has_address rdf:type owl:ObjectProperty ;
             rdfs:subPropertyOf :hasAttribute ;
             rdfs:domain [ rdf:type owl:Class ;
                           owl:unionOf ( :Human
                                         :Organization
                                       )
                         ] .


###  http://www.hozo.jp/owl/EXPOApr19.xml/has_admin_info
:has_admin_info rdf:type owl:ObjectProperty ;
                rdfs:subPropertyOf :hasPart ;
                rdfs:range [ rdf:type owl:Class ;
                             owl:unionOf ( :AdminInfoAuthor
                                           :AdminInfoExperiment
                                           :AdminInfoObjectOfExperiment
                                           :AdminInfoProvider
                                           :AdminInfoSubjectOfExperiment
                                           :AdminInfoSubmitter
                                           :AdminInfoUser
                                         )
                           ] .


###  http://www.hozo.jp/owl/EXPOApr19.xml/has_applicability
:has_applicability rdf:type owl:ObjectProperty ;
                   rdfs:subPropertyOf :hasPart ;
                   rdfs:domain :ExperimentalMethod ;
                   rdfs:range :MethodApplicabilityCondition .


###  http://www.hozo.jp/owl/EXPOApr19.xml/has_author
:has_author rdf:type owl:ObjectProperty ;
            rdfs:subPropertyOf :hasPart ;
            rdfs:domain [ rdf:type owl:Class ;
                          owl:unionOf ( :AdminInfoExperiment
                                        :StandardOperatingProcedure
                                      )
                        ] ;
            rdfs:range :Author .


###  http://www.hozo.jp/owl/EXPOApr19.xml/has_classification
:has_classification rdf:type owl:ObjectProperty ;
                    rdfs:subPropertyOf :hasAttribute ;
                    rdfs:domain [ rdf:type owl:Class ;
                                  owl:unionOf ( :DomainOfExperiment
                                                :ScientificExperiment
                                              )
                                ] ;
                    rdfs:range [ rdf:type owl:Class ;
                                 owl:unionOf ( :ClassificationOfDomains
                                               :ClassificationOfExperiments
                                             )
                               ] .


###  http://www.hozo.jp/owl/EXPOApr19.xml/has_complexity
:has_complexity rdf:type owl:ObjectProperty ;
                rdfs:subPropertyOf :hasAttribute ;
                rdfs:domain :ExperimentalHypothesis ;
                rdfs:range :HypothesisComplexity .


###  http://www.hozo.jp/owl/EXPOApr19.xml/has_content
:has_content rdf:type owl:ObjectProperty ;
             rdfs:subPropertyOf :hasPart ;
             rdfs:domain :Representation ;
             rdfs:range :Proposition .


###  http://www.hozo.jp/owl/EXPOApr19.xml/has_description
:has_description rdf:type owl:ObjectProperty ;
                 rdfs:subPropertyOf :hasPart ;
                 rdfs:domain :ExperimentalEquipment ;
                 rdfs:range :TechnicalDescription .


###  http://www.hozo.jp/owl/EXPOApr19.xml/has_error
:has_error rdf:type owl:ObjectProperty ;
           rdfs:subPropertyOf :hasPart ;
           rdfs:domain [ rdf:type owl:Class ;
                         owl:unionOf ( :ExperimentalObservation
                                       :ExperimentalResults
                                     )
                       ] ;
           rdfs:range [ rdf:type owl:Class ;
                        owl:unionOf ( :ObservationalError
                                      :ResultError
                                    )
                      ] .


###  http://www.hozo.jp/owl/EXPOApr19.xml/has_evaluation
:has_evaluation rdf:type owl:ObjectProperty ;
                rdfs:subPropertyOf :hasPart ;
                rdfs:domain :ExperimentalResults ;
                rdfs:range :ResultsEvaluation .


###  http://www.hozo.jp/owl/EXPOApr19.xml/has_experiment
:has_experiment rdf:type owl:ObjectProperty ;
                rdfs:subPropertyOf :hasPart ;
                rdfs:domain :ScientificInvestigation ;
                rdfs:range :ScientificExperiment .


###  http://www.hozo.jp/owl/EXPOApr19.xml/has_experimental_design
:has_experimental_design rdf:type owl:ObjectProperty ;
                         rdfs:subPropertyOf :hasPart ;
                         rdfs:domain :ScientificInvestigation ;
                         rdfs:range :ExperimentalDesign .


###  http://www.hozo.jp/owl/EXPOApr19.xml/has_experimental_factor
:has_experimental_factor rdf:type owl:ObjectProperty ;
                         rdfs:subPropertyOf :hasPart ;
                         rdfs:domain :ExperimentalModel ;
                         rdfs:range :ExperimentalFactor .


###  http://www.hozo.jp/owl/EXPOApr19.xml/has_experimental_requirements
:has_experimental_requirements rdf:type owl:ObjectProperty ;
                               rdfs:subPropertyOf :hasPart ;
                               rdfs:domain :ExperimentalTechnology ;
                               rdfs:range :ExperimentalRequirements .


###  http://www.hozo.jp/owl/EXPOApr19.xml/has_explicitness
:has_explicitness rdf:type owl:ObjectProperty ;
                  rdfs:subPropertyOf :hasAttribute ;
                  rdfs:domain :ExperimentalHypothesis ;
                  rdfs:range :HypothesisExplicitness .


###  http://www.hozo.jp/owl/EXPOApr19.xml/has_expression
:has_expression rdf:type owl:ObjectProperty ;
                rdfs:subPropertyOf :hasPart ;
                rdfs:domain :RepresentationForm ;
                rdfs:range :LinguisticExpression .


###  http://www.hozo.jp/owl/EXPOApr19.xml/has_fact
:has_fact rdf:type owl:ObjectProperty ;
          rdfs:subPropertyOf :hasPart ;
          rdfs:domain :ExperimentalResults ;
          rdfs:range [ rdf:type owl:Class ;
                       owl:unionOf ( :FactRejectResearchHypothesis
                                     :FactSupportResearchHypothesis
                                   )
                     ] .


###  http://www.hozo.jp/owl/EXPOApr19.xml/has_fax_number
:has_fax_number rdf:type owl:ObjectProperty ;
                rdfs:subPropertyOf :hasAttribute ;
                rdfs:domain [ rdf:type owl:Class ;
                              owl:unionOf ( :Human
                                            :Organization
                                          )
                            ] ;
                rdfs:range :Number .


###  http://www.hozo.jp/owl/EXPOApr19.xml/has_generality
:has_generality rdf:type owl:ObjectProperty ;
                rdfs:subPropertyOf :hasAttribute ;
                rdfs:domain :ExperimentalHypothesis ;
                rdfs:range :GeneralityOfHypothesis .


###  http://www.hozo.jp/owl/EXPOApr19.xml/has_goal
:has_goal rdf:type owl:ObjectProperty ;
          rdfs:subPropertyOf :hasPart ;
          rdfs:domain [ rdf:type owl:Class ;
                        owl:unionOf ( :ExperimentalAction
                                      :ExperimentalMethod
                                      :ScientificExperiment
                                    )
                      ] ;
          rdfs:range [ rdf:type owl:Class ;
                       owl:unionOf ( :ActionGoal
                                     :ExperimentalGoal
                                     :MethodGoal
                                   )
                     ] .


###  http://www.hozo.jp/owl/EXPOApr19.xml/has_hypothesis_formation
:has_hypothesis_formation rdf:type owl:ObjectProperty ;
                          rdfs:subPropertyOf :hasPart ;
                          rdfs:domain :ScientificInvestigation ;
                          rdfs:range :HypothesisFormation .


###  http://www.hozo.jp/owl/EXPOApr19.xml/has_hypothesis_representation
:has_hypothesis_representation rdf:type owl:ObjectProperty ;
                               rdfs:subPropertyOf :hasPart ;
                               rdfs:domain :ExperimentalHypothesis ;
                               rdfs:range :HypothesisRepresentation .


###  http://www.hozo.jp/owl/EXPOApr19.xml/has_information_gethering
:has_information_gethering rdf:type owl:ObjectProperty ;
                           rdfs:subPropertyOf :hasPart ;
                           rdfs:domain :ScientificInvestigation ;
                           rdfs:range :InformationGethering .


###  http://www.hozo.jp/owl/EXPOApr19.xml/has_inherited_variability
:has_inherited_variability rdf:type owl:ObjectProperty ;
                           rdfs:subPropertyOf :hasAttribute ;
                           rdfs:domain :Sample ;
                           rdfs:range :Variability .


###  http://www.hozo.jp/owl/EXPOApr19.xml/has_instrument
:has_instrument rdf:type owl:ObjectProperty ;
                rdfs:subPropertyOf :hasPart ;
                rdfs:domain :ExperimentalAction ;
                rdfs:range :ExperimentalEquipment .


###  http://www.hozo.jp/owl/EXPOApr19.xml/has_latest_modification
:has_latest_modification rdf:type owl:ObjectProperty ;
                         rdfs:subPropertyOf :hasAttribute ;
                         rdfs:domain :StandardOperatingProcedure ;
                         rdfs:range :TimePoint .


###  http://www.hozo.jp/owl/EXPOApr19.xml/has_login
:has_login rdf:type owl:ObjectProperty ;
           rdfs:subPropertyOf :hasAttribute ;
           rdfs:domain :User ;
           rdfs:range :LoginName .


###  http://www.hozo.jp/owl/EXPOApr19.xml/has_method
:has_method rdf:type owl:ObjectProperty ;
            rdfs:subPropertyOf :hasPart ;
            rdfs:domain :ExperimentalAction ;
            rdfs:range :ExperimentalMethod .


###  http://www.hozo.jp/owl/EXPOApr19.xml/has_model
:has_model rdf:type owl:ObjectProperty ;
           rdfs:subPropertyOf :hasPart ;
           rdfs:domain :DomainOfExperiment ;
           rdfs:range :DomainModel .


###  http://www.hozo.jp/owl/EXPOApr19.xml/has_name
:has_name rdf:type owl:ObjectProperty ;
          rdfs:subPropertyOf :hasAttribute ;
          rdfs:domain [ rdf:type owl:Class ;
                        owl:unionOf ( :AdminInfoSubjectOfExperiment
                                      :ExperimentalEquipment
                                      :Human
                                      :Organization
                                    )
                      ] ;
          rdfs:range :Name .


###  http://www.hozo.jp/owl/EXPOApr19.xml/has_number
:has_number rdf:type owl:ObjectProperty ;
            rdfs:subPropertyOf :hasAttribute ;
            rdfs:domain :GroupExperimentalObject ;
            rdfs:range :Number .


###  http://www.hozo.jp/owl/EXPOApr19.xml/has_number_of_exp._objects
:has_number_of_exp._objects rdf:type owl:ObjectProperty ;
                            rdfs:subPropertyOf :hasAttribute ;
                            rdfs:domain :ObjectOfExperiment ;
                            rdfs:range :Number .


###  http://www.hozo.jp/owl/EXPOApr19.xml/has_number_of_factors
:has_number_of_factors rdf:type owl:ObjectProperty ;
                       rdfs:subPropertyOf :hasPart ;
                       rdfs:domain :ClassificationByModel ;
                       rdfs:range :Number .


###  http://www.hozo.jp/owl/EXPOApr19.xml/has_object
:has_object rdf:type owl:ObjectProperty ;
            rdfs:subPropertyOf :hasPart ;
            rdfs:domain [ rdf:type owl:Class ;
                          owl:unionOf ( :ExperimentalAction
                                        :ExperimentalMethod
                                      )
                        ] .


###  http://www.hozo.jp/owl/EXPOApr19.xml/has_observation_characteristic
:has_observation_characteristic rdf:type owl:ObjectProperty ;
                                rdfs:subPropertyOf :hasAttribute ;
                                rdfs:domain :ExperimentalObservation ;
                                rdfs:range :StatisticsCharacteristic .


###  http://www.hozo.jp/owl/EXPOApr19.xml/has_organization
:has_organization rdf:type owl:ObjectProperty ;
                  rdfs:subPropertyOf :hasPart ;
                  rdfs:domain [ rdf:type owl:Class ;
                                owl:unionOf ( :AdminInfoExperiment
                                              :AdminInfoSubjectOfExperiment
                                              :Human
                                            )
                              ] ;
                  rdfs:range :Organization .


###  http://www.hozo.jp/owl/EXPOApr19.xml/has_origin
:has_origin rdf:type owl:ObjectProperty ;
            rdfs:subPropertyOf :hasAttribute ;
            rdfs:domain :Sample ;
            rdfs:range :ParentGroup .


###  http://www.hozo.jp/owl/EXPOApr19.xml/has_pasword
:has_pasword rdf:type owl:ObjectProperty ;
             rdfs:subPropertyOf :hasAttribute ;
             rdfs:domain :User ;
             rdfs:range :Password .


###  http://www.hozo.jp/owl/EXPOApr19.xml/has_plan
:has_plan rdf:type owl:ObjectProperty ;
          rdfs:subPropertyOf :hasPart ;
          rdfs:domain [ rdf:type owl:Class ;
                        owl:unionOf ( :ExperimentalMethod
                                      :ProcedureExecuteExperiment
                                    )
                      ] ;
          rdfs:range :PlanOfExperimentalActions .


###  http://www.hozo.jp/owl/EXPOApr19.xml/has_problem_analysis
:has_problem_analysis rdf:type owl:ObjectProperty ;
                      rdfs:subPropertyOf :hasPart ;
                      rdfs:domain :ScientificInvestigation ;
                      rdfs:range :PoblemAnalysis .


###  http://www.hozo.jp/owl/EXPOApr19.xml/has_procedure
:has_procedure rdf:type owl:ObjectProperty ;
               rdfs:subPropertyOf :hasPart ;
               rdfs:domain :StandardOperatingProcedure ;
               rdfs:range :ProcedureExecuteExperiment .


###  http://www.hozo.jp/owl/EXPOApr19.xml/has_qualification
:has_qualification rdf:type owl:ObjectProperty ;
                   rdfs:subPropertyOf :hasPart ;
                   rdfs:domain :AdminInfoSubjectOfExperiment ;
                   rdfs:range :SubjectQualification .


###  http://www.hozo.jp/owl/EXPOApr19.xml/has_reference
:has_reference rdf:type owl:ObjectProperty ;
               rdfs:subPropertyOf :hasPart ;
               rdfs:domain :AdminInfoExperiment ;
               rdfs:range :BiblioReference .


###  http://www.hozo.jp/owl/EXPOApr19.xml/has_representation
:has_representation rdf:type owl:ObjectProperty ;
                    rdfs:subPropertyOf :hasPart ;
                    rdfs:domain [ rdf:type owl:Class ;
                                  owl:unionOf ( :ExperimentalGoal
                                                :Model
                                                :ProcedureExecuteExperiment
                                              )
                                ] ;
                    rdfs:range [ rdf:type owl:Class ;
                                 owl:unionOf ( :BiblioReference
                                               :ModelRepresentation
                                               :RepresentationExperimentalExecutionProcedure
                                               :RepresentationExperimentalGoal
                                             )
                               ] .


###  http://www.hozo.jp/owl/EXPOApr19.xml/has_representation_style
:has_representation_style rdf:type owl:ObjectProperty ;
                          rdfs:subPropertyOf :hasPart ;
                          rdfs:domain :Representation ;
                          rdfs:range :RepresentationForm .


###  http://www.hozo.jp/owl/EXPOApr19.xml/has_representativeness
:has_representativeness rdf:type owl:ObjectProperty ;
                        rdfs:subPropertyOf :hasAttribute ;
                        rdfs:domain :Sample ;
                        rdfs:range :SampleRepresentativeness .


###  http://www.hozo.jp/owl/EXPOApr19.xml/has_result_evaluation
:has_result_evaluation rdf:type owl:ObjectProperty ;
                       rdfs:subPropertyOf :hasPart ;
                       rdfs:domain :ScientificInvestigation ;
                       rdfs:range :ResultsEvaluation .


###  http://www.hozo.jp/owl/EXPOApr19.xml/has_result_interpretation
:has_result_interpretation rdf:type owl:ObjectProperty ;
                           rdfs:subPropertyOf :hasPart ;
                           rdfs:domain :ScientificInvestigation ;
                           rdfs:range :ResultsInterpretation .


###  http://www.hozo.jp/owl/EXPOApr19.xml/has_sample
:has_sample rdf:type owl:ObjectProperty ;
            rdfs:subPropertyOf :hasPart ;
            rdfs:domain :GroupExperimentalObject ;
            rdfs:range :Sample .


###  http://www.hozo.jp/owl/EXPOApr19.xml/has_sample_size
:has_sample_size rdf:type owl:ObjectProperty ;
                 rdfs:subPropertyOf :hasAttribute ;
                 rdfs:domain :Sample ;
                 rdfs:range :SampleSize .


###  http://www.hozo.jp/owl/EXPOApr19.xml/has_sampling
:has_sampling rdf:type owl:ObjectProperty ;
              rdfs:subPropertyOf :hasAttribute ;
              rdfs:domain :Sample ;
              rdfs:range :SamplingMethod .


###  http://www.hozo.jp/owl/EXPOApr19.xml/has_sampling_rule
:has_sampling_rule rdf:type owl:ObjectProperty ;
                   rdfs:subPropertyOf :hasPart ;
                   rdfs:domain :SystematicSampling ;
                   rdfs:range :SamplingRule .


###  http://www.hozo.jp/owl/EXPOApr19.xml/has_standard
:has_standard rdf:type owl:ObjectProperty ;
              rdfs:subPropertyOf :hasPart ;
              rdfs:domain :ExperimentalTechnology ;
              rdfs:range :ExperimentalStandard .


###  http://www.hozo.jp/owl/EXPOApr19.xml/has_statistics_characteristic
:has_statistics_characteristic rdf:type owl:ObjectProperty ;
                               rdfs:subPropertyOf :hasAttribute ;
                               rdfs:domain :Error ;
                               rdfs:range [ rdf:type owl:Class ;
                                            owl:unionOf ( :Dispersion
                                                          :LevelOfSignificance
                                                        )
                                          ] .


###  http://www.hozo.jp/owl/EXPOApr19.xml/has_status
:has_status rdf:type owl:ObjectProperty ;
            rdfs:subPropertyOf :hasPart ;
            rdfs:domain [ rdf:type owl:Class ;
                          owl:unionOf ( :AdminInfoExperiment
                                        :ProcedureExecuteExperiment
                                      )
                        ] ;
            rdfs:range :StatusExperimentalDocument .


###  http://www.hozo.jp/owl/EXPOApr19.xml/has_strategy
:has_strategy rdf:type owl:ObjectProperty ;
              rdfs:subPropertyOf :hasPart ;
              rdfs:domain :ExperimentalTechnology ;
              rdfs:range :ExperimentalDesignStrategy .


###  http://www.hozo.jp/owl/EXPOApr19.xml/has_subgoal
:has_subgoal rdf:type owl:ObjectProperty ;
             rdfs:subPropertyOf :hasPart ;
             rdfs:domain :ExperimentalGoal ;
             rdfs:range :ExperimentalSubgoal .


###  http://www.hozo.jp/owl/EXPOApr19.xml/has_subject
:has_subject rdf:type owl:ObjectProperty ;
             rdfs:subPropertyOf :hasPart ;
             rdfs:domain [ rdf:type owl:Class ;
                           owl:unionOf ( :ExperimentalAction
                                         :ExperimentalMethod
                                       )
                         ] ;
             rdfs:range :SubjectMethod .


###  http://www.hozo.jp/owl/EXPOApr19.xml/has_synonym
:has_synonym rdf:type owl:ObjectProperty ;
             rdfs:subPropertyOf :hasAttribute ;
             rdfs:domain :BaconianExperiment ;
             rdfs:range :SynonymousExternalConcept .


###  http://www.hozo.jp/owl/EXPOApr19.xml/has_synonymousExternalConcept
:has_synonymousExternalConcept rdf:type owl:ObjectProperty ;
                               rdfs:subPropertyOf :hasPart ;
                               rdfs:domain :SynonymousExternalConcept ;
                               rdfs:range :Name .


###  http://www.hozo.jp/owl/EXPOApr19.xml/has_target_variable
:has_target_variable rdf:type owl:ObjectProperty ;
                     rdfs:subPropertyOf :hasPart ;
                     rdfs:domain :ExperimentalHypothesis ;
                     rdfs:range :TargetVariable .


###  http://www.hozo.jp/owl/EXPOApr19.xml/has_telephone_number
:has_telephone_number rdf:type owl:ObjectProperty ;
                      rdfs:subPropertyOf :hasAttribute ;
                      rdfs:domain [ rdf:type owl:Class ;
                                    owl:unionOf ( :Human
                                                  :Organization
                                                )
                                  ] ;
                      rdfs:range :Number .


###  http://www.hozo.jp/owl/EXPOApr19.xml/has_timing
:has_timing rdf:type owl:ObjectProperty ;
            rdfs:subPropertyOf :hasPart ;
            rdfs:domain :ExperimentalAction ;
            rdfs:range :TimePoint .


###  http://www.hozo.jp/owl/EXPOApr19.xml/has_title
:has_title rdf:type owl:ObjectProperty ;
           rdfs:subPropertyOf :hasPart ;
           rdfs:domain [ rdf:type owl:Class ;
                         owl:unionOf ( :AdminInfoExperiment
                                       :Human
                                     )
                       ] ;
           rdfs:range :Title .


###  http://www.hozo.jp/owl/EXPOApr19.xml/has_unknown_variable
:has_unknown_variable rdf:type owl:ObjectProperty ;
                      rdfs:subPropertyOf :hasPart ;
                      rdfs:domain :ExperimentalModel ;
                      rdfs:range :TargetVariable .


###  http://www.hozo.jp/owl/EXPOApr19.xml/has_value_of_variable_
:has_value_of_variable_ rdf:type owl:ObjectProperty ;
                        rdfs:subPropertyOf :hasPart ;
                        rdfs:domain :ValueEstimate ;
                        rdfs:range :ValueOfVariable .


###  http://www.hozo.jp/owl/EXPOApr19.xml/has_variability
:has_variability rdf:type owl:ObjectProperty ;
                 rdfs:subPropertyOf :hasAttribute ;
                 rdfs:domain :ParentGroup ;
                 rdfs:range :Variability .


###  http://www.hozo.jp/owl/EXPOApr19.xml/has_webpage
:has_webpage rdf:type owl:ObjectProperty ;
             rdfs:subPropertyOf :hasAttribute ;
             rdfs:domain [ rdf:type owl:Class ;
                           owl:unionOf ( :Human
                                         :Organization
                                       )
                         ] .


#################################################################
#    Classes
#################################################################

###  http://www.hozo.jp/owl/EXPOApr19.xml/AbductiveHypothesis
:AbductiveHypothesis rdf:type owl:Class ;
                     rdfs:subClassOf :GeneralityOfHypothesis ;
                     owl:disjointWith :InductiveHypothesis ;
                     rdfs:comment """
An abductive hypothesis is formalized as a prediction, or an explanation of an observation, usually by a propositional clause. Reference: Based on Abe A.: The Relation between Abductive Hypotheses and Inductive Hypotheses, Proc. of IJCAI97 Workshop on Abduction and Induction, pp. 1--6 (1997)
"""^^xsd:string ;
                     rdfs:label "AbductiveHypothesis"^^xsd:string .


###  http://www.hozo.jp/owl/EXPOApr19.xml/Abstract
:Abstract rdf:type owl:Class ;
          rdfs:subClassOf :Entity ;
          owl:disjointWith :Physical ;
          rdfs:comment """
\"Properties or qualities as distinguished from any particular embodiment of the properties/qualities in a physical medium. Instances of Abstract can be said to exist in the same sense as mathematical objects such as sets and relations, but they cannot exist at a particular place and time without some physical encoding or embodiment.\" (SUMO)
"""^^xsd:string ;
          rdfs:label "Abstract"^^xsd:string .


###  http://www.hozo.jp/owl/EXPOApr19.xml/Action-relatedRole
:Action-relatedRole rdf:type owl:Class ;
                    rdfs:subClassOf :Role ;
                    rdfs:comment """the concept is outside EXPO.
Actor role (Any action). For example: 
Teaching Agent role (Teaching Action),
Target object role (Action object)
"""^^xsd:string ;
                    rdfs:label "Action-relatedRole"^^xsd:string .


###  http://www.hozo.jp/owl/EXPOApr19.xml/ActionComplexity
:ActionComplexity rdf:type owl:Class ;
                  rdfs:subClassOf :AttributeOfAction ;
                  rdfs:comment """
Action complexity is an attribute of an experimental action which characterizes whether the action is composed of atomic actions.
"""^^xsd:string ;
                  rdfs:label "ActionComplexity"^^xsd:string .


###  http://www.hozo.jp/owl/EXPOApr19.xml/ActionGoal
:ActionGoal rdf:type owl:Class ;
            rdfs:subClassOf :Goal ;
            rdfs:comment """
An action goal is the state that a plan of action is intended to achieve, and that (when achieved) terminates behavior intended to achieve it. 
Reference: Based on  WordNet: http://www.cogsci.princeton.edu/cgi-bin/webwn2.0?stage=1&word=goal+
"""^^xsd:string ;
            rdfs:label "ActionGoal"^^xsd:string .


###  http://www.hozo.jp/owl/EXPOApr19.xml/ActionName
:ActionName rdf:type owl:Class ;
            rdfs:subClassOf :Name ;
            owl:disjointWith :CorporateName ,
                             :IDExperiment ,
                             :LoginName ,
                             :NameEquipment ,
                             :Password ,
                             :PersonalName ,
                             :Title ;
            rdfs:comment """
An action name is a name that refers to an action
"""^^xsd:string ;
            rdfs:label "ActionName"^^xsd:string .


###  http://www.hozo.jp/owl/EXPOApr19.xml/ActorRole
:ActorRole rdf:type owl:Class ;
           rdfs:subClassOf :Action-relatedRole ;
           rdfs:comment "the concept is outside EXPO."^^xsd:string ;
           rdfs:label "ActorRole"^^xsd:string .


###  http://www.hozo.jp/owl/EXPOApr19.xml/Adequacy
:Adequacy rdf:type owl:Class ;
          rdfs:subClassOf :StatisticsCharacteristic ;
          owl:disjointWith :Dispersion ,
                           :LevelOfSignificance ,
                           :Robustness ,
                           :Validity ;
          rdfs:comment """
The concept is outside of EXPO
"""^^xsd:string ;
          rdfs:label "Adequacy"^^xsd:string .


###  http://www.hozo.jp/owl/EXPOApr19.xml/AdminInfoAuthor
:AdminInfoAuthor rdf:type owl:Class ;
                 rdfs:subClassOf :AdministrativeInformation ;
                 owl:disjointWith :AdminInfoExperiment ,
                                  :AdminInfoObjectOfExperiment ,
                                  :AdminInfoProvider ,
                                  :AdminInfoSubjectOfExperiment ,
                                  :AdminInfoSubmitter ,
                                  :AdminInfoUser ;
                 rdfs:comment """
Administrative information about an author of an experimental data/ protocols, etc. is data about the author (a name, an organization, contact data, etc.) used for administrative purposes such as to provide/ control access/ storage of experimental data etc.
"""^^xsd:string ;
                 rdfs:label "AdminInfoAuthor"^^xsd:string .


###  http://www.hozo.jp/owl/EXPOApr19.xml/AdminInfoExperiment
:AdminInfoExperiment rdf:type owl:Class ;
                     rdfs:subClassOf :AdministrativeInformation ,
                                     [ rdf:type owl:Restriction ;
                                       owl:onProperty :has_ID ;
                                       owl:allValuesFrom :IDExperiment
                                     ] ,
                                     [ rdf:type owl:Restriction ;
                                       owl:onProperty :has_author ;
                                       owl:allValuesFrom :Author
                                     ] ,
                                     [ rdf:type owl:Restriction ;
                                       owl:onProperty :has_organization ;
                                       owl:allValuesFrom :Organization
                                     ] ,
                                     [ rdf:type owl:Restriction ;
                                       owl:onProperty :has_reference ;
                                       owl:allValuesFrom :BiblioReference
                                     ] ,
                                     [ rdf:type owl:Restriction ;
                                       owl:onProperty :has_status ;
                                       owl:allValuesFrom :StatusExperimentalDocument
                                     ] ,
                                     [ rdf:type owl:Restriction ;
                                       owl:onProperty :has_title ;
                                       owl:allValuesFrom :TitleExperiment
                                     ] ,
                                     [ rdf:type owl:Restriction ;
                                       owl:onProperty :has_ID ;
                                       owl:cardinality "1"^^xsd:nonNegativeInteger
                                     ] ;
                     owl:disjointWith :AdminInfoObjectOfExperiment ,
                                      :AdminInfoProvider ,
                                      :AdminInfoSubjectOfExperiment ,
                                      :AdminInfoSubmitter ,
                                      :AdminInfoUser ;
                     rdfs:comment """
Administrative information about an experiment is data about the experiment (status, author, last modification, etc) used for administrative purposes such as to provide/ control access/ storage of the experimental results/ protocols etc.
"""^^xsd:string ;
                     rdfs:label "AdminInfoExperiment"^^xsd:string .


###  http://www.hozo.jp/owl/EXPOApr19.xml/AdminInfoObjectOfExperiment
:AdminInfoObjectOfExperiment rdf:type owl:Class ;
                             rdfs:subClassOf :AdministrativeInformation ;
                             owl:disjointWith :AdminInfoProvider ,
                                              :AdminInfoSubjectOfExperiment ,
                                              :AdminInfoSubmitter ,
                                              :AdminInfoUser ;
                             rdfs:comment """
Administrative information about an object of an experiment is data about the object of the experiment (a name, a code, etc) used for administrative purposes such as to provide/ control access/ storage of the experimental data etc. Note that the description of an experimental object itself belongs to the corresponding domain ontology.
"""^^xsd:string ;
                             rdfs:label "AdminInfoObjectOfExperiment"^^xsd:string .


###  http://www.hozo.jp/owl/EXPOApr19.xml/AdminInfoProvider
:AdminInfoProvider rdf:type owl:Class ;
                   rdfs:subClassOf :AdministrativeInformation ;
                   owl:disjointWith :AdminInfoSubjectOfExperiment ,
                                    :AdminInfoSubmitter ,
                                    :AdminInfoUser ;
                   rdfs:comment """
administrative information about a provider of biological samples, experimental equipment etc, is data (a name, an organization, contact details etc.) used for administrative purposes such as to provide/ control access/ storage of the experimental results/ protocols etc.
"""^^xsd:string ;
                   rdfs:label "AdminInfoProvider"^^xsd:string .


###  http://www.hozo.jp/owl/EXPOApr19.xml/AdminInfoSubjectOfExperiment
:AdminInfoSubjectOfExperiment rdf:type owl:Class ;
                              rdfs:subClassOf :AdministrativeInformation ,
                                              [ rdf:type owl:Restriction ;
                                                owl:onProperty :has_name ;
                                                owl:allValuesFrom :Name
                                              ] ,
                                              [ rdf:type owl:Restriction ;
                                                owl:onProperty :has_organization ;
                                                owl:allValuesFrom :Organization
                                              ] ,
                                              [ rdf:type owl:Restriction ;
                                                owl:onProperty :has_qualification ;
                                                owl:allValuesFrom :SubjectQualification
                                              ] ;
                              owl:disjointWith :AdminInfoSubmitter ,
                                               :AdminInfoUser ;
                              rdfs:comment """
Administrative information about a subject of an experiment is data about the subject of the experiment (a name, qualification, an organization, etc) used for administrative purposes such as to provide/ control storage of the experimental data etc.
"""^^xsd:string ;
                              rdfs:label "AdminInfoSubjectOfExperiment"^^xsd:string .


###  http://www.hozo.jp/owl/EXPOApr19.xml/AdminInfoSubmitter
:AdminInfoSubmitter rdf:type owl:Class ;
                    rdfs:subClassOf :AdministrativeInformation ;
                    owl:disjointWith :AdminInfoUser ;
                    rdfs:comment """
Administrative information about a submitter of an experimental data/ protocols, etc. is data about the submitter (a name, an organization, contact data, etc.) used for administrative purposes such as to provide/ control access/ storage of experimental data etc.
"""^^xsd:string ;
                    rdfs:label "AdminInfoSubmitter"^^xsd:string .


###  http://www.hozo.jp/owl/EXPOApr19.xml/AdminInfoUser
:AdminInfoUser rdf:type owl:Class ;
               rdfs:subClassOf :AdministrativeInformation ;
               rdfs:comment """
Administrative information about a user of an experimental data/ protocols, etc. is data about the user (a name, an organization, contact data, login, password, etc.) used for administrative purposes such as to provide/ control access to experimental data etc.
"""^^xsd:string ;
               rdfs:label "AdminInfoUser"^^xsd:string .


###  http://www.hozo.jp/owl/EXPOApr19.xml/AdministrativeInformation
:AdministrativeInformation rdf:type owl:Class ;
                           rdfs:subClassOf :Proposition ;
                           owl:disjointWith :ExperimentalDesignStrategy ,
                                            :ExperimentalHypothesis ,
                                            :ExperimentalStandard ,
                                            :ExperimentalTechnology ,
                                            :Fact ,
                                            :FieldOfStudy ,
                                            :Model ,
                                            :ModelAssumption ,
                                            :Procedure ,
                                            :Requirements ,
                                            :ScientificTask ,
                                            :SubjectQualification ,
                                            :ValueOfVariable ,
                                            :Variable ;
                           rdfs:comment """
administrative information is data about an experimental subject, an experimental object, experimental documents etc., used for administrative purposes such as to provide/ control access/ storage of the experimental results/ protocols etc.
"""^^xsd:string ;
                           rdfs:label "AdministrativeInformation"^^xsd:string .


###  http://www.hozo.jp/owl/EXPOApr19.xml/Agent
:Agent rdf:type owl:Class ;
       rdfs:subClassOf :Object ;
       rdfs:comment """
\"Something or someone that can act on its own and produce changes in the world.\" (SUMO)
"""^^xsd:string ;
       rdfs:label "Agent"^^xsd:string .


###  http://www.hozo.jp/owl/EXPOApr19.xml/AlternativeHypothesis
:AlternativeHypothesis rdf:type owl:Class ;
                       rdfs:subClassOf :ExperimentalHypothesis ;
                       owl:disjointWith :NullHypothesis ,
                                        :ResearchHypothesis ;
                       rdfs:comment """
An alternative hypothesis an experimental hypothesis that states that factors different from the known controlled variables have specified effect on the unknown (target) variables of the domain.
"""^^xsd:string ;
                       rdfs:label "AlternativeHypothesis"^^xsd:string .


###  http://www.hozo.jp/owl/EXPOApr19.xml/Article
:Article rdf:type owl:Class ;
         rdfs:subClassOf :Text ;
         rdfs:comment """
\"A relatively short Text that either is unbound or is bound with other Articles in a Book.\"
Reference: SUMO: http://www.ontologyportal.org/
"""^^xsd:string ;
         rdfs:label "Article"^^xsd:string .


###  http://www.hozo.jp/owl/EXPOApr19.xml/Artifact
:Artifact rdf:type owl:Class ;
          rdfs:subClassOf :CorpuscularObject ;
          rdfs:comment """
\"A CorpuscularObject that is the product of a Making.\"
"""^^xsd:string ;
          rdfs:label "Artifact"^^xsd:string .


###  http://www.hozo.jp/owl/EXPOApr19.xml/ArtificialLanguage
:ArtificialLanguage rdf:type owl:Class ;
                    rdfs:subClassOf :Language ;
                    owl:disjointWith :HumanLanguage ;
                    rdfs:comment """
\"The subclass of Languages that are designed by Humans.\"SUMO: http://www.ontologyportal.org/
"""^^xsd:string ;
                    rdfs:label "ArtificialLanguage"^^xsd:string .


###  http://www.hozo.jp/owl/EXPOApr19.xml/AtomicAction
:AtomicAction rdf:type owl:Class ;
              rdfs:subClassOf :ActionComplexity ;
              owl:disjointWith :ComplexAction ;
              rdfs:comment """
An atomic action is an experimental action which is not decomposed on sub actions in terms of the domain.
"""^^xsd:string ;
              rdfs:label "AtomicAction"^^xsd:string .


###  http://www.hozo.jp/owl/EXPOApr19.xml/Attribute
:Attribute rdf:type owl:Class ;
           rdfs:subClassOf :Abstract ;
           owl:disjointWith :Proposition ,
                            :Quantity ,
                            :Relation ;
           rdfs:comment """
The concept is outside of EXPO.
\"Qualities which we cannot or choose not to reify into subclasses of Object.\" Reference: SUMO http://berkelium.teknowledge.com:8080/sigma/home.jsp
"""^^xsd:string ;
           rdfs:label "Attribute"^^xsd:string .


###  http://www.hozo.jp/owl/EXPOApr19.xml/AttributeGroup
:AttributeGroup rdf:type owl:Class ;
                rdfs:subClassOf :Attribute ;
                owl:disjointWith :AttributeOfAction ,
                                 :AttributeOfDocument ,
                                 :AttributeOfHypothesis ,
                                 :AttributeOfModel ,
                                 :AttributeOfVariable ,
                                 :Name ,
                                 :StatisticsCharacteristic ;
                rdfs:comment """
An attribute of a group is an essential characteristic of a group, e.g. <variability>.
"""^^xsd:string ;
                rdfs:label "AttributeGroup"^^xsd:string .


###  http://www.hozo.jp/owl/EXPOApr19.xml/AttributeOfAction
:AttributeOfAction rdf:type owl:Class ;
                   rdfs:subClassOf :Attribute ;
                   owl:disjointWith :AttributeOfDocument ,
                                    :AttributeOfHypothesis ,
                                    :AttributeOfModel ,
                                    :AttributeOfVariable ,
                                    :Name ,
                                    :StatisticsCharacteristic ;
                   rdfs:comment """
An attribute of an action is an essential characteristic of an experimental action, e.g. <action complexity>.
"""^^xsd:string ;
                   rdfs:label "AttributeOfAction"^^xsd:string .


###  http://www.hozo.jp/owl/EXPOApr19.xml/AttributeOfDocument
:AttributeOfDocument rdf:type owl:Class ;
                     rdfs:subClassOf :Attribute ;
                     owl:disjointWith :AttributeOfHypothesis ,
                                      :AttributeOfModel ,
                                      :AttributeOfVariable ,
                                      :Name ,
                                      :StatisticsCharacteristic ;
                     rdfs:comment """
An attribute of a document is an essential characteristic of a document, e.g. <status>.
"""^^xsd:string ;
                     rdfs:label "AttributeOfDocument"^^xsd:string .


###  http://www.hozo.jp/owl/EXPOApr19.xml/AttributeOfHypothesis
:AttributeOfHypothesis rdf:type owl:Class ;
                       rdfs:subClassOf :Attribute ;
                       owl:disjointWith :AttributeOfModel ,
                                        :AttributeOfVariable ,
                                        :Name ,
                                        :StatisticsCharacteristic ;
                       rdfs:comment """
An attribute of an hypothesis is an essential characteristic of an experimental hypothesis, e.g. <explicitness of an hypothesis>, <complexity of an hypothesis>.
"""^^xsd:string ;
                       rdfs:label "AttributeOfHypothesis"^^xsd:string .


###  http://www.hozo.jp/owl/EXPOApr19.xml/AttributeOfModel
:AttributeOfModel rdf:type owl:Class ;
                  rdfs:subClassOf :Attribute ;
                  owl:disjointWith :AttributeOfVariable ,
                                   :Name ,
                                   :StatisticsCharacteristic ;
                  rdfs:comment """
An attribute of a model is an essential characteristic of an experimental model, e.g. <dynamism of a model>, <order of a model>.
"""^^xsd:string ;
                  rdfs:label "AttributeOfModel"^^xsd:string .


###  http://www.hozo.jp/owl/EXPOApr19.xml/AttributeOfVariable
:AttributeOfVariable rdf:type owl:Class ;
                     rdfs:subClassOf :Attribute ;
                     owl:disjointWith :Name ,
                                      :StatisticsCharacteristic ;
                     rdfs:comment """
An attribute of a variable is an essential characteristic of a variable, e.g. <independence>, <controllability>.
"""^^xsd:string ;
                     rdfs:label "AttributeOfVariable"^^xsd:string .


###  http://www.hozo.jp/owl/EXPOApr19.xml/AttributeRole
:AttributeRole rdf:type owl:Class ;
               rdfs:subClassOf :Role ;
               rdfs:comment """
Ex: Height role: played by length (it depends on how to put, say, a cube)
"""^^xsd:string ;
               rdfs:label "AttributeRole"^^xsd:string .


###  http://www.hozo.jp/owl/EXPOApr19.xml/AttributeSample
:AttributeSample rdf:type owl:Class ;
                 rdfs:subClassOf :AttributeGroup ;
                 owl:disjointWith :Variability ;
                 rdfs:comment """
An attribute of a sample is an essential characteristic of a sample, e.g. <representativeness>.
"""^^xsd:string ;
                 rdfs:label "AttributeSample"^^xsd:string .


###  http://www.hozo.jp/owl/EXPOApr19.xml/Author
:Author rdf:type owl:Class ;
        rdfs:subClassOf :SubjectRole ,
                        [ rdf:type owl:Restriction ;
                          owl:onProperty :has_admin_info ;
                          owl:allValuesFrom :AdminInfoAuthor
                        ] ,
                        [ rdf:type owl:Restriction ;
                          owl:onProperty :has_admin_info ;
                          owl:cardinality "1"^^xsd:nonNegativeInteger
                        ] ;
        rdfs:comment """
An author of an experimental document is the person (or a group) who developed the document or on whose authority the document is made. Reference: Based on The Oxford English Dictionary. Oxford University Press, 2 Ed., 1989
"""^^xsd:string ;
        rdfs:label "Author"^^xsd:string .


###  http://www.hozo.jp/owl/EXPOApr19.xml/AuthorProtocol
:AuthorProtocol rdf:type owl:Class ;
                rdfs:subClassOf :Author ;
                rdfs:comment """
An author of a protocol is the person (or a group) who developed the protocol.
"""^^xsd:string ;
                rdfs:label "AuthorProtocol"^^xsd:string .


###  http://www.hozo.jp/owl/EXPOApr19.xml/AuthorSOP
:AuthorSOP rdf:type owl:Class ;
           rdfs:subClassOf :Author ;
           rdfs:comment """
An author of a SOP is the person (or a group) on whose authority the SOP is made. Reference: Based on The Oxford English Dictionary. Oxford University Press, 2 Ed., 1989
"""^^xsd:string ;
           rdfs:label "AuthorSOP"^^xsd:string .


###  http://www.hozo.jp/owl/EXPOApr19.xml/BaconianExperiment
:BaconianExperiment rdf:type owl:Class ;
                    rdfs:subClassOf :PhysicalExperiment ,
                                    [ rdf:type owl:Restriction ;
                                      owl:onProperty :has_synonym ;
                                      owl:allValuesFrom :SynonymousExternalConcept
                                    ] ,
                                    [ rdf:type owl:Restriction ;
                                      owl:onProperty :has_synonym ;
                                      owl:cardinality "1"^^xsd:nonNegativeInteger
                                    ] ;
                    rdfs:comment """
A Baconian experiment is a scientific experiment which involves no explicit hypothesis. Reference: Medawar, P.B. Advice to a Young Scientist. Pan Books Ltd, London, 1981
"""^^xsd:string ;
                    rdfs:label "BaconianExperiment"^^xsd:string .


###  http://www.hozo.jp/owl/EXPOApr19.xml/BiblioReference
:BiblioReference rdf:type owl:Class ;
                 rdfs:subClassOf :Reference ;
                 rdfs:comment """
The concept is outside EXPO
"""^^xsd:string ;
                 rdfs:label "BiblioReference"^^xsd:string .


###  http://www.hozo.jp/owl/EXPOApr19.xml/Book
:Book rdf:type owl:Class ;
      rdfs:subClassOf :Text ;
      rdfs:comment """
\"A Text that has pages and is bound.\" 
Reference: SUMO: http://www.ontologyportal.org/
"""^^xsd:string ;
      rdfs:label "Book"^^xsd:string .


###  http://www.hozo.jp/owl/EXPOApr19.xml/CalculableVariable
:CalculableVariable rdf:type owl:Class ;
                    rdfs:subClassOf :Variable ;
                    rdfs:comment """
A calculable variable is a variable where there is an algorithm to determine the value of the variable. Reference: based on Albar`ede, P. A theory of experiment. http://66.102.9.104/search?q=cache:ECOW7jEPfHAJ: arxiv.org/pdf/cs.AI/0201022++a+theory+of+experiment+Albarede&hl=en
"""^^xsd:string ;
                    rdfs:label "CalculableVariable"^^xsd:string .


###  http://www.hozo.jp/owl/EXPOApr19.xml/CapacityRequirements
:CapacityRequirements rdf:type owl:Class ;
                      rdfs:subClassOf :ExperimentalRequirements ;
                      owl:disjointWith :EnvironmentalRequirements ,
                                       :FinancialRequirements ;
                      rdfs:comment """
Capacity requirements are the ability of the experimental equipment, legal competency, qualification, and the ability of a subject of the experiment to provide execution of experimental actions in order to achieve an experimental goal. Reference: Based on The Oxford English Dictionary. Oxford University Press, 2 Ed., 1989
"""^^xsd:string ;
                      rdfs:label "CapacityRequirements"^^xsd:string .


###  http://www.hozo.jp/owl/EXPOApr19.xml/Classification
:Classification rdf:type owl:Class ;
                rdfs:subClassOf :ScientificTask ;
                owl:disjointWith :EperimentalDesignTask ,
                                 :HypothesisFormation ,
                                 :InformationGethering ,
                                 :PoblemAnalysis ,
                                 :ResultsEvaluation ,
                                 :ResultsInterpretation ;
                rdfs:comment """
Classification is the scientific task of forming a hierarchical system of categories.
"""^^xsd:string ;
                rdfs:label "Classification"^^xsd:string .


###  http://www.hozo.jp/owl/EXPOApr19.xml/ClassificationByDomain
:ClassificationByDomain rdf:type owl:Class ;
                        rdfs:subClassOf :ClassificationOfExperiments ;
                        owl:disjointWith :ClassificationByModel ;
                        rdfs:comment """
A classification by a domain is a hierarchical system of categories  - types of experiments  - according to their domains, e.g. microarray experiment, proteomic experiment.
"""^^xsd:string ;
                        rdfs:label "ClassificationByDomain"^^xsd:string .


###  http://www.hozo.jp/owl/EXPOApr19.xml/ClassificationByModel
:ClassificationByModel rdf:type owl:Class ;
                       rdfs:subClassOf :ClassificationOfExperiments ,
                                       [ rdf:type owl:Restriction ;
                                         owl:onProperty :has_number_of_factors ;
                                         owl:allValuesFrom :Number
                                       ] ,
                                       [ rdf:type owl:Restriction ;
                                         owl:onProperty :has_number_of_factors ;
                                         owl:cardinality "1"^^xsd:nonNegativeInteger
                                       ] ;
                       rdfs:comment """
The classification by a model is a hierarchical system of categories  - types of experiments  - according to amount of factors in the design of the experiments, for instance <one-factor experiment >, <two-factor experiment>, <multi-factor experiment>.
"""^^xsd:string ;
                       rdfs:label "ClassificationByModel"^^xsd:string .


###  http://www.hozo.jp/owl/EXPOApr19.xml/ClassificationOfDomains
:ClassificationOfDomains rdf:type owl:Class ;
                         rdfs:subClassOf :Classification ;
                         owl:disjointWith :ClassificationOfExperiments ;
                         rdfs:comment """
A classification of domains is a hierarchical system of categories  - scientific domains.
"""^^xsd:string ;
                         rdfs:label "ClassificationOfDomains"^^xsd:string .


###  http://www.hozo.jp/owl/EXPOApr19.xml/ClassificationOfExperiments
:ClassificationOfExperiments rdf:type owl:Class ;
                             rdfs:subClassOf :Classification ;
                             rdfs:comment """
A classification of experiments is a hierarchical system of categories  - types of experiments  - according to their domains or used models of experiments.
"""^^xsd:string ;
                             rdfs:label "ClassificationOfExperiments"^^xsd:string .


###  http://www.hozo.jp/owl/EXPOApr19.xml/Classifying
:Classifying rdf:type owl:Class ;
             rdfs:subClassOf :ScientificActivity ;
             owl:disjointWith :DesigningExperiment ,
                              :ExecutionOfExperiment ,
                              :FormingClassificationSystem ,
                              :HypothesisForming ,
                              :InterpretingResult ,
                              :ProcessProblemAnalysis ,
                              :ResultEvaluating ;
             rdfs:comment """
A process of classification is the act of classifying into given classes according to common characteristics. Reference:The Oxford English Dictionary. Oxford University Press, 2 Ed., 1989
SUMO: \"The Class of IntentionalPsychologicalProcesses which involve attaching a name or category to a thing or set of things. Note that Classifying is distinguished from Learning by the fact that the latter covers the acquisition by a CognitiveAgent of any Proposition, while the former involves the assignment of a label or category.\"
"""^^xsd:string ;
             rdfs:label "Classifying"^^xsd:string .


###  http://www.hozo.jp/owl/EXPOApr19.xml/CoarseError
:CoarseError rdf:type owl:Class ;
             rdfs:subClassOf :MeasurementError ;
             rdfs:comment """
A coarse error is a measurement error which occurs through incorrect use of an instrument. Reference: Arley, N. & Buch , K.R., Introduction to the theory of probability and statistics. New York : Wiley London. Chapman & Hall, 1950. 236p.
"""^^xsd:string ;
             rdfs:label "CoarseError"^^xsd:string .


###  http://www.hozo.jp/owl/EXPOApr19.xml/Collection
:Collection rdf:type owl:Class ;
            rdfs:subClassOf :Object ;
            rdfs:comment """
\"Collections have members like Classes, but, unlike Classes, they have a position in space-time and members can be added and subtracted without thereby changing the identity of the Collection. Some examples are toolkits, football teams, and flocks of sheep.\" (SUMO)
"""^^xsd:string ;
            rdfs:label "Collection"^^xsd:string .


###  http://www.hozo.jp/owl/EXPOApr19.xml/ComparisonControl_TargetGroups
:ComparisonControl_TargetGroups rdf:type owl:Class ;
                                rdfs:subClassOf :PairedComparison ;
                                owl:disjointWith :PairedComparisonOfMatchingGroups ,
                                                 :PairedComparisonOfSingleSampleGroups ;
                                rdfs:comment """
A comparison control/ target groups is a paired comparison experimental design strategy where two groups of experimental objects are used, a control group which is not affected by experimental factor(s), and a target group which is affected by the experimental factor(s).
"""^^xsd:string ;
                                rdfs:label "ComparisonControl/TargetGroups"^^xsd:string .


###  http://www.hozo.jp/owl/EXPOApr19.xml/ComplexAction
:ComplexAction rdf:type owl:Class ;
               rdfs:subClassOf :ActionComplexity ;
               rdfs:comment """
A complex action is a composition of atomic actions.
"""^^xsd:string ;
               rdfs:label "ComplexAction"^^xsd:string .


###  http://www.hozo.jp/owl/EXPOApr19.xml/ComplexHypothesis
:ComplexHypothesis rdf:type owl:Class ;
                   rdfs:subClassOf :HypothesisComplexity ;
                   owl:disjointWith :SingleHypothesis ;
                   rdfs:comment """
A complex hypothesis of an experimental hypothesis is a Boolean attribute which is false where the hypothesis can be formalized by a single clause.
"""^^xsd:string ;
                   rdfs:label "ComplexHypothesis"^^xsd:string .


###  http://www.hozo.jp/owl/EXPOApr19.xml/ComputationalData
:ComputationalData rdf:type owl:Class ;
                   rdfs:subClassOf :ExperimentalObservation ;
                   rdfs:comment """
Computational data is experimental observations \"represented in a form suitable for processing by computer.\" Reference: WordNet: http://www.answers.com
"""^^xsd:string ;
                   rdfs:label "ComputationalData"^^xsd:string .


###  http://www.hozo.jp/owl/EXPOApr19.xml/ComputationalExperiment
:ComputationalExperiment rdf:type owl:Class ;
                         rdfs:subClassOf :ScientificExperiment ;
                         rdfs:comment """
A computational experiment is a scientific experiment which investigates cause-effect relations between known and unknown (target) variables by manipulating the computational (non-physical) domain adequate to the real-world domain.
"""^^xsd:string ;
                         rdfs:label "ComputationalExperiment"^^xsd:string .


###  http://www.hozo.jp/owl/EXPOApr19.xml/ComputeGoal
:ComputeGoal rdf:type owl:Class ;
             rdfs:subClassOf :ExperimentalGoal ;
             owl:disjointWith :ConfirmGoal ,
                              :ExplainGoal ,
                              :InvestigateGoal ;
             rdfs:comment """
A compute-goal is an experimental goal of a computational experiment.
"""^^xsd:string ;
             rdfs:label "ComputeGoal"^^xsd:string .


###  http://www.hozo.jp/owl/EXPOApr19.xml/ComputerSimulation
:ComputerSimulation rdf:type owl:Class ;
                    rdfs:subClassOf :ComputationalExperiment ;
                    rdfs:comment """
Computer simulation is a computational experiment where the real domain of study is modeling by a computer program imitating the internal processes and not merely the results of the thing being simulated\".
Reference: The Free Dictionary: http://www.thefreedictionary.com/computer+simulation
"""^^xsd:string ;
                    rdfs:label "ComputerSimulation"^^xsd:string .


###  http://www.hozo.jp/owl/EXPOApr19.xml/ConfirmGoal
:ConfirmGoal rdf:type owl:Class ;
             rdfs:subClassOf :ExperimentalGoal ;
             owl:disjointWith :ExplainGoal ,
                              :InvestigateGoal ;
             rdfs:comment """
A confirm-goal is an experimental goal of a hypothesis-driven experiment.
"""^^xsd:string ;
             rdfs:label "ConfirmGoal"^^xsd:string .


###  http://www.hozo.jp/owl/EXPOApr19.xml/ConstantQuantity
:ConstantQuantity rdf:type owl:Class ;
                  rdfs:subClassOf :PhysicalQuantity ;
                  owl:disjointWith :TimeMeasure ;
                  rdfs:comment """
\"A ConstantQuantity is a PhysicalQuantity which has a constant value, e.g. 3 meters and 5 hours. The magnitude (see MagnitudeFn) of every ConstantQuantity is a RealNumber. ConstantQuantities are distinguished from FunctionQuantities, which map ConstantQuantities to other ConstantQuantities. All ConstantQuantites are expressed with the BinaryFunction MeasureFn, which takes a Number and a UnitOfMeasure as arguments. For example, 3 Meters can be expressed as (MeasureFn 3 Meter). ConstantQuantities form a partial order (see PartialOrderingRelation) with the lessThan relation, since lessThan is a RelationExtendedToQuantities and lessThan is defined over the RealNumbers. The lessThan relation is not a total order (see TotalOrderingRelation) over the class ConstantQuantity since elements of some subclasses of ConstantQuantity (such as length quantities) are incomparable to elements of other subclasses of ConstantQuantity (such as mass quantities).\" (SUMO)
"""^^xsd:string ;
                  rdfs:label "ConstantQuantity"^^xsd:string .


###  http://www.hozo.jp/owl/EXPOApr19.xml/ContentBearingObject
:ContentBearingObject rdf:type owl:Class ;
                      rdfs:subClassOf :ContentBearingPhysical ;
                      owl:disjointWith :LinguisticExpression ;
                      rdfs:comment """
\"Any SelfConnectedObject that expresses content. This content may be a Proposition, e.g. when the ContentBearingObject is a Sentence or Text, or it may be a representation of an abstract or physical object, as with an Icon, a Word or a Phrase.\" (SUMO)
"""^^xsd:string ;
                      rdfs:label "ContentBearingObject"^^xsd:string .


###  http://www.hozo.jp/owl/EXPOApr19.xml/ContentBearingPhysical
:ContentBearingPhysical rdf:type owl:Class ;
                        rdfs:subClassOf :Physical ;
                        owl:disjointWith :Object ,
                                         :Process ;
                        rdfs:comment """
\"Any Object or Process that expresses content. This covers Objects that contain a Proposition, such as a book, as well as ManualSignLanguage, which may similarly contain a Proposition.\" (SUMO)
"""^^xsd:string ;
                        rdfs:label "ContentBearingPhysical"^^xsd:string .


###  http://www.hozo.jp/owl/EXPOApr19.xml/Controllability
:Controllability rdf:type owl:Class ;
                 rdfs:subClassOf :AttributeOfVariable ;
                 owl:disjointWith :Independence ;
                 rdfs:comment """
Controllability of a variable is an attribute which characterize whether a subject of the experiment can control/ vary the variable.
"""^^xsd:string ;
                 rdfs:label "Controllability"^^xsd:string .


###  http://www.hozo.jp/owl/EXPOApr19.xml/CorporateName
:CorporateName rdf:type owl:Class ;
               rdfs:subClassOf :Name ;
               owl:disjointWith :IDExperiment ,
                                :LoginName ,
                                :NameEquipment ,
                                :Password ,
                                :PersonalName ,
                                :Title ;
               rdfs:comment """
The concept is outside of EXPO
"""^^xsd:string ;
               rdfs:label "CorporateName"^^xsd:string .


###  http://www.hozo.jp/owl/EXPOApr19.xml/CorpuscularObject
:CorpuscularObject rdf:type owl:Class ;
                   rdfs:subClassOf :SelfConnectedObject ;
                   rdfs:comment """
\"A SelfConnectedObject whose parts have properties that are not shared by the whole.\" (SUMO)
"""^^xsd:string ;
                   rdfs:label "CorpuscularObject"^^xsd:string .


###  http://www.hozo.jp/owl/EXPOApr19.xml/DBReference
:DBReference rdf:type owl:Class ;
             rdfs:subClassOf :Reference ;
             rdfs:comment """
The concept is outside EXPO
"""^^xsd:string ;
             rdfs:label "DBReference"^^xsd:string .


###  http://www.hozo.jp/owl/EXPOApr19.xml/DDC_Dewey_Classification
:DDC_Dewey_Classification rdf:type owl:Class ;
                          rdfs:subClassOf :ClassificationOfDomains ;
                          owl:disjointWith :LibraryOfCongressClassification ,
                                           :NLMClassification ,
                                           :ResearchCouncilsUKClassification ;
                          rdfs:comment """
The Dewey Decimal Classification (DDC) is a system of library classification developed by Melvil Dewey (1851 - 1931) in 1876, and since greatly modified and expanded in the course of twenty-two major revisions occurred until 2004. Reference: Wikipedia: http://en.wikipedia.org/wiki/Dewey_Decimal_Classification
"""^^xsd:string ;
                          rdfs:label "DDC(Dewey)Classification"^^xsd:string .


###  http://www.hozo.jp/owl/EXPOApr19.xml/DataRepresentationStandard
:DataRepresentationStandard rdf:type owl:Class ;
                            rdfs:subClassOf :ExperimentalStandard ;
                            rdfs:comment """
A data representation standard is an accepted way of representing experimental data, e.g. the MIAME standard for representation of microarray experimental data.
"""^^xsd:string ;
                            rdfs:label "DataRepresentationStandard"^^xsd:string .


###  http://www.hozo.jp/owl/EXPOApr19.xml/DegreeOfModel
:DegreeOfModel rdf:type owl:Class ;
               rdfs:subClassOf :AttributeOfModel ;
               owl:disjointWith :DynamismOfModel ;
               rdfs:comment """
A degree of a model is an attribute of a model which characterizes the dependency between its variables. For instance: a <linear model>, a <nonlinear model>.
"""^^xsd:string ;
               rdfs:label "DegreeOfModel"^^xsd:string .


###  http://www.hozo.jp/owl/EXPOApr19.xml/DependentVariable
:DependentVariable rdf:type owl:Class ;
                   rdfs:subClassOf :Independence ;
                   rdfs:comment """
The concept is outside of EXPO
"""^^xsd:string ;
                   rdfs:label "DependentVariable"^^xsd:string .


###  http://www.hozo.jp/owl/EXPOApr19.xml/DesigningExperiment
:DesigningExperiment rdf:type owl:Class ;
                     rdfs:subClassOf :ScientificActivity ;
                     owl:disjointWith :ExecutionOfExperiment ,
                                      :FormingClassificationSystem ,
                                      :HypothesisForming ,
                                      :InterpretingResult ,
                                      :ProcessProblemAnalysis ,
                                      :ResultEvaluating ;
                     rdfs:comment """
Designing an experiment is the act of determining the relationship between factors affecting cause-effect relations between known and unknown variables. Reference: Based on Sigma: http://www.isixsigma.com/dictionary/Design_of_Experiments_-_DOE-41.htm
"""^^xsd:string ;
                     rdfs:label "DesigningExperiment"^^xsd:string .


###  http://www.hozo.jp/owl/EXPOApr19.xml/Device
:Device rdf:type owl:Class ;
        rdfs:subClassOf :ExperimentalEquipment ;
        rdfs:comment """
A device is an experimental equipment that processes data according to a set of instructions. Reference: Collins Softback English Dictionary, HarperCollins Publishers, Glasgow, 1993.
SUMO: \"A Device is an Artifact whose purpose is to serve as an instrument in a specific subclass of Process.\"
"""^^xsd:string ;
        rdfs:label "Device"^^xsd:string .


###  http://www.hozo.jp/owl/EXPOApr19.xml/Dispersion
:Dispersion rdf:type owl:Class ;
            rdfs:subClassOf :StatisticsCharacteristic ;
            owl:disjointWith :LevelOfSignificance ,
                             :Robustness ,
                             :Validity ;
            rdfs:comment """
The concept is outside of EXPO
"""^^xsd:string ;
            rdfs:label "Dispersion"^^xsd:string .


###  http://www.hozo.jp/owl/EXPOApr19.xml/DocumentStage
:DocumentStage rdf:type owl:Class ;
               rdfs:subClassOf :StatusExperimentalDocument ;
               owl:disjointWith :PermissionStatus ;
               rdfs:comment """
A document stage is a status of an experimental document that specifies the current stage of development of the document, e.g. <draft>.
"""^^xsd:string ;
               rdfs:label "DocumentStage"^^xsd:string .


###  http://www.hozo.jp/owl/EXPOApr19.xml/DomainAction
:DomainAction rdf:type owl:Class ;
              rdfs:subClassOf :ExperimentalAction ;
              rdfs:comment """
A domain action is a manipulation in the domain of the experiment.
"""^^xsd:string ;
              rdfs:label "DomainAction"^^xsd:string .


###  http://www.hozo.jp/owl/EXPOApr19.xml/DomainModel
:DomainModel rdf:type owl:Class ;
             rdfs:subClassOf :Model ;
             owl:disjointWith :ExperimentalModel ;
             rdfs:comment """
A domain model is a description of relationships (e.g. logical/ mathematical) between known and unknown variables of the experimental domain.
"""^^xsd:string ;
             rdfs:label "DomainModel"^^xsd:string .


###  http://www.hozo.jp/owl/EXPOApr19.xml/DomainOfExperiment
:DomainOfExperiment rdf:type owl:Class ;
                    rdfs:subClassOf :FieldOfStudy ,
                                    [ rdf:type owl:Restriction ;
                                      owl:onProperty :has_SUMO_sinonym ;
                                      owl:allValuesFrom :SynonymousExternalConcept
                                    ] ,
                                    [ rdf:type owl:Restriction ;
                                      owl:onProperty :has_classification ;
                                      owl:allValuesFrom :ClassificationOfDomains
                                    ] ,
                                    [ rdf:type owl:Restriction ;
                                      owl:onProperty :has_model ;
                                      owl:allValuesFrom :DomainModel
                                    ] ;
                    owl:disjointWith :RelatedDomain ;
                    rdfs:comment """
A domain of an experiment is a field of study in which an experiment is designed to discover new knowledge.
"""^^xsd:string ;
                    rdfs:label "DomainOfExperiment"^^xsd:string .


###  http://www.hozo.jp/owl/EXPOApr19.xml/DoseResponse
:DoseResponse rdf:type owl:Class ;
              rdfs:subClassOf :ComparisonControl_TargetGroups ;
              owl:disjointWith :GeneKnock-in ,
                               :GeneKnock-out ,
                               :Normal_Disease ,
                               :TimeCourse ,
                               :Treated_Untreated ;
              rdfs:comment """
A dose response design strategy is a sub-class of a comparison control/ target groups strategy where a target group receives a specified dose of a specified treatment.
"""^^xsd:string ;
              rdfs:label "DoseResponse"^^xsd:string .


###  http://www.hozo.jp/owl/EXPOApr19.xml/DraftStatus
:DraftStatus rdf:type owl:Class ;
             rdfs:subClassOf :DocumentStage ;
             rdfs:comment """
A draft status means that the current SOP or a protocol is a preliminary description.
"""^^xsd:string ;
             rdfs:label "DraftStatus"^^xsd:string .


###  http://www.hozo.jp/owl/EXPOApr19.xml/DuhemEffect
:DuhemEffect rdf:type owl:Class ;
             rdfs:subClassOf :ExperimentalDesignEffect ;
             owl:disjointWith :InstrumentationEffect ;
             rdfs:comment """
A Duhem effect is an experimental design effect where an effect on the experimental results is due to an inconsistency between the physical world and the domain model. Reference: Philosophy of science: the central issues. Eds. Martine Curd, J.A. Cover, W.W. Norton & Co. N.Y. 1998.
"""^^xsd:string ;
             rdfs:label "DuhemEffect"^^xsd:string .


###  http://www.hozo.jp/owl/EXPOApr19.xml/DynamicModel
:DynamicModel rdf:type owl:Class ;
              rdfs:subClassOf :DynamismOfModel ;
              owl:disjointWith :StaticModel ;
              rdfs:comment """
A dynamic model of the experiment is a model which is changing during the period of the experiment.
"""^^xsd:string ;
              rdfs:label "DynamicModel"^^xsd:string .


###  http://www.hozo.jp/owl/EXPOApr19.xml/DynamismOfModel
:DynamismOfModel rdf:type owl:Class ;
                 rdfs:subClassOf :AttributeOfModel ;
                 rdfs:comment """
Dynamism of a model is an attribute of a model which characterizes whether the model involves time. For instance: a <static model>, a <dynamic model>.
"""^^xsd:string ;
                 rdfs:label "DynamismOfModel"^^xsd:string .


###  http://www.hozo.jp/owl/EXPOApr19.xml/Entity
:Entity rdf:type owl:Class ;
        rdfs:comment """
\"The universal class of individuals. This is the root node of the ontology.\" (SUMO)
"""^^xsd:string ;
        rdfs:label "Entity"^^xsd:string .


###  http://www.hozo.jp/owl/EXPOApr19.xml/EnvironmentalRequirements
:EnvironmentalRequirements rdf:type owl:Class ;
                           rdfs:subClassOf :ExperimentalRequirements ;
                           owl:disjointWith :FinancialRequirements ;
                           rdfs:comment """
Environmental requirements are external conditions or surroundings, esp. those in which people work or live, or a plant or animal lives; for instance food safety, hygiene. Reference: Collins Softback English Dictionary, HarperCollins Publishers, Glasgow, 1993.
"""^^xsd:string ;
                           rdfs:label "EnvironmentalRequirements"^^xsd:string .


###  http://www.hozo.jp/owl/EXPOApr19.xml/EperimentalDesignTask
:EperimentalDesignTask rdf:type owl:Class ;
                       rdfs:subClassOf :ScientificTask ;
                       owl:disjointWith :HypothesisFormation ,
                                        :InformationGethering ,
                                        :PoblemAnalysis ,
                                        :ResultsEvaluation ,
                                        :ResultsInterpretation ;
                       rdfs:comment """
An experimental design task is a scientific task of planning and organizing an experiment in order to achieve an experimental goal.
"""^^xsd:string ;
                       rdfs:label "EperimentalDesignTask"^^xsd:string .


###  http://www.hozo.jp/owl/EXPOApr19.xml/Error
:Error rdf:type owl:Class ;
       rdfs:subClassOf :ProductRole ,
                       [ rdf:type owl:Restriction ;
                         owl:onProperty :has_statistics_characteristic ;
                         owl:allValuesFrom :Dispersion
                       ] ,
                       [ rdf:type owl:Restriction ;
                         owl:onProperty :has_statistics_characteristic ;
                         owl:allValuesFrom :LevelOfSignificance
                       ] ,
                       [ rdf:type owl:Restriction ;
                         owl:onProperty :has_statistics_characteristic ;
                         owl:cardinality "1"^^xsd:nonNegativeInteger
                       ] ;
       rdfs:comment """
An error is the difference between observations or computations from the true values, or to values that are accepted as being true. Reference: USGS glossary: biology.usgs.gov/npsveg/glossary.html
"""^^xsd:string ;
       rdfs:label "Error"^^xsd:string .


###  http://www.hozo.jp/owl/EXPOApr19.xml/ErrorOfConclusion
:ErrorOfConclusion rdf:type owl:Class ;
                   rdfs:subClassOf :ResultError ;
                   rdfs:comment """
An error of a conclusion is an incorrectly inferred conclusion about the phenomena involved in the experiment.
"""^^xsd:string ;
                   rdfs:label "ErrorOfConclusion"^^xsd:string .


###  http://www.hozo.jp/owl/EXPOApr19.xml/ExecutionOfExperiment
:ExecutionOfExperiment rdf:type owl:Class ;
                       rdfs:subClassOf :ScientificActivity ;
                       owl:disjointWith :FormingClassificationSystem ,
                                        :HypothesisForming ,
                                        :InterpretingResult ,
                                        :ProcessProblemAnalysis ,
                                        :ResultEvaluating ;
                       rdfs:comment """
The execution of an experiment is the process of putting into effect a plan of experimental actions in order to archive an experimental goal. Reference: Based on The Oxford English Dictionary. Oxford University Press, 2 Ed., 1989
"""^^xsd:string ;
                       rdfs:label "ExecutionOfExperiment"^^xsd:string .


###  http://www.hozo.jp/owl/EXPOApr19.xml/ExperimentalAction
:ExperimentalAction rdf:type owl:Class ;
                    rdfs:subClassOf :ExecutionOfExperiment ,
                                    [ rdf:type owl:Restriction ;
                                      owl:onProperty :has__name ;
                                      owl:allValuesFrom :ActionName
                                    ] ,
                                    [ rdf:type owl:Restriction ;
                                      owl:onProperty :has_action_complexity ;
                                      owl:allValuesFrom :ActionComplexity
                                    ] ,
                                    [ rdf:type owl:Restriction ;
                                      owl:onProperty :has_goal ;
                                      owl:allValuesFrom :ActionGoal
                                    ] ,
                                    [ rdf:type owl:Restriction ;
                                      owl:onProperty :has_instrument ;
                                      owl:allValuesFrom :ExperimentalEquipment
                                    ] ,
                                    [ rdf:type owl:Restriction ;
                                      owl:onProperty :has_method ;
                                      owl:allValuesFrom :ExperimentalMethod
                                    ] ,
                                    [ rdf:type owl:Restriction ;
                                      owl:onProperty :has_timing ;
                                      owl:allValuesFrom :TimePoint
                                    ] ,
                                    [ rdf:type owl:Restriction ;
                                      owl:onProperty :has_action_complexity ;
                                      owl:cardinality "1"^^xsd:nonNegativeInteger
                                    ] ;
                    rdfs:comment """
An experimental action is a process of manipulation in the domain of the experiment in order to achive a particular sub goal, which is a part of the goal of the experiment.
"""^^xsd:string ;
                    rdfs:label "ExperimentalAction"^^xsd:string .


###  http://www.hozo.jp/owl/EXPOApr19.xml/ExperimentalActionsPlanning
:ExperimentalActionsPlanning rdf:type owl:Class ;
                             rdfs:subClassOf :EperimentalDesignTask ;
                             owl:disjointWith :ExperimentalEquipmentSelecting ,
                                              :ExperimentalModelDesign ,
                                              :ExperimentalObjectSelecting ;
                             rdfs:comment """
Experimental actions' planning is an experimental design task of constructing a sequence of experimental actions in order to achieve an experimental goal.
"""^^xsd:string ;
                             rdfs:label "ExperimentalActionsPlanning"^^xsd:string .


###  http://www.hozo.jp/owl/EXPOApr19.xml/ExperimentalConclusion
:ExperimentalConclusion rdf:type owl:Class ;
                        rdfs:subClassOf :ExperimentalResults ;
                        rdfs:comment """
An experimental conclusion is a conclusion inferred from experimental observations and other experimental data.
"""^^xsd:string ;
                        rdfs:label "ExperimentalConclusion"^^xsd:string .


###  http://www.hozo.jp/owl/EXPOApr19.xml/ExperimentalDesign
:ExperimentalDesign rdf:type owl:Class ;
                    rdfs:subClassOf :ExperimentalMethod ;
                    rdfs:comment """
An experimental design is a structured, organized method for determining the relationship between factors affecting  cause-effect relations between known and unknown variables. Reference: Sigma:http://www.isixsigma.com/dictionary/Design_of_Experiments_-_DOE-41.htm
"""^^xsd:string ;
                    rdfs:label "ExperimentalDesign"^^xsd:string .


###  http://www.hozo.jp/owl/EXPOApr19.xml/ExperimentalDesignEffect
:ExperimentalDesignEffect rdf:type owl:Class ;
                          rdfs:subClassOf :AlternativeHypothesis ;
                          owl:disjointWith :ObjectEffect ,
                                           :SubjectEffect ,
                                           :TimeEffect ;
                          rdfs:comment """
An experimental design effect is an alternative hypothesis where an effect on the experimental results is due to an inadequate experimental design.
"""^^xsd:string ;
                          rdfs:label "ExperimentalDesignEffect"^^xsd:string .


###  http://www.hozo.jp/owl/EXPOApr19.xml/ExperimentalDesignStrategy
:ExperimentalDesignStrategy rdf:type owl:Class ;
                            rdfs:subClassOf :Proposition ;
                            owl:disjointWith :ExperimentalHypothesis ,
                                             :ExperimentalStandard ,
                                             :ExperimentalTechnology ,
                                             :Fact ,
                                             :FieldOfStudy ,
                                             :Model ,
                                             :ModelAssumption ,
                                             :Procedure ,
                                             :Requirements ,
                                             :ScientificTask ,
                                             :SubjectQualification ,
                                             :ValueOfVariable ,
                                             :Variable ;
                            rdfs:comment """
An experimental design strategy is a collection of typical techniques applied to an experimental design, such as e.g. <comparison a control and a target groups>.
"""^^xsd:string ;
                            rdfs:label "ExperimentalDesignStrategy"^^xsd:string .


###  http://www.hozo.jp/owl/EXPOApr19.xml/ExperimentalEquipment
:ExperimentalEquipment rdf:type owl:Class ;
                       rdfs:subClassOf :Process-relatedRole ,
                                       [ rdf:type owl:Restriction ;
                                         owl:onProperty :has_description ;
                                         owl:allValuesFrom :TechnicalDescription
                                       ] ,
                                       [ rdf:type owl:Restriction ;
                                         owl:onProperty :has_name ;
                                         owl:allValuesFrom :NameEquipment
                                       ] ;
                       rdfs:comment """
Experimental equipment is the set of tools, devices, materials, computer systems assembled for performing the experiment. Reference: following Collins Softback English Dictionary, HarperCollins Publishers, Glasgow, 1993.
"""^^xsd:string ;
                       rdfs:label "ExperimentalEquipment"^^xsd:string .


###  http://www.hozo.jp/owl/EXPOApr19.xml/ExperimentalEquipmentSelecting
:ExperimentalEquipmentSelecting rdf:type owl:Class ;
                                rdfs:subClassOf :EperimentalDesignTask ;
                                owl:disjointWith :ExperimentalModelDesign ,
                                                 :ExperimentalObjectSelecting ;
                                rdfs:comment """
Experimental equipment selecting is an experimental design task of selecting appropriate instruments and materials for experimental actions.
"""^^xsd:string ;
                                rdfs:label "ExperimentalEquipmentSelecting"^^xsd:string .


###  http://www.hozo.jp/owl/EXPOApr19.xml/ExperimentalFactor
:ExperimentalFactor rdf:type owl:Class ;
                    rdfs:subClassOf :Variable ;
                    rdfs:comment """
An experimental factor is a known variable of the model of the domain which the object of the experiment can control/vary in order to determine of a value of target variables.
"""^^xsd:string ;
                    rdfs:label "ExperimentalFactor"^^xsd:string .


###  http://www.hozo.jp/owl/EXPOApr19.xml/ExperimentalGoal
:ExperimentalGoal rdf:type owl:Class ;
                  rdfs:subClassOf :RepresentationForm ,
                                  [ rdf:type owl:Restriction ;
                                    owl:onProperty :has_representation ;
                                    owl:allValuesFrom :RepresentationExperimentalGoal
                                  ] ,
                                  [ rdf:type owl:Restriction ;
                                    owl:onProperty :has_subgoal ;
                                    owl:allValuesFrom :ExperimentalSubgoal
                                  ] ;
                  rdfs:comment """
An experimental goal is the state that a plan is intended to achieve and that (when achieved) terminates behaviour intended to achieve it. Reference: WordNet: http://www.cogsci.princeton.edu/cgi-bin/webwn2.0?stage=1&word=goal+
"""^^xsd:string ;
                  rdfs:label "ExperimentalGoal"^^xsd:string .


###  http://www.hozo.jp/owl/EXPOApr19.xml/ExperimentalHypothesis
:ExperimentalHypothesis rdf:type owl:Class ;
                        rdfs:subClassOf :Proposition ,
                                        [ rdf:type owl:Restriction ;
                                          owl:onProperty :has_complexity ;
                                          owl:allValuesFrom :HypothesisComplexity
                                        ] ,
                                        [ rdf:type owl:Restriction ;
                                          owl:onProperty :has_explicitness ;
                                          owl:allValuesFrom :HypothesisExplicitness
                                        ] ,
                                        [ rdf:type owl:Restriction ;
                                          owl:onProperty :has_generality ;
                                          owl:allValuesFrom :GeneralityOfHypothesis
                                        ] ,
                                        [ rdf:type owl:Restriction ;
                                          owl:onProperty :has_hypothesis_representation ;
                                          owl:allValuesFrom :HypothesisRepresentation
                                        ] ,
                                        [ rdf:type owl:Restriction ;
                                          owl:onProperty :has_target_variable ;
                                          owl:allValuesFrom :TargetVariable
                                        ] ,
                                        [ rdf:type owl:Restriction ;
                                          owl:onProperty :has_complexity ;
                                          owl:cardinality "1"^^xsd:nonNegativeInteger
                                        ] ,
                                        [ rdf:type owl:Restriction ;
                                          owl:onProperty :has_explicitness ;
                                          owl:cardinality "1"^^xsd:nonNegativeInteger
                                        ] ,
                                        [ rdf:type owl:Restriction ;
                                          owl:onProperty :has_generality ;
                                          owl:cardinality "1"^^xsd:nonNegativeInteger
                                        ] ;
                        owl:disjointWith :ExperimentalStandard ,
                                         :ExperimentalTechnology ,
                                         :Fact ,
                                         :FieldOfStudy ,
                                         :Model ,
                                         :ModelAssumption ,
                                         :Procedure ,
                                         :Requirements ,
                                         :ScientificTask ,
                                         :SubjectQualification ,
                                         :ValueOfVariable ,
                                         :Variable ;
                        rdfs:comment """
An experimental hypothesis is a statement about cause-effect relations between known and unknown (target) variables of the domain of the experiment \"that shall be in accordance with known facts*\" to be verified at the experiment. Reference: The Oxford English Dictionary. Oxford University Press, 2 Ed., 1989
"""^^xsd:string ;
                        rdfs:label "ExperimentalHypothesis"^^xsd:string .


###  http://www.hozo.jp/owl/EXPOApr19.xml/ExperimentalMethod
:ExperimentalMethod rdf:type owl:Class ;
                    rdfs:subClassOf :ResearchMethod ,
                                    [ rdf:type owl:Restriction ;
                                      owl:onProperty :has_applicability ;
                                      owl:allValuesFrom :MethodApplicabilityCondition
                                    ] ,
                                    [ rdf:type owl:Restriction ;
                                      owl:onProperty :has_goal ;
                                      owl:allValuesFrom :MethodGoal
                                    ] ,
                                    [ rdf:type owl:Restriction ;
                                      owl:onProperty :has_plan ;
                                      owl:allValuesFrom :PlanOfExperimentalActions
                                    ] ,
                                    [ rdf:type owl:Restriction ;
                                      owl:onProperty :has_subject ;
                                      owl:allValuesFrom :SubjectMethod
                                    ] ;
                    rdfs:comment """
An experimental method is a way to solve a scientific task by executing a scientific experiment.
"""^^xsd:string ;
                    rdfs:label "ExperimentalMethod"^^xsd:string .


###  http://www.hozo.jp/owl/EXPOApr19.xml/ExperimentalModel
:ExperimentalModel rdf:type owl:Class ;
                   rdfs:subClassOf :Model ,
                                   [ rdf:type owl:Restriction ;
                                     owl:onProperty :has_experimental_factor ;
                                     owl:allValuesFrom :ExperimentalFactor
                                   ] ,
                                   [ rdf:type owl:Restriction ;
                                     owl:onProperty :has_unknown_variable ;
                                     owl:allValuesFrom :TargetVariable
                                   ] ;
                   rdfs:comment """
An experimental model is a description of dependencies (e.g. logical/mathematical) between experimental factors, others known variables, and unknown variables.  The experimental model is obtained from the domain model by fixing experimental factors from the list of known controllable variables and the target variables from the list of unknown variables.
"""^^xsd:string ;
                   rdfs:label "ExperimentalModel"^^xsd:string .


###  http://www.hozo.jp/owl/EXPOApr19.xml/ExperimentalModelDesign
:ExperimentalModelDesign rdf:type owl:Class ;
                         rdfs:subClassOf :EperimentalDesignTask ;
                         owl:disjointWith :ExperimentalObjectSelecting ;
                         rdfs:comment """
Experimental model design is an experimental design task of construction a model of the experiment from the model of the experimental domain by fixating experimental factors and target variables.
"""^^xsd:string ;
                         rdfs:label "ExperimentalModelDesign"^^xsd:string .


###  http://www.hozo.jp/owl/EXPOApr19.xml/ExperimentalObjectSelecting
:ExperimentalObjectSelecting rdf:type owl:Class ;
                             rdfs:subClassOf :EperimentalDesignTask ;
                             rdfs:comment """
Experimental object selecting is an experimental design task of selecting an appropriate to the experimental goal and experimental requirements an object of the experiment.
"""^^xsd:string ;
                             rdfs:label "ExperimentalObjectSelecting"^^xsd:string .


###  http://www.hozo.jp/owl/EXPOApr19.xml/ExperimentalObservation
:ExperimentalObservation rdf:type owl:Class ;
                         rdfs:subClassOf :ProductRole ,
                                         [ rdf:type owl:Restriction ;
                                           owl:onProperty :has__interpretation ;
                                           owl:allValuesFrom :ResultsInterpretation
                                         ] ,
                                         [ rdf:type owl:Restriction ;
                                           owl:onProperty :has_error ;
                                           owl:allValuesFrom :ObservationalError
                                         ] ,
                                         [ rdf:type owl:Restriction ;
                                           owl:onProperty :has_observation_characteristic ;
                                           owl:allValuesFrom :StatisticsCharacteristic
                                         ] ;
                         rdfs:comment """
An experimental observation is a direct observation of nature, the set of values of target variables (or other variables of the experiment model), \"prior to analysis; interpretation*\" (compare with experimental results). Reference: Based on The Oxford English Dictionary. Oxford University Press, 2 Ed., 1989 * Collins Softback English Dictionary, HarperCollins Publishers, Glasgow, 1993.
"""^^xsd:string ;
                         rdfs:label "ExperimentalObservation"^^xsd:string .


###  http://www.hozo.jp/owl/EXPOApr19.xml/ExperimentalProtocol
:ExperimentalProtocol rdf:type owl:Class ;
                      rdfs:subClassOf :ProcedureExecuteExperiment ;
                      rdfs:comment """
An experimental protocol is an explicit detailed specification of (usually a part of) an experiment which describes a plan of experimental actions to achieve an experimental subgoal (goal).
"""^^xsd:string ;
                      rdfs:label "ExperimentalProtocol"^^xsd:string .


###  http://www.hozo.jp/owl/EXPOApr19.xml/ExperimentalRequirements
:ExperimentalRequirements rdf:type owl:Class ;
                          rdfs:subClassOf :Requirements ;
                          owl:disjointWith :MethodApplicabilityCondition ;
                          rdfs:comment """
Experimental requirements are conditions (legal, ethic, economic, etc.) for preparation and execution of an experiment which must be complied with. Reference: Based on The Oxford English Dictionary. Oxford University Press, 2 Ed., 1989
"""^^xsd:string ;
                          rdfs:label "ExperimentalRequirements"^^xsd:string .


###  http://www.hozo.jp/owl/EXPOApr19.xml/ExperimentalResults
:ExperimentalResults rdf:type owl:Class ;
                     rdfs:subClassOf :ProductRole ,
                                     [ rdf:type owl:Restriction ;
                                       owl:onProperty :has_error ;
                                       owl:allValuesFrom :ResultError
                                     ] ,
                                     [ rdf:type owl:Restriction ;
                                       owl:onProperty :has_evaluation ;
                                       owl:allValuesFrom :ResultsEvaluation
                                     ] ,
                                     [ rdf:type owl:Restriction ;
                                       owl:onProperty :has_fact ;
                                       owl:allValuesFrom :FactRejectResearchHypothesis
                                     ] ,
                                     [ rdf:type owl:Restriction ;
                                       owl:onProperty :has_fact ;
                                       owl:allValuesFrom :FactSupportResearchHypothesis
                                     ] ;
                     rdfs:comment """
Experimental results are the set of facts and conclusions, obtained as a result of the interpretation of the experimental observations, which increase/decrease the probability of a research hypothesis of the experiment.
"""^^xsd:string ;
                     rdfs:label "ExperimentalResults"^^xsd:string .


###  http://www.hozo.jp/owl/EXPOApr19.xml/ExperimentalRule
:ExperimentalRule rdf:type owl:Class ;
                  rdfs:subClassOf :Procedure ;
                  rdfs:comment """
An experimental rule is \"a customary form of procedure; regular course of actions; the common order of things.\"
Reference: Collins Softback English Dictionary, HarperCollins Publishers, Glasgow, 1993.
"""^^xsd:string ;
                  rdfs:label "ExperimentalRule"^^xsd:string .


###  http://www.hozo.jp/owl/EXPOApr19.xml/ExperimentalStandard
:ExperimentalStandard rdf:type owl:Class ;
                      rdfs:subClassOf :Proposition ;
                      owl:disjointWith :ExperimentalTechnology ,
                                       :Fact ,
                                       :FieldOfStudy ,
                                       :Model ,
                                       :ModelAssumption ,
                                       :Procedure ,
                                       :Requirements ,
                                       :ScientificTask ,
                                       :SubjectQualification ,
                                       :ValueOfVariable ,
                                       :Variable ;
                      rdfs:comment """
An experimental standard is \"an accepted or approved\" procedure in the domain of an experiment, for example a standard for data representation, or a standard for measurements.  Reference: Collins Softback English Dictionary, HarperCollins Publishers, Glasgow, 1993.
"""^^xsd:string ;
                      rdfs:label "ExperimentalStandard"^^xsd:string .


###  http://www.hozo.jp/owl/EXPOApr19.xml/ExperimentalSubgoal
:ExperimentalSubgoal rdf:type owl:Class ;
                     rdfs:subClassOf :Goal ;
                     rdfs:comment """
An experimental subgoal is a step to an experimental goal. Decomposition of an experimental goal onto subgoals corresponds to partition of the experiments onto stages, sub-stages, etc.
"""^^xsd:string ;
                     rdfs:label "ExperimentalSubgoal"^^xsd:string .


###  http://www.hozo.jp/owl/EXPOApr19.xml/ExperimentalTechnology
:ExperimentalTechnology rdf:type owl:Class ;
                        rdfs:subClassOf :Proposition ,
                                        [ rdf:type owl:Restriction ;
                                          owl:onProperty :has_experimental_requirements ;
                                          owl:allValuesFrom :ExperimentalRequirements
                                        ] ,
                                        [ rdf:type owl:Restriction ;
                                          owl:onProperty :has_standard ;
                                          owl:allValuesFrom :ExperimentalStandard
                                        ] ,
                                        [ rdf:type owl:Restriction ;
                                          owl:onProperty :has_strategy ;
                                          owl:allValuesFrom :ExperimentalDesignStrategy
                                        ] ;
                        owl:disjointWith :Fact ,
                                         :FieldOfStudy ,
                                         :Model ,
                                         :ModelAssumption ,
                                         :Procedure ,
                                         :Requirements ,
                                         :ScientificTask ,
                                         :SubjectQualification ,
                                         :ValueOfVariable ,
                                         :Variable ;
                        rdfs:comment """
An experimental technology is the total knowledge (theory, methods, and practices), and machinery available to any object of an experiment. Reference: Based on the Collins Softback English Dictionary, HarperCollins Publishers, Glasgow, 1993.
"""^^xsd:string ;
                        rdfs:label "ExperimentalTechnology"^^xsd:string .


###  http://www.hozo.jp/owl/EXPOApr19.xml/ExperimenteeBias
:ExperimenteeBias rdf:type owl:Class ;
                  rdfs:subClassOf :ObjectEffect ;
                  owl:disjointWith :HawthorneEffect ,
                                   :MortalityEffect ;
                  rdfs:comment """
An experimentee bias is an object effect where results of an experiment are due to systematic differences in research participants (\"experimetees\") assigned to different conditions or treatments. Reference: Davis, J., Psychological research methods.
"""^^xsd:string ;
                  rdfs:label "ExperimenteeBias"^^xsd:string .


###  http://www.hozo.jp/owl/EXPOApr19.xml/ExperimenterBias
:ExperimenterBias rdf:type owl:Class ;
                  rdfs:subClassOf :SubjectEffect ;
                  owl:disjointWith :TestingEffect ;
                  rdfs:comment """
An experimenter bias is a subject effect, where results of an experiment are due to the experimenter's actions or expectations. A number of studies have shown that researchers tend to find the results they are looking for, a kind of self-fulfilling prophecy. Reference: Davis, J., Psychological research methods.
"""^^xsd:string ;
                  rdfs:label "ExperimenterBias"^^xsd:string .


###  http://www.hozo.jp/owl/EXPOApr19.xml/ExplainGoal
:ExplainGoal rdf:type owl:Class ;
             rdfs:subClassOf :ExperimentalGoal ;
             owl:disjointWith :InvestigateGoal ;
             rdfs:comment """
An explain-goal is an experimental goal of a hypothesis-forming experiment.
"""^^xsd:string ;
             rdfs:label "ExplainGoal"^^xsd:string .


###  http://www.hozo.jp/owl/EXPOApr19.xml/ExplicitHypothesis
:ExplicitHypothesis rdf:type owl:Class ;
                    rdfs:subClassOf :HypothesisExplicitness ;
                    owl:disjointWith :ImplicitHypothesis ;
                    rdfs:comment """
An explicit hypothesis of an experimental hypothesis is a Boolean attribute which is true when the statement is written in the form of a text, for instance in terms of predicate logic.
"""^^xsd:string ;
                    rdfs:label "ExplicitHypothesis"^^xsd:string .


###  http://www.hozo.jp/owl/EXPOApr19.xml/Fact
:Fact rdf:type owl:Class ;
      rdfs:subClassOf :Proposition ;
      owl:disjointWith :FieldOfStudy ,
                       :Model ,
                       :ModelAssumption ,
                       :Procedure ,
                       :Requirements ,
                       :ScientificTask ,
                       :SubjectQualification ,
                       :ValueOfVariable ,
                       :Variable ;
      rdfs:comment """
The concept is outside EXPO;
A fact is a particular truth known by actual observation or authentic testimony, as opposed to what is merely inferred, or to a conjecture or fiction; a datum of experience, as distinguished from the conclusions that may be based upon it. Reference: The Oxford English Dictionary. Oxford University Press, 2 Ed., 1989
"""^^xsd:string ;
      rdfs:label "Fact"^^xsd:string .


###  http://www.hozo.jp/owl/EXPOApr19.xml/FactRejectResearchHypothesis
:FactRejectResearchHypothesis rdf:type owl:Class ;
                              rdfs:subClassOf :Fact ;
                              owl:disjointWith :FactSupportResearchHypothesis ;
                              rdfs:comment """
A fact which rejects a research hypothesis is a fact which decreases the probability of the hypothesis.
"""^^xsd:string ;
                              rdfs:label "FactRejectResearchHypothesis"^^xsd:string .


###  http://www.hozo.jp/owl/EXPOApr19.xml/FactSupportResearchHypothesis
:FactSupportResearchHypothesis rdf:type owl:Class ;
                               rdfs:subClassOf :Fact ;
                               rdfs:comment """
A fact which rejects a research hypothesis is a fact which increases the probability of the hypothesis.
"""^^xsd:string ;
                               rdfs:label "FactSupportResearchHypothesis"^^xsd:string .


###  http://www.hozo.jp/owl/EXPOApr19.xml/FactorLevel
:FactorLevel rdf:type owl:Class ;
             rdfs:subClassOf :ValueOfVariable ;
             rdfs:comment """
A factor level is a value of the variable <Experimental factor>. \"The word <level> is used for the various strengths, quantities, or concentration of each factor\".
Reference:  Langley, R. Practical Statistics. David&Charles Ltd, Newton,1971.
"""^^xsd:string ;
             rdfs:label "FactorLevel"^^xsd:string .


###  http://www.hozo.jp/owl/EXPOApr19.xml/FactorialDesign
:FactorialDesign rdf:type owl:Class ;
                 rdfs:subClassOf :ExperimentalDesign ;
                 rdfs:comment """
A factorial design is an experimental design where all the sample sizes of experimental objects are determined in advance, Two or more experimental factors of the experimental model, which the object of the experiment can control, are varied in order to determine of a value of target variables. Reference:  Based on: Langley, R. Practical Statistics. David&Charles Ltd, Newton,1971.
"""^^xsd:string ;
                 rdfs:label "FactorialDesign"^^xsd:string .


###  http://www.hozo.jp/owl/EXPOApr19.xml/FalseNegative
:FalseNegative rdf:type owl:Class ;
               rdfs:subClassOf :HypothesisAcceptanceMistake ;
               rdfs:comment """
A false negative is an hypothesis acceptance mistake where the hypothesis being tested is actually true and we conclude that it is false. Reference:  based on Introduction to Probability and Statistics. 4th ed. H.L. Alder, E.B. Roessler, W.H. Freeman & Co., 1968.
"""^^xsd:string ;
               rdfs:label "FalseNegative"^^xsd:string .


###  http://www.hozo.jp/owl/EXPOApr19.xml/FalsePpositive
:FalsePpositive rdf:type owl:Class ;
                rdfs:subClassOf :HypothesisAcceptanceMistake ;
                rdfs:comment """
A false positive is an hypothesis acceptance mistake where the hypothesis being tested is actually false and we conclude that it is. Reference:  based on Introduction to Probability and Statistics. 4th ed. H.L. Alder, E.B. Roessler, W.H. Freeman & Co., 1968.
"""^^xsd:string ;
                rdfs:label "FalsePpositive"^^xsd:string .


###  http://www.hozo.jp/owl/EXPOApr19.xml/FaultyComparison
:FaultyComparison rdf:type owl:Class ;
                  rdfs:subClassOf :ResultError ;
                  rdfs:comment """
A faulty comparison is a result error due to using invalid comparison procedures or applying valid comparison procedures to incomparable objects.
"""^^xsd:string ;
                  rdfs:label "FaultyComparison"^^xsd:string .


###  http://www.hozo.jp/owl/EXPOApr19.xml/FieldOfStudy
:FieldOfStudy rdf:type owl:Class ;
              rdfs:subClassOf :Proposition ;
              owl:disjointWith :Model ,
                               :ModelAssumption ,
                               :Procedure ,
                               :Requirements ,
                               :ScientificTask ,
                               :SubjectQualification ,
                               :ValueOfVariable ,
                               :Variable ;
              rdfs:comment """
SUMO \"An academic or applied discipline with recognized experts and with a core of accepted theory or practice. Note that FieldOfStudy is a subclass of Proposition, because a FieldOfStudy is understood to be a body of abstract, informational content, with varying degrees of certainty attached to each element of this content.\" http://www.ontologyportal.org/
"""^^xsd:string ;
              rdfs:label "FieldOfStudy"^^xsd:string .


###  http://www.hozo.jp/owl/EXPOApr19.xml/FinancialRequirements
:FinancialRequirements rdf:type owl:Class ;
                       rdfs:subClassOf :ExperimentalRequirements ;
                       rdfs:comment """
Financial requirements are financial capacity and restrictions of a subject of the experiment.
"""^^xsd:string ;
                       rdfs:label "FinancialRequirements"^^xsd:string .


###  http://www.hozo.jp/owl/EXPOApr19.xml/FormingClassificationSystem
:FormingClassificationSystem rdf:type owl:Class ;
                             rdfs:subClassOf :ScientificActivity ;
                             owl:disjointWith :HypothesisForming ,
                                              :InterpretingResult ,
                                              :ProcessProblemAnalysis ,
                                              :ResultEvaluating ;
                             rdfs:comment """
Forming a classification system is the scientific activity to form a hierarchical system of categories.
"""^^xsd:string ;
                             rdfs:label "FormingClassificationSystem"^^xsd:string .


###  http://www.hozo.jp/owl/EXPOApr19.xml/Formula
:Formula rdf:type owl:Class ;
         rdfs:subClassOf :Sentence ;
         rdfs:comment """
\"A syntactically well-formed formula in the SUO-KIF knowledge representation language.\" (SUMO) or other formal language.
"""^^xsd:string ;
         rdfs:label "Formula"^^xsd:string .


###  http://www.hozo.jp/owl/EXPOApr19.xml/GalileanExperiment
:GalileanExperiment rdf:type owl:Class ;
                    rdfs:subClassOf :PhysicalExperiment ;
                    rdfs:comment """
A Galilean experiment is a scientific experiment which involves explicit hypotheses. Reference: Medawar, P.B. Advice to a Young Scientist. Pan Books Ltd, London, 1981
"""^^xsd:string ;
                    rdfs:label "GalileanExperiment"^^xsd:string .


###  http://www.hozo.jp/owl/EXPOApr19.xml/GeneKnock-in
:GeneKnock-in rdf:type owl:Class ;
              rdfs:subClassOf :ComparisonControl_TargetGroups ;
              owl:disjointWith :GeneKnock-out ,
                               :Normal_Disease ,
                               :TimeCourse ,
                               :Treated_Untreated ;
              rdfs:comment """
A gene knock-in design strategy is a sub-class of a comparison control/ target groups strategy where a target group has one or more genes added.
"""^^xsd:string ;
              rdfs:label "GeneKnock-in"^^xsd:string .


###  http://www.hozo.jp/owl/EXPOApr19.xml/GeneKnock-out
:GeneKnock-out rdf:type owl:Class ;
               rdfs:subClassOf :ComparisonControl_TargetGroups ;
               owl:disjointWith :Normal_Disease ,
                                :TimeCourse ,
                                :Treated_Untreated ;
               rdfs:comment """
A gene knock-out design strategy is a sub-class of a comparison control/ target groups strategy where a target group has one or more genes removed.
"""^^xsd:string ;
               rdfs:label "GeneKnock-out"^^xsd:string .


###  http://www.hozo.jp/owl/EXPOApr19.xml/GeneralityOfHypothesis
:GeneralityOfHypothesis rdf:type owl:Class ;
                        rdfs:subClassOf :AttributeOfHypothesis ;
                        owl:disjointWith :HypothesisComplexity ,
                                         :HypothesisExplicitness ;
                        rdfs:comment """
The generality of an hypothesis is an attribute of an experimental hypothesis which characterizes whether the hypothesis is inductive (more general) or abductive (less general).
"""^^xsd:string ;
                        rdfs:label "GeneralityOfHypothesis"^^xsd:string .


###  http://www.hozo.jp/owl/EXPOApr19.xml/Goal
:Goal rdf:type owl:Class ;
      rdfs:subClassOf :TaskRole ;
      rdfs:comment """
the concept is outside of EXPO
"""^^xsd:string ;
      rdfs:label "Goal"^^xsd:string .


###  http://www.hozo.jp/owl/EXPOApr19.xml/Group
:Group rdf:type owl:Class ;
       rdfs:subClassOf :Collection ;
       rdfs:comment """
\"A Collection of Agents, e.g. a flock of sheep, a herd of goats, or the local Boy Scout troop.\" (SUMO)
"""^^xsd:string ;
       rdfs:label "Group"^^xsd:string .


###  http://www.hozo.jp/owl/EXPOApr19.xml/GroupExperimentalObject
:GroupExperimentalObject rdf:type owl:Class ;
                         rdfs:subClassOf :ObjectOfExperiment ;
                         rdfs:comment """
A group of experimental objects is a collection of studying in a scientific investigation objects.
"""^^xsd:string ;
                         rdfs:label "GroupExperimentalObject"^^xsd:string .


###  http://www.hozo.jp/owl/EXPOApr19.xml/HandTool
:HandTool rdf:type owl:Class ;
          rdfs:subClassOf :Tool ;
          rdfs:comment """
A hand tool is a small manual instrument traditionally operated by the muscular strength of the user. Reference: Encyclopaedia Britannica online: http://www.britannica.com/
"""^^xsd:string ;
          rdfs:label "HandTool"^^xsd:string .


###  http://www.hozo.jp/owl/EXPOApr19.xml/Hardware
:Hardware rdf:type owl:Class ;
          rdfs:subClassOf :Device ;
          rdfs:comment """
the concept is outside of EXPO
"""^^xsd:string ;
          rdfs:label "Hardware"^^xsd:string .


###  http://www.hozo.jp/owl/EXPOApr19.xml/HawthorneEffect
:HawthorneEffect rdf:type owl:Class ;
                 rdfs:subClassOf :ObjectEffect ;
                 owl:disjointWith :MortalityEffect ;
                 rdfs:comment """
A Hawthorne effect is a object effect where results are due to subjects' expectations of desired behaviour in the research setting or the social psychology of the experiment. Reference: Davis, J., Psychological research methods.
"""^^xsd:string ;
                 rdfs:label "HawthorneEffect"^^xsd:string .


###  http://www.hozo.jp/owl/EXPOApr19.xml/HistoryEffect
:HistoryEffect rdf:type owl:Class ;
               rdfs:subClassOf :TimeEffect ;
               owl:disjointWith :MaturationEffect ;
               rdfs:comment """
A history effect is a time effect where an effect on the experimental results is due to events outside the experiment. Some events that are not part of the research, i.e. a natural disaster, which occurs at the same time as executing the experiment could affect the results. Reference: Davis, J., Psychological research methods.
"""^^xsd:string ;
               rdfs:label "HistoryEffect"^^xsd:string .


###  http://www.hozo.jp/owl/EXPOApr19.xml/Human
:Human rdf:type owl:Class ;
       rdfs:subClassOf :SentientAgent ,
                       [ rdf:type owl:Restriction ;
                         owl:onProperty :has_organization ;
                         owl:allValuesFrom :Organization
                       ] ,
                       [ rdf:type owl:Restriction ;
                         owl:onProperty :has_telephone_number ;
                         owl:allValuesFrom :Number
                       ] ,
                       [ rdf:type owl:Restriction ;
                         owl:onProperty :has_title ;
                         owl:allValuesFrom :Title
                       ] ,
                       [ rdf:type owl:Restriction ;
                         owl:onProperty :has_name ;
                         owl:cardinality "1"^^xsd:nonNegativeInteger
                       ] ;
       owl:disjointWith :Robot ;
       rdfs:comment """
SUMO: Modern man, the only remaining species of the Homo genus.\"http://www.ontologyportal.org/
"""^^xsd:string ;
       rdfs:label "Human"^^xsd:string .


###  http://www.hozo.jp/owl/EXPOApr19.xml/HumanLanguage
:HumanLanguage rdf:type owl:Class ;
               rdfs:subClassOf :Language ;
               rdfs:comment """
\"The subclass of Languages used by Humans.\" (SUMO)
"""^^xsd:string ;
               rdfs:label "HumanLanguage"^^xsd:string .


###  http://www.hozo.jp/owl/EXPOApr19.xml/Hypothesis-drivenExperiment
:Hypothesis-drivenExperiment rdf:type owl:Class ;
                             rdfs:subClassOf :GalileanExperiment ;
                             rdfs:comment """
A hypothesis-driven experiment is a Galilean experiment designed to confirm or reject a given hypothesis.  The deductive consequences of the hypothesis are compared with the experimental result, and the probability of the hypothesis increased (confirmed) or decreased (rejected).
"""^^xsd:string ;
                             rdfs:label "Hypothesis-drivenExperiment"^^xsd:string .


###  http://www.hozo.jp/owl/EXPOApr19.xml/Hypothesis-formingExperiment
:Hypothesis-formingExperiment rdf:type owl:Class ;
                              rdfs:subClassOf :GalileanExperiment ;
                              rdfs:comment """
A hypothesis-forming experiment is a Galilean experiment.  It includes a hypotheses formation stage in which one or more hypotheses are formed using abduction or induction.
"""^^xsd:string ;
                              rdfs:label "Hypothesis-formingExperiment"^^xsd:string .


###  http://www.hozo.jp/owl/EXPOApr19.xml/HypothesisAcceptanceMistake
:HypothesisAcceptanceMistake rdf:type owl:Class ;
                             rdfs:subClassOf :ResultError ;
                             rdfs:comment """
An hypothesis acceptance mistake is the incorrect acceptance or rejecting of the research hypothesis (H1).
"""^^xsd:string ;
                             rdfs:label "HypothesisAcceptanceMistake"^^xsd:string .


###  http://www.hozo.jp/owl/EXPOApr19.xml/HypothesisComplexity
:HypothesisComplexity rdf:type owl:Class ;
                      rdfs:subClassOf :AttributeOfHypothesis ;
                      owl:disjointWith :HypothesisExplicitness ;
                      rdfs:comment """
Hypothesis complexity is an attribute of an hypothesis which characterizes information content.
"""^^xsd:string ;
                      rdfs:label "HypothesisComplexity"^^xsd:string .


###  http://www.hozo.jp/owl/EXPOApr19.xml/HypothesisExplicitness
:HypothesisExplicitness rdf:type owl:Class ;
                        rdfs:subClassOf :AttributeOfHypothesis ;
                        rdfs:comment """
Hypothesis explicitness is an attribute of an hypothesis which characterizes the explicitness of the statement; whether the statement is represented in a form of a text or not. For example: an <explicit hypothesis>, an <implicit hypothesis>.
"""^^xsd:string ;
                        rdfs:label "HypothesisExplicitness"^^xsd:string .


###  http://www.hozo.jp/owl/EXPOApr19.xml/HypothesisFormation
:HypothesisFormation rdf:type owl:Class ;
                     rdfs:subClassOf :ScientificTask ;
                     owl:disjointWith :InformationGethering ,
                                      :PoblemAnalysis ,
                                      :ResultsEvaluation ,
                                      :ResultsInterpretation ;
                     rdfs:comment """
Hypothesis formation is the scientific task to frame a hypothesis or supposition*? on the basis of preliminary information gathering and problem analysis. Reference: The Oxford English Dictionary. Oxford University Press, 2 Ed., 1989
"""^^xsd:string ;
                     rdfs:label "HypothesisFormation"^^xsd:string .


###  http://www.hozo.jp/owl/EXPOApr19.xml/HypothesisForming
:HypothesisForming rdf:type owl:Class ;
                   rdfs:subClassOf :ScientificActivity ;
                   owl:disjointWith :InterpretingResult ,
                                    :ProcessProblemAnalysis ,
                                    :ResultEvaluating ;
                   rdfs:comment """
Hypothesis forming is the act \"to frame a hypothesis or supposition\"* on the basis of preliminary information gathering and problem analysis. Reference: The Oxford English Dictionary. Oxford University Press, 2 Ed., 1989
"""^^xsd:string ;
                   rdfs:label "HypothesisForming"^^xsd:string .


###  http://www.hozo.jp/owl/EXPOApr19.xml/HypothesisRepresentation
:HypothesisRepresentation rdf:type owl:Class ;
                          rdfs:subClassOf :Representation ;
                          owl:disjointWith :ModelRepresentation ,
                                           :RepresentationExperimentalExecutionProcedure ,
                                           :RepresentationExperimentalGoal ,
                                           :RepresentationExperimentalObservation ,
                                           :RepresentationExperimentalResults ,
                                           :TechnicalDescription ;
                          rdfs:comment """
An hypothesis representation is a reproduction of the hypothesis in some material or tangible form? Reference: The Oxford English Dictionary. Oxford University Press, 2 Ed., 1989
"""^^xsd:string ;
                          rdfs:label "HypothesisRepresentation"^^xsd:string .


###  http://www.hozo.jp/owl/EXPOApr19.xml/IDExperiment
:IDExperiment rdf:type owl:Class ;
              rdfs:subClassOf :Name ;
              owl:disjointWith :LoginName ,
                               :NameEquipment ,
                               :Password ,
                               :PersonalName ,
                               :Title ;
              rdfs:label "IDExperiment"^^xsd:string .


###  http://www.hozo.jp/owl/EXPOApr19.xml/Image
:Image rdf:type owl:Class ;
       rdfs:subClassOf :RepresentationForm ;
       rdfs:comment """
Dublin Core: http://www.lub.lu.se/cgi-bin/nmdc.pl
"""^^xsd:string ;
       rdfs:label "Image"^^xsd:string .


###  http://www.hozo.jp/owl/EXPOApr19.xml/ImplicitHypothesis
:ImplicitHypothesis rdf:type owl:Class ;
                    rdfs:subClassOf :HypothesisExplicitness ;
                    rdfs:comment """
An implicit hypothesis of an experimental hypothesis is a Boolean attribute which is false where the statement can be written in the form of a text.
"""^^xsd:string ;
                    rdfs:label "ImplicitHypothesis"^^xsd:string .


###  http://www.hozo.jp/owl/EXPOApr19.xml/ImproperSampling
:ImproperSampling rdf:type owl:Class ;
                  rdfs:subClassOf :ObservationalError ;
                  rdfs:comment """
Improper sampling is an observational error due to mistakes in a forming a sample: applying sampling methods.
"""^^xsd:string ;
                  rdfs:label "ImproperSampling"^^xsd:string .


###  http://www.hozo.jp/owl/EXPOApr19.xml/IncompleteDataError
:IncompleteDataError rdf:type owl:Class ;
                     rdfs:subClassOf :ResultError ;
                     rdfs:comment """
An incomplete data error is a result error due to the data being incapable of providing evidence for a research hypothesis.
"""^^xsd:string ;
                     rdfs:label "IncompleteDataError"^^xsd:string .


###  http://www.hozo.jp/owl/EXPOApr19.xml/Independence
:Independence rdf:type owl:Class ;
              rdfs:subClassOf :AttributeOfVariable ;
              rdfs:label "Independence"^^xsd:string .


###  http://www.hozo.jp/owl/EXPOApr19.xml/IndependentVariable
:IndependentVariable rdf:type owl:Class ;
                     rdfs:subClassOf :Independence ;
                     rdfs:comment """
The concept is outside of EXPO
"""^^xsd:string ;
                     rdfs:label "IndependentVariable"^^xsd:string .


###  http://www.hozo.jp/owl/EXPOApr19.xml/InductiveHypothesis
:InductiveHypothesis rdf:type owl:Class ;
                     rdfs:subClassOf :GeneralityOfHypothesis ;
                     rdfs:comment """
An inductive hypothesis is formalized as the generalization of examples by a predicate clause. Reference: Based on Abe A.: The Relation between Abductive Hypotheses and Inductive Hypotheses, Proc. of IJCAI97 Workshop on Abduction and Induction, pp. 1--6 (1997)
"""^^xsd:string ;
                     rdfs:label "InductiveHypothesis"^^xsd:string .


###  http://www.hozo.jp/owl/EXPOApr19.xml/InferableVariable
:InferableVariable rdf:type owl:Class ;
                   rdfs:subClassOf :Variable ;
                   rdfs:comment """
An inferable variable is an instance-of a variable where it is possible to make a computational inference about its value. Reference:  based on Albar`ede, P. A theory of experiment. http://66.102.9.104/search?q=cache:ECOW7jEPfHAJ: arxiv.org/pdf/cs.AI/0201022++a+theory+of+experiment+Albarede&hl=en
"""^^xsd:string ;
                   rdfs:label "InferableVariable"^^xsd:string .


###  http://www.hozo.jp/owl/EXPOApr19.xml/InformationGethering
:InformationGethering rdf:type owl:Class ;
                      rdfs:subClassOf :ScientificTask ;
                      owl:disjointWith :PoblemAnalysis ,
                                       :ResultsEvaluation ,
                                       :ResultsInterpretation ;
                      rdfs:comment """
Information gathering is the scientific task of collecting information for further analysis or for other scientific purposes.
"""^^xsd:string ;
                      rdfs:label "InformationGethering"^^xsd:string .


###  http://www.hozo.jp/owl/EXPOApr19.xml/InstrumentationEffect
:InstrumentationEffect rdf:type owl:Class ;
                       rdfs:subClassOf :ExperimentalDesignEffect ;
                       rdfs:comment """
An instrumentation effect is an experimental design effect where an effect on the experimental results is due to an aberration in the measuring tools, either mechanical instrument or test. Reference: Davis, J., Psychological research methods.
"""^^xsd:string ;
                       rdfs:label "InstrumentationEffect"^^xsd:string .


###  http://www.hozo.jp/owl/EXPOApr19.xml/InternalStatus
:InternalStatus rdf:type owl:Class ;
                rdfs:subClassOf :RestrictedStatus ;
                rdfs:comment """
An internal status is a status which controls the access to a SOP, a protocol, and/ or experimental results to within an organization.
"""^^xsd:string ;
                rdfs:label "InternalStatus"^^xsd:string .


###  http://www.hozo.jp/owl/EXPOApr19.xml/InterpretingResult
:InterpretingResult rdf:type owl:Class ;
                    rdfs:subClassOf :ScientificActivity ;
                    owl:disjointWith :ProcessProblemAnalysis ,
                                     :ResultEvaluating ;
                    rdfs:comment """
Interpreting a result is the act of interpreting or explaining, the meaning of an experimental result. Reference: Based on The Oxford English Dictionary. Oxford University Press, 2 Ed., 1989
"""^^xsd:string ;
                    rdfs:label "InterpretingResult"^^xsd:string .


###  http://www.hozo.jp/owl/EXPOApr19.xml/InvestigateGoal
:InvestigateGoal rdf:type owl:Class ;
                 rdfs:subClassOf :ExperimentalGoal ;
                 rdfs:comment """
An investigate-goal is an experimental goal of a Baconian experiment.
"""^^xsd:string ;
                 rdfs:label "InvestigateGoal"^^xsd:string .


###  http://www.hozo.jp/owl/EXPOApr19.xml/Journal
:Journal rdf:type owl:Class ;
         rdfs:subClassOf :Text ;
         rdfs:comment """
Dublin Core: http://www.lub.lu.se/cgi-bin/nmdc.pl
"""^^xsd:string ;
         rdfs:label "Journal"^^xsd:string .


###  http://www.hozo.jp/owl/EXPOApr19.xml/Language
:Language rdf:type owl:Class ;
          rdfs:subClassOf :LinguisticExpression ;
          owl:disjointWith :Sentence ;
          rdfs:comment """
SUMO: http://www.ontologyportal.org/ \"A system of signs for expressing thought. The system can be either natural or artificial, i.e. something that emerges gradually as a cultural artifact or something that is intentionally created by a person or group of people.\"
"""^^xsd:string ;
          rdfs:label "Language"^^xsd:string .


###  http://www.hozo.jp/owl/EXPOApr19.xml/LevelOfSignificance
:LevelOfSignificance rdf:type owl:Class ;
                     rdfs:subClassOf :StatisticsCharacteristic ;
                     owl:disjointWith :Robustness ,
                                      :Validity ;
                     rdfs:comment """
The concept is outside of EXPO
"""^^xsd:string ;
                     rdfs:label "LevelOfSignificance"^^xsd:string .


###  http://www.hozo.jp/owl/EXPOApr19.xml/LibraryOfCongressClassification
:LibraryOfCongressClassification rdf:type owl:Class ;
                                 rdfs:subClassOf :ClassificationOfDomains ;
                                 owl:disjointWith :NLMClassification ,
                                                  :ResearchCouncilsUKClassification ;
                                 rdfs:comment """
Library of Congress classification is the system of library organization developed during the reorganization of the U.S. Library of Congress. It consists of separate, mutually exclusive, special classifications, often having no connection save the accidental one of alphabetical notation. Reference: Encyclopedia Britannica online: http://www.britannica.com/
"""^^xsd:string ;
                                 rdfs:label "LibraryOfCongressClassification"^^xsd:string .


###  http://www.hozo.jp/owl/EXPOApr19.xml/LinearModel
:LinearModel rdf:type owl:Class ;
             rdfs:subClassOf :DegreeOfModel ;
             owl:disjointWith :NonlinearModel ;
             rdfs:comment """
A linear model is a mathematical model where the relationship between the variables is linear.
"""^^xsd:string ;
             rdfs:label "LinearModel"^^xsd:string .


###  http://www.hozo.jp/owl/EXPOApr19.xml/LinguisticExpression
:LinguisticExpression rdf:type owl:Class ;
                      rdfs:subClassOf :ContentBearingPhysical ;
                      rdfs:comment """
\"This is the subclass of ContentBearingPhysical which are language-related. Note that this Class encompasses both Language and the the elements of Languages, e.g. Words.\" SUMO: http://www.ontologyportal.org/
"""^^xsd:string ;
                      rdfs:label "LinguisticExpression"^^xsd:string .


###  http://www.hozo.jp/owl/EXPOApr19.xml/LogicalModelRepresentation
:LogicalModelRepresentation rdf:type owl:Class ;
                            rdfs:subClassOf :ModelRepresentation ;
                            rdfs:comment """
A logical model is a representation of an experimental model where the relationship between the variables is logical.
"""^^xsd:string ;
                            rdfs:label "LogicalModelRepresentation"^^xsd:string .


###  http://www.hozo.jp/owl/EXPOApr19.xml/LoginName
:LoginName rdf:type owl:Class ;
           rdfs:subClassOf :Name ;
           owl:disjointWith :NameEquipment ,
                            :Password ,
                            :PersonalName ,
                            :Title ;
           rdfs:comment """
The concept is outside of EXPO
"""^^xsd:string ;
           rdfs:label "LoginName"^^xsd:string .


###  http://www.hozo.jp/owl/EXPOApr19.xml/Machine
:Machine rdf:type owl:Class ;
         rdfs:subClassOf :Device ;
         rdfs:comment """
Machines are Devices that have a well-defined resource and result and that automatically convert the resource into the result.\" Reference: SUMO: http://www.ontologyportal.org/
"""^^xsd:string ;
         rdfs:label "Machine"^^xsd:string .


###  http://www.hozo.jp/owl/EXPOApr19.xml/MachineTool
:MachineTool rdf:type owl:Class ;
             rdfs:subClassOf :Tool ;
             rdfs:comment """
A machine tool is a power-driven mechanism used to cut, shape, or form materials such as wood and metal. Reference: Encyclopaedia Britannica online: http://www.britannica.com/
"""^^xsd:string ;
             rdfs:label "MachineTool"^^xsd:string .


###  http://www.hozo.jp/owl/EXPOApr19.xml/Magazine
:Magazine rdf:type owl:Class ;
          rdfs:subClassOf :Text ;
          rdfs:comment """
Dublin Core: http://www.lub.lu.se/cgi-bin/nmdc.pl
"""^^xsd:string ;
          rdfs:label "Magazine"^^xsd:string .


###  http://www.hozo.jp/owl/EXPOApr19.xml/Materials
:Materials rdf:type owl:Class ;
           rdfs:subClassOf :ExperimentalEquipment ;
           rdfs:comment """
Materials are culture collections and chemicals used for executing of an experiment.
"""^^xsd:string ;
           rdfs:label "Materials"^^xsd:string .


###  http://www.hozo.jp/owl/EXPOApr19.xml/MathematicalModelRepresentation
:MathematicalModelRepresentation rdf:type owl:Class ;
                                 rdfs:subClassOf :ModelRepresentation ;
                                 rdfs:comment """
A mathematical model is a representation of an experimental model where the relationship between the variables is mathematical.
"""^^xsd:string ;
                                 rdfs:label "MathematicalModelRepresentation"^^xsd:string .


###  http://www.hozo.jp/owl/EXPOApr19.xml/MaturationEffect
:MaturationEffect rdf:type owl:Class ;
                  rdfs:subClassOf :TimeEffect ;
                  rdfs:comment """
A maturation effect is a time effect where an effect on the experimental results is due to changes within subjects over time, e.g., growth, warm-up, fatigue, learning to learn. Reference: Davis, J., Psychological research methods.
"""^^xsd:string ;
                  rdfs:label "MaturationEffect"^^xsd:string .


###  http://www.hozo.jp/owl/EXPOApr19.xml/MeasurementError
:MeasurementError rdf:type owl:Class ;
                  rdfs:subClassOf :ObservationalError ;
                  rdfs:comment """
A measurement error is an error involving the observation of a physical quantity. Reference: Arley, N. & Buch , K.R., Introduction to the theory of probability and statistics. New York : Wiley London. Chapman & Hall, 1950. 236p.
"""^^xsd:string ;
                  rdfs:label "MeasurementError"^^xsd:string .


###  http://www.hozo.jp/owl/EXPOApr19.xml/MetabolomicExperiment
:MetabolomicExperiment rdf:type owl:Class ;
                       rdfs:subClassOf :ClassificationByDomain ;
                       rdfs:comment """
The concept is outside of EXPO, it belongs to the metabolomic domain.
"""^^xsd:string ;
                       rdfs:label "MetabolomicExperiment"^^xsd:string .


###  http://www.hozo.jp/owl/EXPOApr19.xml/MethodApplicabilityCondition
:MethodApplicabilityCondition rdf:type owl:Class ;
                              rdfs:subClassOf :Requirements ;
                              rdfs:comment """
A method applicability condition is an applicability condition that specifies the contexts in which the experimental method may be applied to achieve the method goal.
"""^^xsd:string ;
                              rdfs:label "MethodApplicabilityCondition"^^xsd:string .


###  http://www.hozo.jp/owl/EXPOApr19.xml/MethodGoal
:MethodGoal rdf:type owl:Class ;
            rdfs:subClassOf :Goal ;
            rdfs:comment """
A method goal is the state that a plan of method actions 
is intended to achieve, and that (when achieved) terminates behavior intended to achieve it. 
Reference: Based on  WordNet: http://www.cogsci.princeton.edu/cgi-bin/webwn2.0?stage=1&word=goal+
"""^^xsd:string ;
            rdfs:label "MethodGoal"^^xsd:string .


###  http://www.hozo.jp/owl/EXPOApr19.xml/MethodsComparison
:MethodsComparison rdf:type owl:Class ;
                   rdfs:subClassOf :PairedComparisonOfSingleSampleGroups ;
                   owl:disjointWith :SubjectsComparison ;
                   rdfs:comment """
A methods comparison is a paired comparison of single sample groups experimental design strategy where the result of applying different methods to achieve the same goal are compared. Reference:  Based on: Langley, R. Practical Statistics. David&Charles Ltd, Newton,1971.
"""^^xsd:string ;
                   rdfs:label "MethodsComparison"^^xsd:string .


###  http://www.hozo.jp/owl/EXPOApr19.xml/MicroarrayExperiment
:MicroarrayExperiment rdf:type owl:Class ;
                      rdfs:subClassOf :ClassificationByDomain ;
                      rdfs:comment """
The concept is outside of EXPO.
"""^^xsd:string ;
                      rdfs:label "MicroarrayExperiment"^^xsd:string .


###  http://www.hozo.jp/owl/EXPOApr19.xml/Model
:Model rdf:type owl:Class ;
       rdfs:subClassOf :Proposition ,
                       [ rdf:type owl:Restriction ;
                         owl:onProperty :has_representation ;
                         owl:allValuesFrom :ModelRepresentation
                       ] ;
       owl:disjointWith :ModelAssumption ,
                        :Procedure ,
                        :Requirements ,
                        :ScientificTask ,
                        :SubjectQualification ,
                        :ValueOfVariable ,
                        :Variable ;
       rdfs:comment """
The concept is outside of EXPO
"""^^xsd:string ;
       rdfs:label "Model"^^xsd:string .


###  http://www.hozo.jp/owl/EXPOApr19.xml/ModelAssumption
:ModelAssumption rdf:type owl:Class ;
                 rdfs:subClassOf :Proposition ;
                 owl:disjointWith :Procedure ,
                                  :Requirements ,
                                  :ScientificTask ,
                                  :SubjectQualification ,
                                  :ValueOfVariable ,
                                  :Variable ;
                 rdfs:comment """
A model assumption is an assumption about the domain used as a premise, it is necessarily explicit - written in the form of a text.
"""^^xsd:string ;
                 rdfs:label "ModelAssumption"^^xsd:string .


###  http://www.hozo.jp/owl/EXPOApr19.xml/ModelRepresentation
:ModelRepresentation rdf:type owl:Class ;
                     rdfs:subClassOf :Representation ;
                     owl:disjointWith :RepresentationExperimentalExecutionProcedure ,
                                      :RepresentationExperimentalGoal ,
                                      :RepresentationExperimentalObservation ,
                                      :RepresentationExperimentalResults ,
                                      :TechnicalDescription ;
                     rdfs:comment """
A model representation is a formalized description of the experimental model, for instance a text or formulas.
"""^^xsd:string ;
                     rdfs:label "ModelRepresentation"^^xsd:string .


###  http://www.hozo.jp/owl/EXPOApr19.xml/MortalityEffect
:MortalityEffect rdf:type owl:Class ;
                 rdfs:subClassOf :ObjectEffect ;
                 rdfs:comment """
A mortality effect is an object effect which occurs when subjects leave an experiment before it is complete (e.g. die) and so bias the experimental results. This is especially true when more subjects leave one treatment condition more than another. This leads to a kind of subject effect because the subjects in the different groups are no longer equivalent. Reference: Davis, J., Psychological research methods.
"""^^xsd:string ;
                 rdfs:label "MortalityEffect"^^xsd:string .


###  http://www.hozo.jp/owl/EXPOApr19.xml/Multi-factorExperiment
:Multi-factorExperiment rdf:type owl:Class ;
                        rdfs:subClassOf :ClassificationByModel ;
                        owl:disjointWith :One-factorExperiment ,
                                         :Two-factorExperiment ;
                        rdfs:comment """
A multi-factor experiment is an experiment with a model containing 3, 4, or more fixed controllable variables.
"""^^xsd:string ;
                        rdfs:label "Multi-factorExperiment"^^xsd:string .


###  http://www.hozo.jp/owl/EXPOApr19.xml/NLMClassification
:NLMClassification rdf:type owl:Class ;
                   rdfs:subClassOf :ClassificationOfDomains ;
                   owl:disjointWith :ResearchCouncilsUKClassification ;
                   rdfs:comment """
The NML (National Library of Medicine) classification is a product of the National Library of Medicine for the arrangement of library materials in the field of medicine and related sciences used internationally? Reference: NLM: http://wwwcf.nlm.nih.gov/class/
"""^^xsd:string ;
                   rdfs:label "NLMClassification"^^xsd:string .


###  http://www.hozo.jp/owl/EXPOApr19.xml/Name
:Name rdf:type owl:Class ;
      rdfs:subClassOf :Attribute ;
      owl:disjointWith :StatisticsCharacteristic ;
      rdfs:comment """
A name a word or phrase constituting the individual designation by which a particular person or thing is known, referred to, or addressed. Reference: The Oxford English Dictionary. Oxford University Press, 2 Ed., 1989
"""^^xsd:string ;
      rdfs:label "Name"^^xsd:string .


###  http://www.hozo.jp/owl/EXPOApr19.xml/NameEquipment
:NameEquipment rdf:type owl:Class ;
               rdfs:subClassOf :Name ;
               owl:disjointWith :Password ,
                                :PersonalName ,
                                :Title ;
               rdfs:comment """
An equipment name is a name that refers to a piece of experimental equipment.
"""^^xsd:string ;
               rdfs:label "NameEquipment"^^xsd:string .


###  http://www.hozo.jp/owl/EXPOApr19.xml/NaturalLanguage
:NaturalLanguage rdf:type owl:Class ;
                 rdfs:subClassOf :HumanLanguage ;
                 rdfs:comment """
\"The subclass of HumanLanguages which are not designed and which evolve from generation to generation. This Class includes all of the national languages, e.g. English, Spanish, Japanese, etc. Note that this class includes dialects of natural languages.\" SUMO: http://www.ontologyportal.org/
"""^^xsd:string ;
                 rdfs:label "NaturalLanguage"^^xsd:string .


###  http://www.hozo.jp/owl/EXPOApr19.xml/NonRestrictedStatus
:NonRestrictedStatus rdf:type owl:Class ;
                     rdfs:subClassOf :PermissionStatus ;
                     owl:disjointWith :RestrictedStatus ;
                     rdfs:comment """
A non restricted status is a status which allows the access to a SOP, a protocol, and/ or experimental results for legal purposes.
"""^^xsd:string ;
                     rdfs:label "NonRestrictedStatus"^^xsd:string .


###  http://www.hozo.jp/owl/EXPOApr19.xml/NonlinearModel
:NonlinearModel rdf:type owl:Class ;
                rdfs:subClassOf :DegreeOfModel ;
                rdfs:comment """
A nonlinear model is a mathematical model where the relationship between the variables is nonlinear.
"""^^xsd:string ;
                rdfs:label "NonlinearModel"^^xsd:string .


###  http://www.hozo.jp/owl/EXPOApr19.xml/Normal_Disease
:Normal_Disease rdf:type owl:Class ;
                rdfs:subClassOf :ComparisonControl_TargetGroups ;
                owl:disjointWith :TimeCourse ,
                                 :Treated_Untreated ;
                rdfs:comment """
A normal/ disease design strategy is a sub-class of a comparison control/ target groups strategy, where the target group is group of experimental objects with a disease.
"""^^xsd:string ;
                rdfs:label "Normal/Disease"^^xsd:string .


###  http://www.hozo.jp/owl/EXPOApr19.xml/NormalizationStrategy
:NormalizationStrategy rdf:type owl:Class ;
                       rdfs:subClassOf :ExperimentalDesignStrategy ;
                       owl:disjointWith :PairedComparison ,
                                        :QualityControl ;
                       rdfs:comment """
A normalization strategy is an experimental design strategy to reduce experimental result variation.
"""^^xsd:string ;
                       rdfs:label "NormalizationStrategy"^^xsd:string .


###  http://www.hozo.jp/owl/EXPOApr19.xml/NullHypothesis
:NullHypothesis rdf:type owl:Class ;
                rdfs:subClassOf :ExperimentalHypothesis ;
                owl:disjointWith :ResearchHypothesis ;
                rdfs:comment """
A null hypothesis is an experimental hypothesis that states that a known controlled variable or variables does not have a specified effect on the unknown (target) variable or variables of the domain.
"""^^xsd:string ;
                rdfs:label "NullHypothesis"^^xsd:string .


###  http://www.hozo.jp/owl/EXPOApr19.xml/Number
:Number rdf:type owl:Class ;
        rdfs:subClassOf :Quantity ;
        owl:disjointWith :PhysicalQuantity ;
        rdfs:comment """
\"A measure of how many things there are, or how much there is, of a certain kind. Numbers are subclassed into RealNumber, ComplexNumber, and ImaginaryNumber.\" (SUMO)
"""^^xsd:string ;
        rdfs:label "Number"^^xsd:string .


###  http://www.hozo.jp/owl/EXPOApr19.xml/Object
:Object rdf:type owl:Class ;
        rdfs:subClassOf :Physical ;
        owl:disjointWith :Process ;
        rdfs:comment """
SUMO: Corresponds roughly to the class of ordinary objects. Examples include normal physical objects, geographical regions, and locations of Processes, the complement of Objects in the Physical class. In a 4D ontology, an Object is something whose spatiotemporal extent is thought of as dividing into spatial parts roughly parallel to the time-axis.\"http://www.ontologyportal.org/
"""^^xsd:string ;
        rdfs:label "Object"^^xsd:string .


###  http://www.hozo.jp/owl/EXPOApr19.xml/ObjectEffect
:ObjectEffect rdf:type owl:Class ;
              rdfs:subClassOf :AlternativeHypothesis ;
              owl:disjointWith :SubjectEffect ,
                               :TimeEffect ;
              rdfs:comment """
An object effect is an alternative hypothesis where an effect on the experimental results is due to uncontrolled object's action or expectations.
"""^^xsd:string ;
              rdfs:label "ObjectEffect"^^xsd:string .


###  http://www.hozo.jp/owl/EXPOApr19.xml/ObjectMethod
:ObjectMethod rdf:type owl:Class ;
              rdfs:subClassOf :ObjectOfExperiment ;
              rdfs:comment """
An object of a method is \"on whom?\"the method is applied. For instance: a <plant>, a <robot>.
Reference: based on The Oxford English Dictionary http://dictionary.oed.com
"""^^xsd:string ;
              rdfs:label "ObjectMethod"^^xsd:string .


###  http://www.hozo.jp/owl/EXPOApr19.xml/ObjectOfAction
:ObjectOfAction rdf:type owl:Class ;
                rdfs:subClassOf :ObjectOfExperiment ;
                rdfs:comment """
An object of an action is \"on whom an action is made\". For instance: a <plant>, a <robot>. The Oxford English Dictionary. Oxford University Press, 2 Ed., 1990
"""^^xsd:string ;
                rdfs:label "ObjectOfAction"^^xsd:string .


###  http://www.hozo.jp/owl/EXPOApr19.xml/ObjectOfExperiment
:ObjectOfExperiment rdf:type owl:Class ;
                    rdfs:subClassOf :ActorRole ,
                                    [ rdf:type owl:Restriction ;
                                      owl:onProperty :has_admin_info ;
                                      owl:cardinality "1"^^xsd:nonNegativeInteger
                                    ] ;
                    rdfs:comment """
An object of an experiment is \"on whom an experiment is made.\" For instance: a <plant>, a <robot>. The Oxford English Dictionary. Oxford University Press, 2 Ed., 1989
"""^^xsd:string ;
                    rdfs:label "ObjectOfExperiment"^^xsd:string .


###  http://www.hozo.jp/owl/EXPOApr19.xml/ObservableVariable
:ObservableVariable rdf:type owl:Class ;
                    rdfs:subClassOf :Variable ;
                    rdfs:comment """
An observable variable is a variable where it is possible to directly observe (measure) the variable. Reference:  based on Albar`ede, P. A theory of experiment. http://66.102.9.104/search?q=cache:ECOW7jEPfHAJ: arxiv.org/pdf/cs.AI/0201022++a+theory+of+experiment+Albarede&hl=en
"""^^xsd:string ;
                    rdfs:label "ObservableVariable"^^xsd:string .


###  http://www.hozo.jp/owl/EXPOApr19.xml/ObservationalError
:ObservationalError rdf:type owl:Class ;
                    rdfs:subClassOf :Error ;
                    rdfs:comment """
An observational error is the difference between observations and their true values, or to values that are accepted as being true. Reference: USGS glossary: biology.usgs.gov/npsveg/glossary.html
"""^^xsd:string ;
                    rdfs:label "ObservationalError"^^xsd:string .


###  http://www.hozo.jp/owl/EXPOApr19.xml/One-factorExperiment
:One-factorExperiment rdf:type owl:Class ;
                      rdfs:subClassOf :ClassificationByModel ;
                      owl:disjointWith :Two-factorExperiment ;
                      rdfs:comment """
One-factor experiment is an experiment with a model containing one fixed controllable variable.
"""^^xsd:string ;
                      rdfs:label "One-factorExperiment"^^xsd:string .


###  http://www.hozo.jp/owl/EXPOApr19.xml/Organization
:Organization rdf:type owl:Class ;
              rdfs:subClassOf :Group ,
                              [ rdf:type owl:Restriction ;
                                owl:onProperty :has_fax_number ;
                                owl:allValuesFrom :Number
                              ] ,
                              [ rdf:type owl:Restriction ;
                                owl:onProperty :has_name ;
                                owl:allValuesFrom :Name
                              ] ,
                              [ rdf:type owl:Restriction ;
                                owl:onProperty :has_telephone_number ;
                                owl:allValuesFrom :Number
                              ] ,
                              [ rdf:type owl:Restriction ;
                                owl:onProperty :has_name ;
                                owl:cardinality "1"^^xsd:nonNegativeInteger
                              ] ;
              rdfs:comment """
SUMO: An Organization is a corporate or similar institution. The members of an Organization typically have a common purpose or function. Note that this class also covers divisions, departments, etc. of organizations. For example, both the Shell Corporation and the accounting department at Shell would both be instances of Organization. Note too that the existence of an Organization is dependent on the existence of at least one member (since Organization is a subclass of Collection). Accordingly, in cases of purely legal organizations, a fictitious member should be assumed.\"http://www.ontologyportal.org/
"""^^xsd:string ;
              rdfs:label "Organization"^^xsd:string .


###  http://www.hozo.jp/owl/EXPOApr19.xml/PairedComparison
:PairedComparison rdf:type owl:Class ;
                  rdfs:subClassOf :ExperimentalDesignStrategy ;
                  owl:disjointWith :QualityControl ;
                  rdfs:comment """
A paired comparison is an experimental design strategy where two groups of experimental objects are used to compare affects of the experimental factor(s). Reference:  Based on: Langley, R. Practical Statistics. David&Charles Ltd, Newton,1971.
"""^^xsd:string ;
                  rdfs:label "PairedComparison"^^xsd:string .


###  http://www.hozo.jp/owl/EXPOApr19.xml/PairedComparisonOfMatchingGroups
:PairedComparisonOfMatchingGroups rdf:type owl:Class ;
                                  rdfs:subClassOf :PairedComparison ;
                                  owl:disjointWith :PairedComparisonOfSingleSampleGroups ;
                                  rdfs:comment """
A paired comparison of matching groups is a paired comparison experimental design strategy where each member of one group of experimental objects matches (by a definite rule) a member (a pair) of another group of experimental objects. Reference:  Based on: Langley, R. Practical Statistics. David&Charles Ltd, Newton,1971.
"""^^xsd:string ;
                                  rdfs:label "PairedComparisonOfMatchingGroups"^^xsd:string .


###  http://www.hozo.jp/owl/EXPOApr19.xml/PairedComparisonOfSingleSampleGroups
:PairedComparisonOfSingleSampleGroups rdf:type owl:Class ;
                                      rdfs:subClassOf :PairedComparison ;
                                      rdfs:comment """
A paired comparison of single sample groups is a paired comparison experimental design strategy where the same group of experimental objects is examined twice or more in order to compare the effects of experimental factors. Reference:  Based on: Langley, R. Practical Statistics. David&Charles Ltd, Newton,1971.
"""^^xsd:string ;
                                      rdfs:label "PairedComparisonOfSingleSampleGroups"^^xsd:string .


###  http://www.hozo.jp/owl/EXPOApr19.xml/Paper
:Paper rdf:type owl:Class ;
       rdfs:subClassOf :Artifact ;
       rdfs:comment """
\"An Artifact made of cellulose pulp that is intended to contain a Text.\" (SUMO)
It can play a role: RepresenationalMedium
"""^^xsd:string ;
       rdfs:label "Paper"^^xsd:string .


###  http://www.hozo.jp/owl/EXPOApr19.xml/ParentGroup
:ParentGroup rdf:type owl:Class ;
             rdfs:subClassOf :GroupExperimentalObject ;
             rdfs:comment """
A parent group is a group of studying in a scientific investigation objects, which is used to form a sample as an object of the experiment.
"""^^xsd:string ;
             rdfs:label "ParentGroup"^^xsd:string .


###  http://www.hozo.jp/owl/EXPOApr19.xml/ParticlePhysicsExperiment
:ParticlePhysicsExperiment rdf:type owl:Class ;
                           rdfs:subClassOf :ClassificationByDomain ;
                           rdfs:comment """
A particle physics experiment is a scientific experiment producing knowledge about the particle physics field of study.
"""^^xsd:string ;
                           rdfs:label "ParticlePhysicsExperiment"^^xsd:string .


###  http://www.hozo.jp/owl/EXPOApr19.xml/Password
:Password rdf:type owl:Class ;
          rdfs:subClassOf :Name ;
          owl:disjointWith :PersonalName ,
                           :Title ;
          rdfs:comment """
The concept is outside of EXPO
"""^^xsd:string ;
          rdfs:label "Password"^^xsd:string .


###  http://www.hozo.jp/owl/EXPOApr19.xml/PermissionStatus
:PermissionStatus rdf:type owl:Class ;
                  rdfs:subClassOf :StatusExperimentalDocument ;
                  rdfs:comment """
A permission status is a status of an experimental document that specifies current a condition or privilege allowing use of the experimental document, e.g. <public status>.
"""^^xsd:string ;
                  rdfs:label "PermissionStatus"^^xsd:string .


###  http://www.hozo.jp/owl/EXPOApr19.xml/PersonalName
:PersonalName rdf:type owl:Class ;
              rdfs:subClassOf :Name ;
              owl:disjointWith :Title ;
              rdfs:comment """
The concept is outside of EXPO
"""^^xsd:string ;
              rdfs:label "PersonalName"^^xsd:string .


###  http://www.hozo.jp/owl/EXPOApr19.xml/Physical
:Physical rdf:type owl:Class ;
          rdfs:subClassOf :Entity ;
          rdfs:comment """
SUMO: http://www.ontologyportal.org/
"""^^xsd:string ;
          rdfs:label "Physical"^^xsd:string .


###  http://www.hozo.jp/owl/EXPOApr19.xml/PhysicalExperiment
:PhysicalExperiment rdf:type owl:Class ;
                    rdfs:subClassOf :ScientificExperiment ;
                    rdfs:comment """
A physical experiment is a scientific experiment which investigates cause-effect relations between known and unknown variables by manipulating the real-world (physical) domain.
"""^^xsd:string ;
                    rdfs:label "PhysicalExperiment"^^xsd:string .


###  http://www.hozo.jp/owl/EXPOApr19.xml/PhysicalQuantity
:PhysicalQuantity rdf:type owl:Class ;
                  rdfs:subClassOf :Quantity ;
                  rdfs:comment """
\"A PhysicalQuantity is a measure of some quantifiable aspect of the modeled world, such as 'the earth's diameter' (a constant length) and 'the stress in a loaded deformable solid' (a measure of stress, which is a function of three spatial coordinates). All PhysicalQuantities are either ConstantQuantities or FunctionQuantities. Instances of ConstantQuantity are dependent on a UnitOfMeasure, while instances of FunctionQuantity are Functions that map instances of ConstantQuantity to other instances of ConstantQuantity (e.g., TimeDependentQuantities are FunctionQuantities). Although the name and definition of PhysicalQuantity is borrowed from physics, PhysicalQuantities need not be material. Aside from the dimensions of length, time, velocity, etc., nonphysical dimensions such as currency are also possible. Accordingly, amounts of money would be instances of PhysicalQuantity. PhysicalQuantities are distinguished from Numbers by the fact that the former are associated with a dimension of measurement.\" SUMO: http://www.ontologyportal.org/
"""^^xsd:string ;
                  rdfs:label "PhysicalQuantity"^^xsd:string .


###  http://www.hozo.jp/owl/EXPOApr19.xml/Plan
:Plan rdf:type owl:Class ;
      rdfs:subClassOf :Procedure ;
      rdfs:comment """
The concept is outside of EXPO;
SUMO: \"A specification of a sequence of Processes which is intended to satisfy a specified purpose at some future time.\" http://www.ontologyportal.org/
"""^^xsd:string ;
      rdfs:label "Plan"^^xsd:string .


###  http://www.hozo.jp/owl/EXPOApr19.xml/PlanOfExperimentalActions
:PlanOfExperimentalActions rdf:type owl:Class ;
                           rdfs:subClassOf :Plan ;
                           rdfs:comment """
A plan of experimental actions is an explicitly described sequence of experimental actions according to which the experiment is to be done. See also <protocol>, <SOP>. Reference: based on The Oxford English Dictionary. Oxford University Press, 2 Ed., 1989
"""^^xsd:string ;
                           rdfs:label "PlanOfExperimentalActions"^^xsd:string .


###  http://www.hozo.jp/owl/EXPOApr19.xml/PoblemAnalysis
:PoblemAnalysis rdf:type owl:Class ;
                rdfs:subClassOf :ScientificTask ;
                owl:disjointWith :ResultsEvaluation ,
                                 :ResultsInterpretation ;
                rdfs:comment """
Problem analysis is the scientific task of reducing a problem's complexity. Reference: based on The Oxford English Dictionary. Oxford University Press, 2 Ed., 1989
"""^^xsd:string ;
                rdfs:label "PoblemAnalysis"^^xsd:string .


###  http://www.hozo.jp/owl/EXPOApr19.xml/Predicate
:Predicate rdf:type owl:Class ;
           rdfs:subClassOf :Relation ;
           rdfs:comment """
\"A Predicate is a sentence-forming Relation. Each tuple in the Relation is a finite, ordered sequence of objects. The fact that a particular tuple is an element of a Predicate is denoted by '(*predicate* arg_1 arg_2 .. arg_n)', where the arg_i are the objects so related. In the case of BinaryPredicates, the fact can be read as `arg_1 is *predicate* arg_2' or `a *predicate* of arg_1 is arg_2'.\" (SUMO)
"""^^xsd:string ;
           rdfs:label "Predicate"^^xsd:string .


###  http://www.hozo.jp/owl/EXPOApr19.xml/PresentingSampling
:PresentingSampling rdf:type owl:Class ;
                    rdfs:subClassOf :SamplingMethod ;
                    rdfs:comment """
Presenting sampling is a sampling method where members of a sample are individuals available \"at present\". It is \"a common kind sampling in medical research, for instance, a doctor can report on the last 50 cases of appendicitis that he has seen.\" Reference: Based on Langley, R. Practical Statistics. David&Charles Ltd, Newton,1971.
"""^^xsd:string ;
                    rdfs:label "PresentingSampling"^^xsd:string .


###  http://www.hozo.jp/owl/EXPOApr19.xml/Procedure
:Procedure rdf:type owl:Class ;
           rdfs:subClassOf :Proposition ;
           owl:disjointWith :Requirements ,
                            :ScientificTask ,
                            :SubjectQualification ,
                            :ValueOfVariable ,
                            :Variable ;
           rdfs:comment """
A sequence-dependent specification. Some examples are ComputerPrograms, finite-state machines, cooking recipes, musical scores, conference schedules, driving directions, and the scripts of plays and movies. Reference: SUMO http://berkelium.teknowledge.com:8080/sigma/home.jsp
"""^^xsd:string ;
           rdfs:label "Procedure"^^xsd:string .


###  http://www.hozo.jp/owl/EXPOApr19.xml/ProcedureExecuteExperiment
:ProcedureExecuteExperiment rdf:type owl:Class ;
                            rdfs:subClassOf :Procedure ,
                                            [ rdf:type owl:Restriction ;
                                              owl:onProperty :has_plan ;
                                              owl:allValuesFrom :PlanOfExperimentalActions
                                            ] ,
                                            [ rdf:type owl:Restriction ;
                                              owl:onProperty :has_representation ;
                                              owl:allValuesFrom :RepresentationExperimentalExecutionProcedure
                                            ] ,
                                            [ rdf:type owl:Restriction ;
                                              owl:onProperty :has_status ;
                                              owl:allValuesFrom :DocumentStage
                                            ] ,
                                            [ rdf:type owl:Restriction ;
                                              owl:onProperty :has_status ;
                                              owl:allValuesFrom :PermissionStatus
                                            ] ,
                                            [ rdf:type owl:Restriction ;
                                              owl:onProperty :has_status ;
                                              owl:cardinality "1"^^xsd:nonNegativeInteger
                                            ] ;
                            rdfs:comment """
A procedure to execute an experiment is an explicit detailed specification of an experiment, which describes experimental methods, experimental equipment, a plan of experimental actions, a status of the procedure, etc.
"""^^xsd:string ;
                            rdfs:label "ProcedureExecuteExperiment"^^xsd:string .


###  http://www.hozo.jp/owl/EXPOApr19.xml/Proceedings
:Proceedings rdf:type owl:Class ;
             rdfs:subClassOf :Text ;
             rdfs:comment """
Dublin Core: http://www.lub.lu.se/cgi-bin/nmdc.pl
"""^^xsd:string ;
             rdfs:label "Proceedings"^^xsd:string .


###  http://www.hozo.jp/owl/EXPOApr19.xml/Process
:Process rdf:type owl:Class ;
         rdfs:subClassOf :Physical ;
         rdfs:comment """
The concept is out EXPO.
\"Intuitively, the class of things that happen and have temporal parts or stages. Examples include extended events like a football match or a race, actions like Pursuing and Reading, and biological processes. The formal definition is: anything that lasts for a time but is not an Object. Note that a Process may have participants 'inside' it which are Objects, such as the players in a football match. In a 4D ontology, a Process is something whose spatiotemporal extent is thought of as dividing into temporal stages roughly perpendicular to the time-axis.\" Reference:SUMO http://berkelium.teknowledge.com:8080/sigma/home.jsp
"""^^xsd:string ;
         rdfs:label "Process"^^xsd:string .


###  http://www.hozo.jp/owl/EXPOApr19.xml/Process-relatedRole
:Process-relatedRole rdf:type owl:Class ;
                     rdfs:subClassOf :Role ;
                     rdfs:comment """
Product role (Final output)
Residue role (How it is processed)
"""^^xsd:string ;
                     rdfs:label "Process-relatedRole"^^xsd:string .


###  http://www.hozo.jp/owl/EXPOApr19.xml/ProcessProblemAnalysis
:ProcessProblemAnalysis rdf:type owl:Class ;
                        rdfs:subClassOf :ScientificActivity ;
                        owl:disjointWith :ResultEvaluating ;
                        rdfs:comment """
process of problem analysis  is an act of reducing a problem's complexity. Reference: based on The Oxford English Dictionary. Oxford University Press, 2 Ed., 1989
"""^^xsd:string ;
                        rdfs:label "ProcessProblemAnalysis"^^xsd:string .


###  http://www.hozo.jp/owl/EXPOApr19.xml/ProductRole
:ProductRole rdf:type owl:Class ;
             rdfs:subClassOf :Process-relatedRole ;
             rdfs:comment """
Final output
"""^^xsd:string ;
             rdfs:label "ProductRole"^^xsd:string .


###  http://www.hozo.jp/owl/EXPOApr19.xml/Program
:Program rdf:type owl:Class ;
         rdfs:subClassOf :Artifact ;
         rdfs:label "Program"^^xsd:string .


###  http://www.hozo.jp/owl/EXPOApr19.xml/Proposition
:Proposition rdf:type owl:Class ;
             rdfs:subClassOf :Abstract ;
             owl:disjointWith :Quantity ,
                              :Relation ;
             rdfs:comment """
Propositions are Abstract entities that express a complete thought or a set of such thoughts. As an example, the formula '     (instance Yojo Cat)' expresses the Proposition that the entity named Yojo is an element of the Class of Cats. Note that propositions are not restricted to the content expressed by individual sentences of a Language. They may encompass the content expressed by theories, books, and even whole libraries. It is important to distinguish Propositions from the ContentBearingObjects that express them. A Proposition is a piece of information, e.g. that the cat is on the mat, but a ContentBearingObject is an Object that represents this information. A Proposition is an abstraction that may have multiple representations: strings, sounds, icons, etc. For example, the Proposition that the cat is on the mat is represented here as a string of graphical characters displayed on a monitor and/or printed on paper, but it can be represented by a sequence of sounds or by some non-latin alphabet or by some cryptographic form. 
Reference: SUMO http://berkelium.teknowledge.com:8080/sigma/home.jsp
"""^^xsd:string ;
             rdfs:label "Proposition"^^xsd:string .


###  http://www.hozo.jp/owl/EXPOApr19.xml/ProteomicExperiment
:ProteomicExperiment rdf:type owl:Class ;
                     rdfs:subClassOf :ClassificationByDomain ;
                     rdfs:comment "The concept is outside of EXPO."^^xsd:string ;
                     rdfs:label "ProteomicExperiment"^^xsd:string .


###  http://www.hozo.jp/owl/EXPOApr19.xml/Provider
:Provider rdf:type owl:Class ;
          rdfs:subClassOf :SubjectRole ,
                          [ rdf:type owl:Restriction ;
                            owl:onProperty :has_admin_info ;
                            owl:allValuesFrom :AdminInfoProvider
                          ] ,
                          [ rdf:type owl:Restriction ;
                            owl:onProperty :has_admin_info ;
                            owl:cardinality "1"^^xsd:nonNegativeInteger
                          ] ;
          rdfs:comment """
A provider is a person or organization that provides or supplies experimental materials, equipment, objects of an experiment, etc. Reference: Based on The Oxford English Dictionary. Oxford University Press, 2 Ed., 1989
"""^^xsd:string ;
          rdfs:label "Provider"^^xsd:string .


###  http://www.hozo.jp/owl/EXPOApr19.xml/PublicAcademicStatus
:PublicAcademicStatus rdf:type owl:Class ;
                      rdfs:subClassOf :NonRestrictedStatus ;
                      rdfs:comment """
A public academic status restricts the use of a SOP, a protocol, and/or experimental results to academic purposes only.
"""^^xsd:string ;
                      rdfs:label "PublicAcademicStatus"^^xsd:string .


###  http://www.hozo.jp/owl/EXPOApr19.xml/PublicStatus
:PublicStatus rdf:type owl:Class ;
              rdfs:subClassOf :NonRestrictedStatus ;
              rdfs:comment """
A public status allows the use of a SOP, a protocol, and/ or experimental results for all legal purposes.
"""^^xsd:string ;
              rdfs:label "PublicStatus"^^xsd:string .


###  http://www.hozo.jp/owl/EXPOApr19.xml/QualityControl
:QualityControl rdf:type owl:Class ;
                rdfs:subClassOf :ExperimentalDesignStrategy ;
                rdfs:comment """
Quality control in an experimental design strategy to control of the relative quality of the experimental results, for example independent biological replicates made from different individual biosources, or introduction of spikes into hybridizations. Reference: MGED http://mged.sourceforge.net/ontologies/MGEDontology.php
"""^^xsd:string ;
                rdfs:label "QualityControl"^^xsd:string .


###  http://www.hozo.jp/owl/EXPOApr19.xml/Quantity
:Quantity rdf:type owl:Class ;
          rdfs:subClassOf :Abstract ;
          owl:disjointWith :Relation ;
          rdfs:comment """
\"Any specification of how many or how much of something there is. Accordingly, there are two subclasses of Quantity: Number (how many) and PhysicalQuantity (how much).\" (SUMO)
"""^^xsd:string ;
          rdfs:label "Quantity"^^xsd:string .


###  http://www.hozo.jp/owl/EXPOApr19.xml/RandomError
:RandomError rdf:type owl:Class ;
             rdfs:subClassOf :MeasurementError ;
             rdfs:comment """
A random error is an error that is without any regularity or of unknown regularity. Reference: Arley, N. & Buch , K.R., Introduction to the theory of probability and statistics. New York : Wiley London. Chapman & Hall, 1950. 236p.
"""^^xsd:string ;
             rdfs:label "RandomError"^^xsd:string .


###  http://www.hozo.jp/owl/EXPOApr19.xml/RandomSampling
:RandomSampling rdf:type owl:Class ;
                rdfs:subClassOf :SamplingMethod ;
                rdfs:comment """
Random sampling is a sampling method where \"every single individual in the parent group has an equal chance to be chosen in the sample.\"
Reference: Langley, R. Practical Statistics. David&Charles Ltd, Newton,1971.
"""^^xsd:string ;
                rdfs:label "RandomSampling"^^xsd:string .


###  http://www.hozo.jp/owl/EXPOApr19.xml/RecommendationSatus
:RecommendationSatus rdf:type owl:Class ;
                     rdfs:subClassOf :NonRestrictedStatus ;
                     rdfs:comment """
A recommendation is a status of a proposal or suggestion, advice.? Reference: The Oxford English Dictionary. Oxford University Press, 2 Ed., 1989
"""^^xsd:string ;
                     rdfs:label "RecommendationSatus"^^xsd:string .


###  http://www.hozo.jp/owl/EXPOApr19.xml/RecordingAction
:RecordingAction rdf:type owl:Class ;
                 rdfs:subClassOf :ExperimentalAction ;
                 rdfs:comment """
A recording action is an experimental action for preserving information about variables of the experiment for control, analysis, and interpretation of the experimental results.
"""^^xsd:string ;
                 rdfs:label "RecordingAction"^^xsd:string .


###  http://www.hozo.jp/owl/EXPOApr19.xml/Reference
:Reference rdf:type owl:Class ;
           rdfs:subClassOf :RepresentationForm ;
           rdfs:comment """
The concept is outside EXPO
"""^^xsd:string ;
           rdfs:label "Reference"^^xsd:string .


###  http://www.hozo.jp/owl/EXPOApr19.xml/Region
:Region rdf:type owl:Class ;
        rdfs:subClassOf :Object ;
        rdfs:comment """
\"A topographic location. Regions encompass surfaces of Objects, imaginary places, and GeographicAreas. Note that a Region is the only kind of Object which can be located at itself. Note too that Region is not a subclass of SelfConnectedObject, because some Regions, e.g. archipelagos, have parts which are not connected with one another.\" (SUMO)
"""^^xsd:string ;
        rdfs:label "Region"^^xsd:string .


###  http://www.hozo.jp/owl/EXPOApr19.xml/RelatedDomain
:RelatedDomain rdf:type owl:Class ;
               rdfs:subClassOf :FieldOfStudy ;
               rdfs:comment """
A related domain of an experiment is a domain (field of study) to which belong used in the experiment methods, materials, experimental objects, or other entities involved into the experiment, but is not considered as the domain of the experiment.
"""^^xsd:string ;
               rdfs:label "RelatedDomain"^^xsd:string .


###  http://www.hozo.jp/owl/EXPOApr19.xml/Relation
:Relation rdf:type owl:Class ;
          rdfs:subClassOf :Abstract ;
          rdfs:comment """
\"The Class of relations. There are three kinds of Relation: Predicate, Function, and List. Predicates and Functions both denote sets of ordered n-tuples. The difference between these two Classes is that Predicates cover formula-forming operators, while Functions cover term-forming operators. A List, on the other hand, is a particular ordered n-tuple.\" (SUMO)
"""^^xsd:string ;
          rdfs:label "Relation"^^xsd:string .


###  http://www.hozo.jp/owl/EXPOApr19.xml/RepresenationalMedium
:RepresenationalMedium rdf:type owl:Class ;
                       rdfs:subClassOf :Role ;
                       rdfs:comment "the concept is outside EXPO."^^xsd:string ;
                       rdfs:label "RepresenationalMedium"^^xsd:string .


###  http://www.hozo.jp/owl/EXPOApr19.xml/Representation
:Representation rdf:type owl:Class ;
                rdfs:subClassOf :ContentBearingObject ,
                                [ rdf:type owl:Restriction ;
                                  owl:onProperty :has_content ;
                                  owl:allValuesFrom :Proposition
                                ] ,
                                [ rdf:type owl:Restriction ;
                                  owl:onProperty :has_representation_style ;
                                  owl:allValuesFrom :RepresentationForm
                                ] ,
                                [ rdf:type owl:Restriction ;
                                  owl:onProperty :has_content ;
                                  owl:cardinality "1"^^xsd:nonNegativeInteger
                                ] ,
                                [ rdf:type owl:Restriction ;
                                  owl:onProperty :has_representation_style ;
                                  owl:cardinality "1"^^xsd:nonNegativeInteger
                                ] ;
                rdfs:comment """
The concept is outside EXPO
"""^^xsd:string ;
                rdfs:label "Representation"^^xsd:string .


###  http://www.hozo.jp/owl/EXPOApr19.xml/RepresentationExperimentalExecutionProcedure
:RepresentationExperimentalExecutionProcedure rdf:type owl:Class ;
                                              rdfs:subClassOf :Representation ;
                                              owl:disjointWith :RepresentationExperimentalGoal ,
                                                               :RepresentationExperimentalObservation ,
                                                               :RepresentationExperimentalResults ,
                                                               :TechnicalDescription ;
                                              rdfs:comment """
A representation of the experimental execution procedure is the expression of a plan of experimental actions in some accepted scientific form. Reference: Based on The Oxford English Dictionary. Oxford University Press, 2 Ed., 1989
"""^^xsd:string ;
                                              rdfs:label "RepresentationExperimentalExecutionProcedure"^^xsd:string .


###  http://www.hozo.jp/owl/EXPOApr19.xml/RepresentationExperimentalGoal
:RepresentationExperimentalGoal rdf:type owl:Class ;
                                rdfs:subClassOf :Representation ;
                                owl:disjointWith :RepresentationExperimentalObservation ,
                                                 :RepresentationExperimentalResults ,
                                                 :TechnicalDescription ;
                                rdfs:comment """
A representation of an experimental goal is a \"reproduction in some material or tangible form.\" Reference: The Oxford English Dictionary. Oxford University Press, 2 Ed., 1989
"""^^xsd:string ;
                                rdfs:label "RepresentationExperimentalGoal"^^xsd:string .


###  http://www.hozo.jp/owl/EXPOApr19.xml/RepresentationExperimentalObservation
:RepresentationExperimentalObservation rdf:type owl:Class ;
                                       rdfs:subClassOf :Representation ;
                                       owl:disjointWith :RepresentationExperimentalResults ,
                                                        :TechnicalDescription ;
                                       rdfs:comment """
A representation of experimental observations is a reproduction of the observations in some material or tangible form? preferably according to a data representation standard.  Reference: The Oxford English Dictionary. Oxford University Press, 2 Ed., 1989
"""^^xsd:string ;
                                       rdfs:label "RepresentationExperimentalObservation"^^xsd:string .


###  http://www.hozo.jp/owl/EXPOApr19.xml/RepresentationExperimentalResults
:RepresentationExperimentalResults rdf:type owl:Class ;
                                   rdfs:subClassOf :Representation ;
                                   owl:disjointWith :TechnicalDescription ;
                                   rdfs:comment """
A representation of experimental results is a reproduction of the results in some material or tangible form? Reference: The Oxford English Dictionary. Oxford University Press, 2 Ed., 1989
"""^^xsd:string ;
                                   rdfs:label "RepresentationExperimentalResults"^^xsd:string .


###  http://www.hozo.jp/owl/EXPOApr19.xml/RepresentationForm
:RepresentationForm rdf:type owl:Class ;
                    rdfs:subClassOf :Role ,
                                    [ rdf:type owl:Restriction ;
                                      owl:onProperty :has_ ;
                                      owl:allValuesFrom :Artifact
                                    ] ,
                                    [ rdf:type owl:Restriction ;
                                      owl:onProperty :has_expression ;
                                      owl:allValuesFrom :LinguisticExpression
                                    ] ;
                    rdfs:comment """
The concept is outside EXPO
"""^^xsd:string ;
                    rdfs:label "RepresentationForm"^^xsd:string .


###  http://www.hozo.jp/owl/EXPOApr19.xml/Requirements
:Requirements rdf:type owl:Class ;
              rdfs:subClassOf :Proposition ;
              owl:disjointWith :ScientificTask ,
                               :SubjectQualification ,
                               :ValueOfVariable ,
                               :Variable ;
              rdfs:comment """
The concept is outside of EXPO
"""^^xsd:string ;
              rdfs:label "Requirements"^^xsd:string .


###  http://www.hozo.jp/owl/EXPOApr19.xml/ResearchCouncilsUKClassification
:ResearchCouncilsUKClassification rdf:type owl:Class ;
                                  rdfs:subClassOf :ClassificationOfDomains ;
                                  rdfs:comment """
The research councils UK classification is a classification of domains used by Britain's councils for academic research.
"""^^xsd:string ;
                                  rdfs:label "ResearchCouncilsUKClassification"^^xsd:string .


###  http://www.hozo.jp/owl/EXPOApr19.xml/ResearchHypothesis
:ResearchHypothesis rdf:type owl:Class ;
                    rdfs:subClassOf :ExperimentalHypothesis ;
                    rdfs:comment """
A research hypothesis is an experimental hypothesis that states that a known controlled variable or variables has/have a specified effect on the unknown (target) variable or variables of the domain.
"""^^xsd:string ;
                    rdfs:label "ResearchHypothesis"^^xsd:string .


###  http://www.hozo.jp/owl/EXPOApr19.xml/ResearchMethod
:ResearchMethod rdf:type owl:Class ;
                rdfs:subClassOf :Procedure ;
                rdfs:comment """
A research method is a way to solve a scientific task \"based upon or regulated by science, as opposed to mere traditional rules or empirical dexterity.\"
Reference: The Oxford English Dictionary http://dictionary.oed.com
"""^^xsd:string ;
                rdfs:label "ResearchMethod"^^xsd:string .


###  http://www.hozo.jp/owl/EXPOApr19.xml/RestrictedStatus
:RestrictedStatus rdf:type owl:Class ;
                  rdfs:subClassOf :PermissionStatus ;
                  rdfs:comment """
A restricted status is a status which controls in some way the access to a SOP, a protocol, and/ or experimental results.
"""^^xsd:string ;
                  rdfs:label "RestrictedStatus"^^xsd:string .


###  http://www.hozo.jp/owl/EXPOApr19.xml/ResultError
:ResultError rdf:type owl:Class ;
             rdfs:subClassOf :Error ;
             rdfs:comment """
A result error is an incorrectly inferred conclusion about: a research hypothesis, such as an hypothesis acceptance mistake (e.g. false positive); or about the phenomena involved in the experiment.
"""^^xsd:string ;
             rdfs:label "ResultError"^^xsd:string .


###  http://www.hozo.jp/owl/EXPOApr19.xml/ResultEvaluating
:ResultEvaluating rdf:type owl:Class ;
                  rdfs:subClassOf :ScientificActivity ;
                  rdfs:comment """
Result evaluating is the act of determining the value of experimental results. Reference: Based on The Oxford English Dictionary. Oxford University Press, 2 Ed., 1989
"""^^xsd:string ;
                  rdfs:label "ResultEvaluating"^^xsd:string .


###  http://www.hozo.jp/owl/EXPOApr19.xml/ResultsEvaluation
:ResultsEvaluation rdf:type owl:Class ;
                   rdfs:subClassOf :ScientificTask ;
                   owl:disjointWith :ResultsInterpretation ;
                   rdfs:comment """
Results evaluation is the scientific task to working out the value of an experimental result; or in general, to express the result in terms of something already known. Reference: Based on The Oxford English Dictionary. Oxford University Press, 2 Ed., 1989
"""^^xsd:string ;
                   rdfs:label "ResultsEvaluation"^^xsd:string .


###  http://www.hozo.jp/owl/EXPOApr19.xml/ResultsInterpretation
:ResultsInterpretation rdf:type owl:Class ;
                       rdfs:subClassOf :ScientificTask ;
                       rdfs:comment """
Results interpretation is the scientific task of explaining, the meaning of experimental results. Reference: Based on The Oxford English Dictionary. Oxford University Press, 2 Ed., 1989
"""^^xsd:string ;
                       rdfs:label "ResultsInterpretation"^^xsd:string .


###  http://www.hozo.jp/owl/EXPOApr19.xml/Robot
:Robot rdf:type owl:Class ;
       rdfs:subClassOf :SentientAgent ;
       rdfs:comment "the concept is outside EXPO."^^xsd:string ;
       rdfs:label "Robot"^^xsd:string .


###  http://www.hozo.jp/owl/EXPOApr19.xml/Robustness
:Robustness rdf:type owl:Class ;
            rdfs:subClassOf :StatisticsCharacteristic ;
            owl:disjointWith :Validity ;
            rdfs:comment """
The concept is outside of EXPO
"""^^xsd:string ;
            rdfs:label "Robustness"^^xsd:string .


###  http://www.hozo.jp/owl/EXPOApr19.xml/Role
:Role rdf:type owl:Class ;
      rdfs:subClassOf :Predicate ;
      rdfs:comment """
(role ?OBJECT ?ENTITY) means that ?OBJECT - a Role holder, plays a  Role ?ENTITY   in some context. In EXPO we always consider the context: experiment. For example in context of experiment an object <human> can play the role <subject of experiment> if the human is \"one who executes the experiment\" (OED) or the role <object of experiment> if the human is one \"on whom an experiment is made.\" (OED).
"""^^xsd:string ;
      rdfs:label "Role"^^xsd:string .


###  http://www.hozo.jp/owl/EXPOApr19.xml/SUMOSynonym
:SUMOSynonym rdf:type owl:Class ;
             rdfs:subClassOf :SynonymousExternalConcept ;
             rdfs:comment """
A SUMO synonym is a synonymous concept between the SUMO ontology concept and the concept.
"""^^xsd:string ;
             rdfs:label "SUMOSynonym"^^xsd:string .


###  http://www.hozo.jp/owl/EXPOApr19.xml/Sample
:Sample rdf:type owl:Class ;
        rdfs:subClassOf :ObjectOfExperiment ;
        rdfs:comment """
A sample is \"a portion drawn from a population (EXPO: <parent group>), the study of which is intended to lead to statistical estimates of the attributes of the whole population.\" Reference: The Oxford English Dictionary. Oxford University Press, 2 Ed., 1989
"""^^xsd:string ;
        rdfs:label "Sample"^^xsd:string .


###  http://www.hozo.jp/owl/EXPOApr19.xml/SampleForming
:SampleForming rdf:type owl:Class ;
               rdfs:subClassOf :DesigningExperiment ;
               rdfs:comment """
Sample forming is an act of composing a sample for the experiment.
"""^^xsd:string ;
               rdfs:label "SampleForming"^^xsd:string .


###  http://www.hozo.jp/owl/EXPOApr19.xml/SampleRepresentativeness
:SampleRepresentativeness rdf:type owl:Class ;
                          rdfs:subClassOf :AttributeSample ;
                          owl:disjointWith :SampleSize ;
                          rdfs:comment """
Sample representativeness is an attribute of a sample which characterizes how the sample is representative for analysis and  estimation the characteristics of a the parent group.
"""^^xsd:string ;
                          rdfs:label "SampleRepresentativeness"^^xsd:string .


###  http://www.hozo.jp/owl/EXPOApr19.xml/SampleSize
:SampleSize rdf:type owl:Class ;
            rdfs:subClassOf :AttributeSample ;
            rdfs:comment """
The sample size is a number of members of the sample.
"""^^xsd:string ;
            rdfs:label "SampleSize"^^xsd:string .


###  http://www.hozo.jp/owl/EXPOApr19.xml/SamplingMethod
:SamplingMethod rdf:type owl:Class ;
                rdfs:subClassOf :ExperimentalMethod ;
                rdfs:comment """
A sampling method is a way to form a sample, an object of the experiment.
"""^^xsd:string ;
                rdfs:label "SamplingMethod"^^xsd:string .


###  http://www.hozo.jp/owl/EXPOApr19.xml/SamplingRule
:SamplingRule rdf:type owl:Class ;
              rdfs:subClassOf :ExperimentalRule ;
              rdfs:comment """
A sampling rule is \"a prescribed method for finding\" a member of a sample. 
Reference: The Oxford English Dictionary. Oxford University Press, 2 Ed., 1989
"""^^xsd:string ;
              rdfs:label "SamplingRule"^^xsd:string .


###  http://www.hozo.jp/owl/EXPOApr19.xml/ScientificActivity
:ScientificActivity rdf:type owl:Class ;
                    rdfs:subClassOf :Process ;
                    rdfs:comment """
Scientific activity is the process of performing a scientific task.
"""^^xsd:string ;
                    rdfs:label "ScientificActivity"^^xsd:string .


###  http://www.hozo.jp/owl/EXPOApr19.xml/ScientificExperiment
:ScientificExperiment rdf:type owl:Class ;
                      rdfs:subClassOf :Procedure ,
                                      [ rdf:type owl:Restriction ;
                                        owl:onProperty :has_ExperimentalDesign ;
                                        owl:allValuesFrom :ExperimentalDesign
                                      ] ,
                                      [ rdf:type owl:Restriction ;
                                        owl:onProperty :has_admin_info ;
                                        owl:allValuesFrom :AdminInfoExperiment
                                      ] ,
                                      [ rdf:type owl:Restriction ;
                                        owl:onProperty :has_classification ;
                                        owl:allValuesFrom :ClassificationOfExperiments
                                      ] ,
                                      [ rdf:type owl:Restriction ;
                                        owl:onProperty :has_goal ;
                                        owl:allValuesFrom :ExperimentalGoal
                                      ] ;
                      rdfs:comment """
A scientific experiment is a research method which permits the investigation of cause-effect relations between known and unknown (target) variables of the field of study (domain). An experimental result cannot be known with certainty in advance.
"""^^xsd:string ;
                      rdfs:label "ScientificExperiment"^^xsd:string .


###  http://www.hozo.jp/owl/EXPOApr19.xml/ScientificInvestigation
:ScientificInvestigation rdf:type owl:Class ;
                         rdfs:subClassOf :Procedure ,
                                         [ rdf:type owl:Restriction ;
                                           owl:onProperty :has_experiment ;
                                           owl:allValuesFrom :ScientificExperiment
                                         ] ,
                                         [ rdf:type owl:Restriction ;
                                           owl:onProperty :has_experimental_design ;
                                           owl:allValuesFrom :ExperimentalDesign
                                         ] ,
                                         [ rdf:type owl:Restriction ;
                                           owl:onProperty :has_hypothesis_formation ;
                                           owl:allValuesFrom :HypothesisFormation
                                         ] ,
                                         [ rdf:type owl:Restriction ;
                                           owl:onProperty :has_information_gethering ;
                                           owl:allValuesFrom :InformationGethering
                                         ] ,
                                         [ rdf:type owl:Restriction ;
                                           owl:onProperty :has_problem_analysis ;
                                           owl:allValuesFrom :PoblemAnalysis
                                         ] ,
                                         [ rdf:type owl:Restriction ;
                                           owl:onProperty :has_result_evaluation ;
                                           owl:allValuesFrom :ResultsEvaluation
                                         ] ,
                                         [ rdf:type owl:Restriction ;
                                           owl:onProperty :has_result_interpretation ;
                                           owl:allValuesFrom :ResultsInterpretation
                                         ] ;
                         rdfs:comment """
Scientific investigation is a systematic examination; careful and detailed research. Reference: The Oxford English Dictionary. Oxford University Press, 2 Ed., 1989
"""^^xsd:string ;
                         rdfs:label "ScientificInvestigation"^^xsd:string .


###  http://www.hozo.jp/owl/EXPOApr19.xml/ScientificTask
:ScientificTask rdf:type owl:Class ;
                rdfs:subClassOf :Proposition ;
                owl:disjointWith :SubjectQualification ,
                                 :ValueOfVariable ,
                                 :Variable ;
                rdfs:comment """
A scientific task is a portion of scientific study. Reference: Based on The Oxford English Dictionary. Oxford University Press, 2 Ed., 1989
"""^^xsd:string ;
                rdfs:label "ScientificTask"^^xsd:string .


###  http://www.hozo.jp/owl/EXPOApr19.xml/SelfConnectedObject
:SelfConnectedObject rdf:type owl:Class ;
                     rdfs:subClassOf :Object ;
                     rdfs:comment """
\"A SelfConnectedObject is any Object that does not consist of two or more disconnected parts.\" (SUMO)
"""^^xsd:string ;
                     rdfs:label "SelfConnectedObject"^^xsd:string .


###  http://www.hozo.jp/owl/EXPOApr19.xml/Sentence
:Sentence rdf:type owl:Class ;
          rdfs:subClassOf :LinguisticExpression ;
          rdfs:comment """
\"A syntactically well-formed formula of a Language. It includes, at minimum, a predicate and a subject (which may be explicit or implicit), and it expresses a Proposition.\" (SUMO)
"""^^xsd:string ;
          rdfs:label "Sentence"^^xsd:string .


###  http://www.hozo.jp/owl/EXPOApr19.xml/SentientAgent
:SentientAgent rdf:type owl:Class ;
               rdfs:subClassOf :Agent ;
               rdfs:comment """
\"An Agent that has rights but may or may not have responsibilities and the ability to reason. If the latter are present, then the Agent is also an instance of CognitiveAgent. Domesticated animals are an example of SentientAgents that are not also CognitiveAgents.\" (SUMO)
"""^^xsd:string ;
               rdfs:label "SentientAgent"^^xsd:string .


###  http://www.hozo.jp/owl/EXPOApr19.xml/SequentialDesign
:SequentialDesign rdf:type owl:Class ;
                  rdfs:subClassOf :ExperimentalDesign ;
                  rdfs:comment """
A sequential design is an experimental design where a sample group size of experimental objects is not determined in advance. The experiment is continued until the moment when the results are conclusive according to predetermined degree of significance or non-significance.
Reference:  Based on Langley, R. Practical Statistics. David&Charles Ltd, Newton,1971.

Reference:  Based on: Langley, R. Practical Statistics. David&Charles Ltd, Newton,1971.
"""^^xsd:string ;
                  rdfs:label "SequentialDesign"^^xsd:string .


###  http://www.hozo.jp/owl/EXPOApr19.xml/SingleHypothesis
:SingleHypothesis rdf:type owl:Class ;
                  rdfs:subClassOf :HypothesisComplexity ;
                  rdfs:comment """
A single hypothesis of an experimental hypothesis is a Boolean attribute which is true when the hypothesis can be formalized by a single clause.
"""^^xsd:string ;
                  rdfs:label "SingleHypothesis"^^xsd:string .


###  http://www.hozo.jp/owl/EXPOApr19.xml/Software
:Software rdf:type owl:Class ;
          rdfs:subClassOf :ExperimentalEquipment ;
          rdfs:comment """
the concept is outside of EXPO
"""^^xsd:string ;
          rdfs:label "Software"^^xsd:string .


###  http://www.hozo.jp/owl/EXPOApr19.xml/Sound
:Sound rdf:type owl:Class ;
       rdfs:subClassOf :RepresentationForm ;
       rdfs:comment """
Dublin Core: http://www.lub.lu.se/cgi-bin/nmdc.pl
"""^^xsd:string ;
       rdfs:label "Sound"^^xsd:string .


###  http://www.hozo.jp/owl/EXPOApr19.xml/SplitSamples
:SplitSamples rdf:type owl:Class ;
              rdfs:subClassOf :PairedComparisonOfMatchingGroups ;
              owl:disjointWith :SymmetricalMatching ;
              rdfs:comment """
Split samples is a matching groups experimental design strategy where each member of a sample group of experimental objects is divided into two parts in order to form two groups for the experiment. Reference:  Based on: Langley, R. Practical Statistics. David&Charles Ltd, Newton,1971.
"""^^xsd:string ;
              rdfs:label "SplitSamples"^^xsd:string .


###  http://www.hozo.jp/owl/EXPOApr19.xml/StandardOperatingProcedure
:StandardOperatingProcedure rdf:type owl:Class ;
                            rdfs:subClassOf :ProcedureExecuteExperiment ,
                                            [ rdf:type owl:Restriction ;
                                              owl:onProperty :has_author ;
                                              owl:allValuesFrom :AuthorSOP
                                            ] ,
                                            [ rdf:type owl:Restriction ;
                                              owl:onProperty :has_latest_modification ;
                                              owl:allValuesFrom :TimePoint
                                            ] ,
                                            [ rdf:type owl:Restriction ;
                                              owl:onProperty :has_procedure ;
                                              owl:allValuesFrom :ProcedureExecuteExperiment
                                            ] ,
                                            [ rdf:type owl:Restriction ;
                                              owl:onProperty :has_representation ;
                                              owl:allValuesFrom :BiblioReference
                                            ] ,
                                            [ rdf:type owl:Restriction ;
                                              owl:onProperty :has_latest_modification ;
                                              owl:cardinality "1"^^xsd:nonNegativeInteger
                                            ] ;
                            rdfs:comment """
A standard operating procedure is a prescribed procedure to be followed routinely. Reference: HyperDictionary:  http://searchbox.hyperdictionary.com/dictionary/standard+operating+procedure
"""^^xsd:string ;
                            rdfs:label "StandardOperatingProcedure"^^xsd:string .


###  http://www.hozo.jp/owl/EXPOApr19.xml/StaticModel
:StaticModel rdf:type owl:Class ;
             rdfs:subClassOf :DynamismOfModel ;
             rdfs:comment """
A static model of the experiment is a model which remains unchanged during the period of the experiment.
"""^^xsd:string ;
             rdfs:label "StaticModel"^^xsd:string .


###  http://www.hozo.jp/owl/EXPOApr19.xml/StatisticalError
:StatisticalError rdf:type owl:Class ;
                  rdfs:subClassOf :RandomError ;
                  rdfs:comment """
Statistical error is a random error which can be described by statistical laws.
"""^^xsd:string ;
                  rdfs:label "StatisticalError"^^xsd:string .


###  http://www.hozo.jp/owl/EXPOApr19.xml/StatisticsCharacteristic
:StatisticsCharacteristic rdf:type owl:Class ;
                          rdfs:subClassOf :Attribute ;
                          rdfs:comment """
The concept is outside of EXPO
"""^^xsd:string ;
                          rdfs:label "StatisticsCharacteristic"^^xsd:string .


###  http://www.hozo.jp/owl/EXPOApr19.xml/StatusExperimentalDocument
:StatusExperimentalDocument rdf:type owl:Class ;
                            rdfs:subClassOf :AttributeOfDocument ;
                            rdfs:comment """
A status of an experimental document is a permission status or a document stage.
"""^^xsd:string ;
                            rdfs:label "StatusExperimentalDocument"^^xsd:string .


###  http://www.hozo.jp/owl/EXPOApr19.xml/StratifiedSampling
:StratifiedSampling rdf:type owl:Class ;
                    rdfs:subClassOf :SamplingMethod ;
                    rdfs:comment """
Stratified sampling is a sampling method where a random sample is taking from different levels (strata) of the parent group. Reference: Based on Langley, R. Practical Statistics. David&Charles Ltd, Newton,1971.
"""^^xsd:string ;
                    rdfs:label "StratifiedSampling"^^xsd:string .


###  http://www.hozo.jp/owl/EXPOApr19.xml/SubjectEffect
:SubjectEffect rdf:type owl:Class ;
               rdfs:subClassOf :AlternativeHypothesis ;
               owl:disjointWith :TimeEffect ;
               rdfs:comment """
A subject effect is an alternative hypothesis where an effect on the experimental results is due to difference in subjects or subjects? action or expectations.
"""^^xsd:string ;
               rdfs:label "SubjectEffect"^^xsd:string .


###  http://www.hozo.jp/owl/EXPOApr19.xml/SubjectMethod
:SubjectMethod rdf:type owl:Class ;
               rdfs:subClassOf :SubjectRole ;
               rdfs:comment """
A subject of a method is: \"one who executes the method.\" For instance: a <human>, a <robot>. Reference: Based on The Oxford English Dictionary. Oxford University Press, 2 Ed., 1989
"""^^xsd:string ;
               rdfs:label "SubjectMethod"^^xsd:string .


###  http://www.hozo.jp/owl/EXPOApr19.xml/SubjectOfAction
:SubjectOfAction rdf:type owl:Class ;
                 rdfs:subClassOf :SubjectOfExperiment ;
                 rdfs:comment """
A subject of an action is: \"one who executes the action\" For instance: a <human>, a <robot>. Reference: Based on The Oxford English Dictionary. Oxford University Press, 2 Ed., 1989"""^^xsd:string .


###  http://www.hozo.jp/owl/EXPOApr19.xml/SubjectOfExperiment
:SubjectOfExperiment rdf:type owl:Class ;
                     rdfs:subClassOf :SubjectRole ,
                                     [ rdf:type owl:Restriction ;
                                       owl:onProperty :has_admin_info ;
                                       owl:allValuesFrom :AdminInfoSubjectOfExperiment
                                     ] ,
                                     [ rdf:type owl:Restriction ;
                                       owl:onProperty :has_admin_info ;
                                       owl:cardinality "1"^^xsd:nonNegativeInteger
                                     ] ;
                     rdfs:comment """
A subject of an experimental is: \"one who executes the experiment\" For instance: a <human>, a <robot>. Reference: The Oxford English Dictionary. Oxford University Press, 2 Ed., 1989
"""^^xsd:string ;
                     rdfs:label "SubjectOfExperiment"^^xsd:string .


###  http://www.hozo.jp/owl/EXPOApr19.xml/SubjectQualification
:SubjectQualification rdf:type owl:Class ;
                      rdfs:subClassOf :Proposition ;
                      owl:disjointWith :ValueOfVariable ,
                                       :Variable ;
                      rdfs:comment """
Subject qualification is a \"formal certification, issued by a relevant approved body, in recognition that a person has achieved competency relevant to identified individual, professional, industry or community needs.\" Reference: Training: www.training.wa.gov.au/publications/cbt/framework/glossary.htm
"""^^xsd:string ;
                      rdfs:label "SubjectQualification"^^xsd:string .


###  http://www.hozo.jp/owl/EXPOApr19.xml/SubjectRole
:SubjectRole rdf:type owl:Class ;
             rdfs:subClassOf :ActorRole ;
             rdfs:comment """
the concept is outside EXPO.
"""^^xsd:string ;
             rdfs:label "SubjectRole"^^xsd:string .


###  http://www.hozo.jp/owl/EXPOApr19.xml/SubjectsComparison
:SubjectsComparison rdf:type owl:Class ;
                    rdfs:subClassOf :PairedComparisonOfSingleSampleGroups ;
                    rdfs:comment """
A subjects comparison is a paired comparison of single sample groups experimental design strategy where effects on the results of different subjects of the experiment are compared. Reference:  Based on: Langley, R. Practical Statistics. David&Charles Ltd, Newton,1971.
"""^^xsd:string ;
                    rdfs:label "SubjectsComparison"^^xsd:string .


###  http://www.hozo.jp/owl/EXPOApr19.xml/Submitter
:Submitter rdf:type owl:Class ;
           rdfs:subClassOf :SubjectRole ,
                           [ rdf:type owl:Restriction ;
                             owl:onProperty :has_admin_info ;
                             owl:allValuesFrom :AdminInfoSubmitter
                           ] ,
                           [ rdf:type owl:Restriction ;
                             owl:onProperty :has_admin_info ;
                             owl:cardinality "1"^^xsd:nonNegativeInteger
                           ] ;
           rdfs:comment """
A submitter of a protocol, a SOP, experimental results, etc. is the person (or a group) who submits the document. Reference: Based on The Oxford English Dictionary. Oxford University Press, 2 Ed., 1989
"""^^xsd:string ;
           rdfs:label "Submitter"^^xsd:string .


###  http://www.hozo.jp/owl/EXPOApr19.xml/Summary
:Summary rdf:type owl:Class ;
         rdfs:subClassOf :Text ;
         rdfs:comment """
\"A short Text that is a summary of another, longer Text.\"
Reference: SUMO: http://www.ontologyportal.org/
"""^^xsd:string ;
         rdfs:label "Summary"^^xsd:string .


###  http://www.hozo.jp/owl/EXPOApr19.xml/SymmetricalMatching
:SymmetricalMatching rdf:type owl:Class ;
                     rdfs:subClassOf :PairedComparisonOfMatchingGroups ;
                     rdfs:comment """
Symmetrical matching is a matching groups experimental design strategy where pairs are symmetrical parts of a body. For instance comparing the effect of 2 ointments applied to 2 arms. Reference:  Based on: Langley, R. Practical Statistics. David&Charles Ltd, Newton,1971.
"""^^xsd:string ;
                     rdfs:label "SymmetricalMatching"^^xsd:string .


###  http://www.hozo.jp/owl/EXPOApr19.xml/SynonymousExternalConcept
:SynonymousExternalConcept rdf:type owl:Class ;
                           rdfs:subClassOf :AttributeRole ,
                                           [ rdf:type owl:Restriction ;
                                             owl:onProperty :has_EXPO_concept ;
                                             owl:allValuesFrom :Name
                                           ] ,
                                           [ rdf:type owl:Restriction ;
                                             owl:onProperty :has_synonymousExternalConcept ;
                                             owl:allValuesFrom :Name
                                           ] ,
                                           [ rdf:type owl:Restriction ;
                                             owl:onProperty :has_EXPO_concept ;
                                             owl:cardinality "1"^^xsd:nonNegativeInteger
                                           ] ;
                           rdfs:comment """
SUMO: http://www.ontologyportal.org/
"""^^xsd:string ;
                           rdfs:label "SynonymousExternalConcept"^^xsd:string .


###  http://www.hozo.jp/owl/EXPOApr19.xml/SystematicError
:SystematicError rdf:type owl:Class ;
                 rdfs:subClassOf :MeasurementError ;
                 rdfs:comment """
A systematic error is an error due to a definite cause acting according to a definite law. Reference: Arley, N. & Buch , K.R., Introduction to the theory of probability and statistics. New York : Wiley London. Chapman & Hall, 1950. 236p.
"""^^xsd:string ;
                 rdfs:label "SystematicError"^^xsd:string .


###  http://www.hozo.jp/owl/EXPOApr19.xml/SystematicSampling
:SystematicSampling rdf:type owl:Class ;
                    rdfs:subClassOf :SamplingMethod ,
                                    [ rdf:type owl:Restriction ;
                                      owl:onProperty :has_sampling_rule ;
                                      owl:allValuesFrom :SamplingRule
                                    ] ;
                    rdfs:comment """
Systematic sampling is a sampling method where each member of a sample is selecting according to a definite rule (except of random choice).
"""^^xsd:string ;
                    rdfs:label "SystematicSampling"^^xsd:string .


###  http://www.hozo.jp/owl/EXPOApr19.xml/TargetVariable
:TargetVariable rdf:type owl:Class ;
                rdfs:subClassOf :Variable ;
                rdfs:comment """
A target variable is an unknown variable of the domain model about which the experiment is designed to discover new knowledge.
"""^^xsd:string ;
                rdfs:label "TargetVariable"^^xsd:string .


###  http://www.hozo.jp/owl/EXPOApr19.xml/TaskRole
:TaskRole rdf:type owl:Class ;
          rdfs:subClassOf :Role ;
          rdfs:comment """the concept is outside EXPO.
EX: Symptom role (Fault Diagnosis; Conclusion role (Reasoning)
"""^^xsd:string ;
          rdfs:label "TaskRole"^^xsd:string .


###  http://www.hozo.jp/owl/EXPOApr19.xml/TechnicalDescription
:TechnicalDescription rdf:type owl:Class ;
                      rdfs:subClassOf :Representation ;
                      rdfs:comment """
A technical description is a representation of technical information about experimental equipment or a subject (robot) in order to provide the user with information about a technology's purpose and functions, components and construction, and operation and maintenance? Reference: UA: http://www.u.arizona.edu/~menchaca/engl308/assignments/descriptions.htm
"""^^xsd:string ;
                      rdfs:label "TechnicalDescription"^^xsd:string .


###  http://www.hozo.jp/owl/EXPOApr19.xml/TechnicalReport
:TechnicalReport rdf:type owl:Class ;
                 rdfs:subClassOf :Text ;
                 rdfs:comment """
Dublin Core: http://www.lub.lu.se/cgi-bin/nmdc.pl
"""^^xsd:string ;
                 rdfs:label "TechnicalReport"^^xsd:string .


###  http://www.hozo.jp/owl/EXPOApr19.xml/TestingEffect
:TestingEffect rdf:type owl:Class ;
               rdfs:subClassOf :SubjectEffect ;
               rdfs:comment """
A testing effect is a subject effect where the results are due to the data gathering procedures. Reference: Davis, J., Psychological research methods.
"""^^xsd:string ;
               rdfs:label "TestingEffect"^^xsd:string .


###  http://www.hozo.jp/owl/EXPOApr19.xml/Text
:Text rdf:type owl:Class ;
      rdfs:subClassOf :Artifact ;
      rdfs:comment """
\"A LinguisticExpression or set of LinguisticExpressions that perform a specific function related to Communication, e.g. express a discourse about a particular topic, and that are inscribed in a CorpuscularObject by Humans.\"
SUMO: http://www.ontologyportal.org/
"""^^xsd:string ;
      rdfs:label "Text"^^xsd:string .


###  http://www.hozo.jp/owl/EXPOApr19.xml/TimeCourse
:TimeCourse rdf:type owl:Class ;
            rdfs:subClassOf :ComparisonControl_TargetGroups ;
            owl:disjointWith :Treated_Untreated ;
            rdfs:comment """
A time course design strategy is a sub-class of a comparison control/ target groups strategy where an experimental factor is time.
"""^^xsd:string ;
            rdfs:label "TimeCourse"^^xsd:string .


###  http://www.hozo.jp/owl/EXPOApr19.xml/TimeDuration
:TimeDuration rdf:type owl:Class ;
              rdfs:subClassOf :TimeMeasure ;
              owl:disjointWith :TimePosition ;
              rdfs:comment """
\"Any measure of length of time, with or without respect to the universal timeline.\" (SUMO)
"""^^xsd:string ;
              rdfs:label "TimeDuration"^^xsd:string .


###  http://www.hozo.jp/owl/EXPOApr19.xml/TimeEffect
:TimeEffect rdf:type owl:Class ;
            rdfs:subClassOf :AlternativeHypothesis ;
            rdfs:comment """
A time effect is an alternative hypothesis where an effect on the experimental results is due to uncontrolled changes over time.
"""^^xsd:string ;
            rdfs:label "TimeEffect"^^xsd:string .


###  http://www.hozo.jp/owl/EXPOApr19.xml/TimeInterval
:TimeInterval rdf:type owl:Class ;
              rdfs:subClassOf :TimePosition ;
              owl:disjointWith :TimePoint ;
              rdfs:comment """
\"An interval of time. Note that a TimeInterval has both an extent and a location on the universal timeline. Note too that a TimeInterval has no gaps, i.e. this class contains only convex time intervals.\" SUMO: http://www.ontologyportal.org/
"""^^xsd:string ;
              rdfs:label "TimeInterval"^^xsd:string .


###  http://www.hozo.jp/owl/EXPOApr19.xml/TimeMeasure
:TimeMeasure rdf:type owl:Class ;
             rdfs:subClassOf :PhysicalQuantity ;
             rdfs:comment """
\"The class of temporal durations (instances of TimeDuration) and positions of TimePoints and TimeIntervals along the universal timeline (instances of TimePosition).\" (SUMO)
"""^^xsd:string ;
             rdfs:label "TimeMeasure"^^xsd:string .


###  http://www.hozo.jp/owl/EXPOApr19.xml/TimePoint
:TimePoint rdf:type owl:Class ;
           rdfs:subClassOf :TimePosition ;
           rdfs:comment """
\"An extensionless point on the universal timeline. The TimePoints at which Processes occur can be known with various degrees of precision and approximation, but conceptually TimePoints are point-like and not interval-like. That is, it doesn't make sense to talk about how long a TimePoint lasts.\" SUMO: http://www.ontologyportal.org/
"""^^xsd:string ;
           rdfs:label "TimePoint"^^xsd:string .


###  http://www.hozo.jp/owl/EXPOApr19.xml/TimePosition
:TimePosition rdf:type owl:Class ;
              rdfs:subClassOf :TimeMeasure ;
              rdfs:comment """
\"Any TimePoint or TimeInterval along the universal timeline from NegativeInfinity to PositiveInfinity.\" (SUMO)
"""^^xsd:string ;
              rdfs:label "TimePosition"^^xsd:string .


###  http://www.hozo.jp/owl/EXPOApr19.xml/Title
:Title rdf:type owl:Class ;
       rdfs:subClassOf :Name ;
       rdfs:comment """
The concept is outside of EXPO;
\"The name given to the resource by the CREATOR or PUBLISHER.\"
Reference: Dublin Core: http://www.lub.lu.se/cgi-bin/nmdc.pl
"""^^xsd:string ;
       rdfs:label "Title"^^xsd:string .


###  http://www.hozo.jp/owl/EXPOApr19.xml/TitleExperiment
:TitleExperiment rdf:type owl:Class ;
                 rdfs:subClassOf :Title ;
                 rdfs:comment """
The title of an experiment is a descriptive heading name that refers to the experiment.
"""^^xsd:string ;
                 rdfs:label "TitleExperiment"^^xsd:string .


###  http://www.hozo.jp/owl/EXPOApr19.xml/Tool
:Tool rdf:type owl:Class ;
      rdfs:subClassOf :ExperimentalEquipment ;
      rdfs:comment """
A tool is an instrument for making material changes on other objects, as by cutting, shearing, striking, rubbing, grinding, squeezing, measuring, or other process. Reference: Encyclopaedia Britannica online: http://www.britannica.com/
"""^^xsd:string ;
      rdfs:label "Tool"^^xsd:string .


###  http://www.hozo.jp/owl/EXPOApr19.xml/Treated_Untreated
:Treated_Untreated rdf:type owl:Class ;
                   rdfs:subClassOf :ComparisonControl_TargetGroups ;
                   rdfs:comment """
A treated/ untreated design strategy is a sub-class of a comparison control/ target groups strategy where the target group receives a specified treatment.
"""^^xsd:string ;
                   rdfs:label "Treated/Untreated"^^xsd:string .


###  http://www.hozo.jp/owl/EXPOApr19.xml/Two-factorExperiment
:Two-factorExperiment rdf:type owl:Class ;
                      rdfs:subClassOf :ClassificationByModel ;
                      rdfs:comment """
A two-factor experiment is an experiment with a model containing two fixed controllable variables.
"""^^xsd:string ;
                      rdfs:label "Two-factorExperiment"^^xsd:string .


###  http://www.hozo.jp/owl/EXPOApr19.xml/URL
:URL rdf:type owl:Class ;
     rdfs:subClassOf :Reference ;
     rdfs:comment """
The concept is outside EXPO
"""^^xsd:string ;
     rdfs:label "URL"^^xsd:string .


###  http://www.hozo.jp/owl/EXPOApr19.xml/User
:User rdf:type owl:Class ;
      rdfs:subClassOf :SubjectRole ,
                      [ rdf:type owl:Restriction ;
                        owl:onProperty :has_admin_info ;
                        owl:allValuesFrom :AdminInfoUser
                      ] ,
                      [ rdf:type owl:Restriction ;
                        owl:onProperty :has_login ;
                        owl:allValuesFrom :LoginName
                      ] ,
                      [ rdf:type owl:Restriction ;
                        owl:onProperty :has_pasword ;
                        owl:allValuesFrom :Password
                      ] ,
                      [ rdf:type owl:Restriction ;
                        owl:onProperty :has_admin_info ;
                        owl:cardinality "1"^^xsd:nonNegativeInteger
                      ] ;
      rdfs:comment """
A user is a person or organization that makes use of a protocol, a SOP, experimental results, etc. Reference: Based on The Oxford English Dictionary. Oxford University Press, 2 Ed., 1989
"""^^xsd:string ;
      rdfs:label "User"^^xsd:string .


###  http://www.hozo.jp/owl/EXPOApr19.xml/Validity
:Validity rdf:type owl:Class ;
          rdfs:subClassOf :StatisticsCharacteristic ;
          rdfs:comment """
The concept is outside of EXPO.  The extent to which a test measures what it suppose to measure.  Georgetown: http://www.georgetown.edu/departments/psychology/researchmethods/glossary.htm#dependentvariable
"""^^xsd:string ;
          rdfs:label "Validity"^^xsd:string .


###  http://www.hozo.jp/owl/EXPOApr19.xml/ValueEstimate
:ValueEstimate rdf:type owl:Class ;
               rdfs:subClassOf :ComputationalData ,
                               [ rdf:type owl:Restriction ;
                                 owl:onProperty :has_value_of_variable_ ;
                                 owl:allValuesFrom :ValueOfVariable
                               ] ;
               rdfs:comment """
Value estimate is \"an approximate calculation of quantity or degree or worth\" of the value of a variable. Reference: WordNet: http://www.answers.com
"""^^xsd:string ;
               rdfs:label "ValueEstimate"^^xsd:string .


###  http://www.hozo.jp/owl/EXPOApr19.xml/ValueOfVariable
:ValueOfVariable rdf:type owl:Class ;
                 rdfs:subClassOf :Proposition ;
                 owl:disjointWith :Variable ;
                 rdfs:comment """
A value of an experimental variable is \"the particular quantity, number or amount\" of the variable. Reference: Collins Softback English Dictionary, HarperCollins Publishers, Glasgow, 1993.
"""^^xsd:string ;
                 rdfs:label "ValueOfVariable"^^xsd:string .


###  http://www.hozo.jp/owl/EXPOApr19.xml/Variability
:Variability rdf:type owl:Class ;
             rdfs:subClassOf :AttributeGroup ;
             rdfs:comment """
Variability is an essential characteristic of a group of experimental objects, \"quality of being variable in some respect\". Reference: The Oxford English Dictionary. Oxford University Press, 2 Ed., 1989
"""^^xsd:string ;
             rdfs:label "Variability"^^xsd:string .


###  http://www.hozo.jp/owl/EXPOApr19.xml/Variable
:Variable rdf:type owl:Class ;
          rdfs:subClassOf :Proposition ;
          rdfs:comment """
The concept is outside of EXPO
"""^^xsd:string ;
          rdfs:label "Variable"^^xsd:string .


###  Generated by the OWL API (version 4.5.9.2019-02-01T07:24:44Z) https://github.com/owlcs/owlapi
